{
  "processInformation": {
    "dataSetInformation": {
      "UUID": "073460b5-315d-4480-af0f-e54b496204cd",
      "name": {
        "baseName": [
          {
            "value": "Tropea S Block",
            "lang": "en"
          }
        ]
      },
      "classificationInformation": {
        "classification": [
          {
            "class": [
              {
                "value": "Other transportable goods, except metal products, machinery and equipment",
                "level": 0,
                "classId": "3"
              },
              {
                "value": "Rubber and plastics products",
                "level": 1,
                "classId": "36"
              }
            ],
            "name": "CPC 2.1"
          }
        ]
      },
      "generalComment": [
        {
          "value": "EPDITALY0174\r\nViene considerato l'intero ciclo di vita del prodotto dalla culla alla tomba \u201cfrom cradle to grave\" e i moduli di seguito descritti: A1, A2, A3, A4, A5, B6, C1, C2, C3, C4, D",
          "lang": "en"
        }
      ]
    },
    "quantitativeReference": {
      "referenceToReferenceFlow": [
        1
      ],
      "type": "Reference flow(s)"
    },
    "time": {
      "referenceYear": 2019,
      "dataSetValidUntil": 2026,
      "timeRepresentativenessDescription": [
        {
          "value": "dal 21/10/2021 al 21/10/2026 (Reference year: anno di raccolta dati 2019)",
          "lang": "en"
        }
      ],
      "other": {
        "anies": [
          {
            "name": "publicationDateOfEPD",
            "value": 1639094400000
          }
        ]
      }
    },
    "geography": {
      "locationOfOperationSupplyOrProduction": {
        "descriptionOfRestrictions": [
          {
            "value": "Le cisterne Tropea S Block, vengono prodotte nello stabilimento di Localit\u00e0 Merlaro, 2 - 25078 Vestone (BS)",
            "lang": "en"
          }
        ],
        "location": "GLO"
      }
    },
    "technology": {
      "technologyDescriptionAndIncludedProcesses": [
        {
          "value": "Qui di seguito viene descritto il processo di produzione delle cisterne Tropea S Block\u00ae oggetto della presente EPD: Le cisterne sono prodotte con un processo di stampaggio mediante presse a iniezione. Per quanto riguarda il processo di stampaggio, la pressa riceve, attraverso un sistema di distribuzione pneumatica, il materiale plastico in granuli direttamente dai sili di stoccaggio. il materiale una volta entrato nella camera di pressatura, grazie al riscaldamento all'interno della camera, raggiunge il punto di rammollimento e si lega, permettendo cos\u00ec di essere iniettato attraverso l'ugello nello stampo. Lo stampo viene mantenuto chiuso con una pressione controllata per il tempo necessario a raffreddare il pezzo. Alla fine del ciclo, lo stampo si apre, i perni utilizzati per modellare il pezzo e il componente viene spinto fuori dalla cavit\u00e0 dagli espulsori dello stampo e poi prelevato da un robot con una pinza. Il robot scarica quindi il pezzo sul nastro che lo porta alle stazioni di assemblaggio della pressa (dove previste) o ai contenitori previsti. Quindi tutti i componenti vengono portati in una linea di assemblaggio dove le diverse parti vengono installate all'interno del contenitore della cisterna.",
          "lang": "en"
        }
      ],
      "technologicalApplicability": [
        {
          "value": "The cisterns Tropea S Block represents the first cistern in the world designed to reduce the noise generated during use and is designed for installations in light or mixed walls (plasterboard, wall) with a wall-hung pan.",
          "lang": "en"
        }
      ],
      "referenceToTechnologyFlowDiagrammOrPicture": [
        {
          "shortDescription": [
            {
              "value": "EPDITALY0174 flowchart",
              "lang": "en"
            }
          ],
          "type": "source data set",
          "refObjectId": "43a54009-ab2c-492d-87a9-624486b1a6a0",
          "version": "00.00.002"
        }
      ]
    }
  },
  "modellingAndValidation": {
    "LCIMethodAndAllocation": {
      "typeOfDataSet": "EPD",
      "referenceToLCAMethodDetails": [
        {
          "shortDescription": [
            {
              "value": "PCR ICMQ-001/15 rev3",
              "lang": "en"
            }
          ],
          "type": "source data set",
          "refObjectId": "c36cdafa-45ef-40ed-bccf-ee5184b21c3e",
          "version": "00.00.003"
        }
      ],
      "other": {
        "anies": [
          {
            "name": "subType",
            "value": "average dataset"
          }
        ]
      }
    },
    "dataSourcesTreatmentAndRepresentativeness": {
      "referenceToDataSource": [
        {
          "shortDescription": [
            {
              "value": "GaBi database (general)",
              "lang": "en"
            }
          ],
          "type": "source data set",
          "refObjectId": "28d74cc0-db8b-4d7e-bc44-5f6d56ce0c4a",
          "version": "00.03.002"
        }
      ],
      "other": {
        "anies": [
          {
            "name": "referenceToOriginalEPD",
            "value": {
              "shortDescription": {
                "value": "EPDITALY0174 PDF",
                "defaultValue": "EPDITALY0174 PDF",
                "lstrings": [
                  {
                    "lang": "en",
                    "value": "EPDITALY0174 PDF"
                  }
                ]
              },
              "version": {
                "version": 1,
                "majorVersion": 0,
                "minorVersion": 0,
                "subMinorVersion": 1,
                "zero": false,
                "versionString": "00.00.001"
              },
              "type": "source data set",
              "uuid": {
                "uuid": "ef17c114-a72a-43b9-b1ca-86d83aa0a3ce"
              },
              "refObjectId": "ef17c114-a72a-43b9-b1ca-86d83aa0a3ce",
              "versionAsString": "00.00.001",
              "resourceURLs": [
                "https://node.epditaly.it/resource/sources/ef17c114-a72a-43b9-b1ca-86d83aa0a3ce/EPDITALY0174.pdf?version=00.00.001"
              ]
            }
          }
        ]
      }
    },
    "validation": {
      "review": [
        {
          "referenceToNameOfReviewerAndInstitution": [
            {
              "shortDescription": [
                {
                  "value": "ICMQ S.p.A.",
                  "lang": "en"
                }
              ],
              "type": "contact data set",
              "refObjectId": "6a2483f7-d823-4b36-ab56-f3b5bbaa976a",
              "version": "00.00.001"
            }
          ],
          "type": "Accredited third party review"
        }
      ]
    },
    "complianceDeclarations": {
      "compliance": [
        {
          "referenceToComplianceSystem": {
            "shortDescription": [
              {
                "value": "ISO 14025",
                "lang": "en"
              }
            ],
            "type": "source data set",
            "refObjectId": "4f2eb655-6e44-4874-a95a-e28f5442cd4d",
            "version": "00.00.001"
          }
        },
        {
          "referenceToComplianceSystem": {
            "shortDescription": [
              {
                "value": "EN 15804+A2",
                "lang": "de"
              },
              {
                "value": "EN 15804+A2",
                "lang": "en"
              }
            ],
            "type": "source data set",
            "refObjectId": "c0016b33-8cf7-415c-ac6e-deba0d21440d",
            "version": "00.01.000"
          }
        }
      ]
    }
  },
  "administrativeInformation": {
    "dataEntryBy": {
      "timeStamp": 1666002020901,
      "referenceToDataSetFormat": [
        {
          "shortDescription": [
            {
              "value": "EPD Data Format Extension",
              "lang": "de"
            },
            {
              "value": "EPD Data Format Extension",
              "lang": "en"
            }
          ],
          "type": "source data set",
          "refObjectId": "bb3d16d8-fdf6-4cd7-b5d8-f6427b99bb4b",
          "version": "00.01.000"
        },
        {
          "shortDescription": [
            {
              "value": "EPD Data Format Extensions v1.2",
              "lang": "en"
            },
            {
              "value": "EPD-Datenformaterweiterungen v1.2",
              "lang": "de"
            }
          ],
          "type": "source data set",
          "refObjectId": "a29449fd-aa2f-4de8-b5d7-4b06b43c6fde",
          "version": "00.01.000"
        },
        {
          "shortDescription": [
            {
              "value": "ILCD format",
              "lang": "en"
            }
          ],
          "type": "source data set",
          "refObjectId": "a97a0155-0234-4b87-b4ce-a45da52f2a40",
          "version": "01.00.000",
          "uri": "http://lca.jrc.ec.europa.eu/lcainfohub/sample_data/ilcd/sources/ILCD_Format_a97a0155-0234-4b87-b4ce-a45da52f2a40_01.00.000.xml"
        }
      ]
    },
    "publicationAndOwnership": {
      "dataSetVersion": "00.00.033",
      "referenceToRegistrationAuthority": {
        "shortDescription": [
          {
            "value": "ICMQ S.p.A.",
            "lang": "en"
          }
        ],
        "type": "contact data set",
        "refObjectId": "6a2483f7-d823-4b36-ab56-f3b5bbaa976a",
        "version": "00.00.001"
      },
      "registrationNumber": "EPDITALY0174",
      "referenceToOwnershipOfDataSet": {
        "shortDescription": [
          {
            "value": "Valsir S.p.A.",
            "lang": "en"
          }
        ],
        "type": "contact data set",
        "refObjectId": "faa9df3a-9483-4bd4-b010-5281f7e721f8",
        "version": "00.00.002"
      },
      "other": {
        "anies": [
          {
            "name": "referenceToPublisher",
            "value": {
              "shortDescription": [
                {
                  "value": "EPDItaly",
                  "lang": "en"
                }
              ],
              "type": "contact data set",
              "refObjectId": "9433b9cf-1d4a-420f-8c09-88d2472225b9",
              "version": "00.00.001"
            }
          }
        ]
      }
    }
  },
  "exchanges": {
    "exchange": [
      {
        "dataSetInternalID": 1,
        "referenceToFlowDataSet": {
          "shortDescription": [
            {
              "value": "Tropea S Block",
              "lang": "en"
            }
          ],
          "type": "flow data set",
          "refObjectId": "f6abc262-4f0b-42ef-8d3b-a15c33cced65",
          "version": "00.00.001"
        },
        "meanAmount": 1.0,
        "resultingAmount": 1.0,
        "referenceFlow": true,
        "resultingflowAmount": 0.087,
        "flowProperties": [
          {
            "name": [
              {
                "lang": "en",
                "value": "Mass"
              },
              {
                "lang": "de",
                "value": "Masse"
              }
            ],
            "uuid": "93a60a56-a3c8-11da-a746-0800200b9a66",
            "referenceFlowProperty": true,
            "meanValue": 0.087,
            "referenceUnit": "kg",
            "unitGroupUUID": "ad38d542-3fe9-439d-9b95-2f5f7752acaf"
          }
        ],
        "typeOfFlow": "Product flow"
      },
      {
        "dataSetInternalID": 2,
        "referenceToFlowDataSet": {
          "shortDescription": [
            {
              "value": "Components for re-use (CRU)",
              "lang": "en"
            },
            {
              "value": "Komponenten f\u00fcr die Wiederverwendung (CRU)",
              "lang": "de"
            },
            {
              "value": "Componentes para su reutilizaci\u00f3n (CRU)",
              "lang": "es"
            }
          ],
          "type": "flow data set",
          "refObjectId": "a2b32f97-3fc7-4af2-b209-525bc6426f33",
          "version": "30.00.000"
        },
        "exchange direction": "OUTPUT",
        "meanAmount": 0.0,
        "other": {
          "anies": [
            {
              "value": "0.0",
              "module": "A1"
            },
            {
              "value": "0.0",
              "module": "A2"
            },
            {
              "value": "0.0",
              "module": "A3"
            },
            {
              "module": "A1-A3"
            },
            {
              "value": "0.0",
              "module": "A4"
            },
            {
              "value": "0.0",
              "module": "A5"
            },
            {
              "module": "B1"
            },
            {
              "module": "B2"
            },
            {
              "module": "B3"
            },
            {
              "module": "B4"
            },
            {
              "module": "B5"
            },
            {
              "value": "0.0",
              "module": "B6"
            },
            {
              "module": "B7"
            },
            {
              "value": "0.0",
              "module": "C1"
            },
            {
              "value": "0.0",
              "module": "C2"
            },
            {
              "value": "0.0",
              "module": "C3"
            },
            {
              "value": "0.0",
              "module": "C4"
            },
            {
              "value": "0.0",
              "module": "D"
            },
            {
              "name": "referenceToUnitGroupDataSet",
              "value": {
                "shortDescription": [
                  {
                    "value": "kg"
                  }
                ],
                "type": "unit group data set",
                "refObjectId": "ad38d542-3fe9-439d-9b95-2f5f7752acaf",
                "uri": "../unitgroups/ad38d542-3fe9-439d-9b95-2f5f7752acaf"
              }
            }
          ]
        },
        "flowProperties": [],
        "typeOfFlow": "Other flow",
        "classification": {
          "classHierarchy": "Gr\u00f6\u00dfen / Umweltliche Gr\u00f6\u00dfen / EPD EN 15804 / LCI Indikatoren",
          "name": "GaBiCategories"
        }
      },
      {
        "dataSetInternalID": 3,
        "referenceToFlowDataSet": {
          "shortDescription": [
            {
              "value": "Exported electrical energy (EEE)",
              "lang": "en"
            },
            {
              "value": "Exportierte elektrische Energie (EEE)",
              "lang": "de"
            },
            {
              "value": "Energ\u00eda exportada electrica (EEE)",
              "lang": "es"
            }
          ],
          "type": "flow data set",
          "refObjectId": "4da0c987-2b76-40d6-9e9e-82a017aaaf29",
          "version": "30.00.000"
        },
        "exchange direction": "OUTPUT",
        "meanAmount": 0.0,
        "other": {
          "anies": [
            {
              "value": "0.0",
              "module": "A1"
            },
            {
              "value": "0.0",
              "module": "A2"
            },
            {
              "value": "0.0",
              "module": "A3"
            },
            {
              "module": "A1-A3"
            },
            {
              "value": "0.0",
              "module": "A4"
            },
            {
              "value": "0.455",
              "module": "A5"
            },
            {
              "module": "B1"
            },
            {
              "module": "B2"
            },
            {
              "module": "B3"
            },
            {
              "module": "B4"
            },
            {
              "module": "B5"
            },
            {
              "value": "0.0",
              "module": "B6"
            },
            {
              "module": "B7"
            },
            {
              "value": "0.0",
              "module": "C1"
            },
            {
              "value": "0.0",
              "module": "C2"
            },
            {
              "value": "7.11",
              "module": "C3"
            },
            {
              "value": "0.0",
              "module": "C4"
            },
            {
              "value": "0.0",
              "module": "D"
            },
            {
              "name": "referenceToUnitGroupDataSet",
              "value": {
                "shortDescription": [
                  {
                    "value": "MJ"
                  }
                ],
                "type": "unit group data set",
                "refObjectId": "93a60a57-a3c8-11da-a746-0800200c9a66",
                "uri": "../unitgroups/93a60a57-a3c8-11da-a746-0800200c9a66"
              }
            }
          ]
        },
        "flowProperties": [],
        "typeOfFlow": "Other flow",
        "classification": {
          "classHierarchy": "Gr\u00f6\u00dfen / Umweltliche Gr\u00f6\u00dfen / EPD EN 15804 / LCI Indikatoren",
          "name": "GaBiCategories"
        }
      },
      {
        "dataSetInternalID": 4,
        "referenceToFlowDataSet": {
          "shortDescription": [
            {
              "value": "Exported thermal energy (EET)",
              "lang": "en"
            },
            {
              "value": "Exportierte thermische Energie (EET)",
              "lang": "de"
            },
            {
              "value": "Energ\u00eda exportada termal (EET)",
              "lang": "es"
            }
          ],
          "type": "flow data set",
          "refObjectId": "98daf38a-7a79-46d3-9a37-2b7bd0955810",
          "version": "30.00.000"
        },
        "exchange direction": "OUTPUT",
        "meanAmount": 0.0,
        "other": {
          "anies": [
            {
              "value": "0.0",
              "module": "A1"
            },
            {
              "value": "0.0",
              "module": "A2"
            },
            {
              "value": "0.0",
              "module": "A3"
            },
            {
              "module": "A1-A3"
            },
            {
              "value": "0.0",
              "module": "A4"
            },
            {
              "value": "0.675",
              "module": "A5"
            },
            {
              "module": "B1"
            },
            {
              "module": "B2"
            },
            {
              "module": "B3"
            },
            {
              "module": "B4"
            },
            {
              "module": "B5"
            },
            {
              "value": "0.0",
              "module": "B6"
            },
            {
              "module": "B7"
            },
            {
              "value": "0.0",
              "module": "C1"
            },
            {
              "value": "0.0",
              "module": "C2"
            },
            {
              "value": "14.5",
              "module": "C3"
            },
            {
              "value": "0.0",
              "module": "C4"
            },
            {
              "value": "0.0",
              "module": "D"
            },
            {
              "name": "referenceToUnitGroupDataSet",
              "value": {
                "shortDescription": [
                  {
                    "value": "MJ"
                  }
                ],
                "type": "unit group data set",
                "refObjectId": "93a60a57-a3c8-11da-a746-0800200c9a66",
                "uri": "../unitgroups/93a60a57-a3c8-11da-a746-0800200c9a66"
              }
            }
          ]
        },
        "flowProperties": [],
        "typeOfFlow": "Other flow",
        "classification": {
          "classHierarchy": "Gr\u00f6\u00dfen / Umweltliche Gr\u00f6\u00dfen / EPD EN 15804 / LCI Indikatoren",
          "name": "GaBiCategories"
        }
      },
      {
        "dataSetInternalID": 5,
        "referenceToFlowDataSet": {
          "shortDescription": [
            {
              "value": "Hazardous waste disposed (HWD)",
              "lang": "en"
            },
            {
              "value": "Gef\u00e4hrlicher Abfall zur Deponie (HWD)",
              "lang": "de"
            },
            {
              "value": "Residuos peligrosos eliminados (HWD)",
              "lang": "es"
            }
          ],
          "type": "flow data set",
          "refObjectId": "430f9e0f-59b2-46a0-8e0d-55e0e84948fc",
          "version": "30.00.000"
        },
        "exchange direction": "OUTPUT",
        "meanAmount": 0.0,
        "other": {
          "anies": [
            {
              "value": "1.91E-5",
              "module": "A1"
            },
            {
              "value": "2.7E-11",
              "module": "A2"
            },
            {
              "value": "1.2E-7",
              "module": "A3"
            },
            {
              "module": "A1-A3"
            },
            {
              "value": "7.79E-11",
              "module": "A4"
            },
            {
              "value": "9.65E-8",
              "module": "A5"
            },
            {
              "module": "B1"
            },
            {
              "module": "B2"
            },
            {
              "module": "B3"
            },
            {
              "module": "B4"
            },
            {
              "module": "B5"
            },
            {
              "value": "6.27E-8",
              "module": "B6"
            },
            {
              "module": "B7"
            },
            {
              "value": "5.96E-10",
              "module": "C1"
            },
            {
              "value": "4.04E-11",
              "module": "C2"
            },
            {
              "value": "1.59E-9",
              "module": "C3"
            },
            {
              "value": "9.58E-10",
              "module": "C4"
            },
            {
              "value": "-2.34E-8",
              "module": "D"
            },
            {
              "name": "referenceToUnitGroupDataSet",
              "value": {
                "shortDescription": [
                  {
                    "value": "kg"
                  }
                ],
                "type": "unit group data set",
                "refObjectId": "ad38d542-3fe9-439d-9b95-2f5f7752acaf",
                "uri": "../unitgroups/ad38d542-3fe9-439d-9b95-2f5f7752acaf"
              }
            }
          ]
        },
        "flowProperties": [],
        "typeOfFlow": "Other flow",
        "classification": {
          "classHierarchy": "Gr\u00f6\u00dfen / Umweltliche Gr\u00f6\u00dfen / EPD EN 15804 / LCI Indikatoren",
          "name": "GaBiCategories"
        }
      },
      {
        "dataSetInternalID": 6,
        "referenceToFlowDataSet": {
          "shortDescription": [
            {
              "value": "Materials for energy recovery (MER)",
              "lang": "en"
            },
            {
              "value": "Stoffe f\u00fcr die Energier\u00fcckgewinnung (MER)",
              "lang": "de"
            },
            {
              "value": "Materiales para valorizaci\u00f3n energ\u00e9tica (recuperaci\u00f3n de energ\u00eda) (MER)",
              "lang": "es"
            }
          ],
          "type": "flow data set",
          "refObjectId": "59a9181c-3aaf-46ee-8b13-2b3723b6e447",
          "version": "30.00.000"
        },
        "exchange direction": "OUTPUT",
        "meanAmount": 0.0,
        "other": {
          "anies": [
            {
              "value": "0.0",
              "module": "A1"
            },
            {
              "value": "0.0",
              "module": "A2"
            },
            {
              "value": "0.0",
              "module": "A3"
            },
            {
              "module": "A1-A3"
            },
            {
              "value": "0.0",
              "module": "A4"
            },
            {
              "value": "0.0",
              "module": "A5"
            },
            {
              "module": "B1"
            },
            {
              "module": "B2"
            },
            {
              "module": "B3"
            },
            {
              "module": "B4"
            },
            {
              "module": "B5"
            },
            {
              "value": "0.0",
              "module": "B6"
            },
            {
              "module": "B7"
            },
            {
              "value": "0.0",
              "module": "C1"
            },
            {
              "value": "0.0",
              "module": "C2"
            },
            {
              "value": "0.0",
              "module": "C3"
            },
            {
              "value": "0.0",
              "module": "C4"
            },
            {
              "value": "0.0",
              "module": "D"
            },
            {
              "name": "referenceToUnitGroupDataSet",
              "value": {
                "shortDescription": [
                  {
                    "value": "kg"
                  }
                ],
                "type": "unit group data set",
                "refObjectId": "ad38d542-3fe9-439d-9b95-2f5f7752acaf",
                "uri": "../unitgroups/ad38d542-3fe9-439d-9b95-2f5f7752acaf"
              }
            }
          ]
        },
        "flowProperties": [],
        "typeOfFlow": "Other flow",
        "classification": {
          "classHierarchy": "Gr\u00f6\u00dfen / Umweltliche Gr\u00f6\u00dfen / EPD EN 15804 / LCI Indikatoren",
          "name": "GaBiCategories"
        }
      },
      {
        "dataSetInternalID": 7,
        "referenceToFlowDataSet": {
          "shortDescription": [
            {
              "value": "Materials for recycling (MFR)",
              "lang": "en"
            },
            {
              "value": "Stoffe zum Recycling (MFR)",
              "lang": "de"
            },
            {
              "value": "Materiales para el reciclaje (MFR)",
              "lang": "es"
            }
          ],
          "type": "flow data set",
          "refObjectId": "d7fe48a5-4103-49c8-9aae-b0b5dfdbd6ae",
          "version": "30.00.000"
        },
        "exchange direction": "OUTPUT",
        "meanAmount": 0.0,
        "other": {
          "anies": [
            {
              "value": "0.0",
              "module": "A1"
            },
            {
              "value": "0.0",
              "module": "A2"
            },
            {
              "value": "0.0",
              "module": "A3"
            },
            {
              "module": "A1-A3"
            },
            {
              "value": "0.0",
              "module": "A4"
            },
            {
              "value": "1.08",
              "module": "A5"
            },
            {
              "module": "B1"
            },
            {
              "module": "B2"
            },
            {
              "module": "B3"
            },
            {
              "module": "B4"
            },
            {
              "module": "B5"
            },
            {
              "value": "0.0",
              "module": "B6"
            },
            {
              "module": "B7"
            },
            {
              "value": "0.0",
              "module": "C1"
            },
            {
              "value": "0.0",
              "module": "C2"
            },
            {
              "value": "3.63",
              "module": "C3"
            },
            {
              "value": "0.0",
              "module": "C4"
            },
            {
              "value": "0.0",
              "module": "D"
            },
            {
              "name": "referenceToUnitGroupDataSet",
              "value": {
                "shortDescription": [
                  {
                    "value": "kg"
                  }
                ],
                "type": "unit group data set",
                "refObjectId": "ad38d542-3fe9-439d-9b95-2f5f7752acaf",
                "uri": "../unitgroups/ad38d542-3fe9-439d-9b95-2f5f7752acaf"
              }
            }
          ]
        },
        "flowProperties": [],
        "typeOfFlow": "Other flow",
        "classification": {
          "classHierarchy": "Gr\u00f6\u00dfen / Umweltliche Gr\u00f6\u00dfen / EPD EN 15804 / LCI Indikatoren",
          "name": "GaBiCategories"
        }
      },
      {
        "dataSetInternalID": 8,
        "referenceToFlowDataSet": {
          "shortDescription": [
            {
              "value": "Use of net fresh water (FW)",
              "lang": "en"
            },
            {
              "value": "Einsatz von S\u00fc\u00dfwasserressourcen (FW)",
              "lang": "de"
            },
            {
              "value": "Uso neto de recursos de agua dulce (FW)",
              "lang": "es"
            }
          ],
          "type": "flow data set",
          "refObjectId": "3cf952c8-f3a4-461d-8c96-96456ca62246",
          "version": "30.00.000"
        },
        "exchange direction": "INPUT",
        "meanAmount": 0.0,
        "other": {
          "anies": [
            {
              "value": "0.148",
              "module": "A1"
            },
            {
              "value": "2.16E-5",
              "module": "A2"
            },
            {
              "value": "0.0506",
              "module": "A3"
            },
            {
              "module": "A1-A3"
            },
            {
              "value": "6.17E-5",
              "module": "A4"
            },
            {
              "value": "0.00171",
              "module": "A5"
            },
            {
              "module": "B1"
            },
            {
              "module": "B2"
            },
            {
              "module": "B3"
            },
            {
              "module": "B4"
            },
            {
              "module": "B5"
            },
            {
              "value": "0.0559",
              "module": "B6"
            },
            {
              "module": "B7"
            },
            {
              "value": "0.00101",
              "module": "C1"
            },
            {
              "value": "3.22E-5",
              "module": "C2"
            },
            {
              "value": "0.0123",
              "module": "C3"
            },
            {
              "value": "1.11E-4",
              "module": "C4"
            },
            {
              "value": "-0.0188",
              "module": "D"
            },
            {
              "name": "referenceToUnitGroupDataSet",
              "value": {
                "shortDescription": [
                  {
                    "value": "m3"
                  }
                ],
                "type": "unit group data set",
                "refObjectId": "cd950537-0a98-4044-9ba7-9f9a68d0a504",
                "uri": "../unitgroups/cd950537-0a98-4044-9ba7-9f9a68d0a504"
              }
            }
          ]
        },
        "flowProperties": [],
        "typeOfFlow": "Other flow",
        "classification": {
          "classHierarchy": "Gr\u00f6\u00dfen / Umweltliche Gr\u00f6\u00dfen / EPD EN 15804 / LCI Indikatoren",
          "name": "GaBiCategories"
        }
      },
      {
        "dataSetInternalID": 9,
        "referenceToFlowDataSet": {
          "shortDescription": [
            {
              "value": "Non hazardous waste dispose (NHWD)",
              "lang": "en"
            },
            {
              "value": "Entsorgter nicht gef\u00e4hrlicher Abfall (NHWD)",
              "lang": "de"
            },
            {
              "value": "Residuos no peligrosos eliminados (NHWD)",
              "lang": "es"
            }
          ],
          "type": "flow data set",
          "refObjectId": "b29ef66b-e286-4afa-949f-62f1a7b4d7fa",
          "version": "30.00.000"
        },
        "exchange direction": "OUTPUT",
        "meanAmount": 0.0,
        "other": {
          "anies": [
            {
              "value": "0.972",
              "module": "A1"
            },
            {
              "value": "3.07E-4",
              "module": "A2"
            },
            {
              "value": "0.147",
              "module": "A3"
            },
            {
              "module": "A1-A3"
            },
            {
              "value": "8.97E-4",
              "module": "A4"
            },
            {
              "value": "0.349",
              "module": "A5"
            },
            {
              "module": "B1"
            },
            {
              "module": "B2"
            },
            {
              "module": "B3"
            },
            {
              "module": "B4"
            },
            {
              "module": "B5"
            },
            {
              "value": "0.0677",
              "module": "B6"
            },
            {
              "module": "B7"
            },
            {
              "value": "0.0016",
              "module": "C1"
            },
            {
              "value": "4.59E-4",
              "module": "C2"
            },
            {
              "value": "0.479",
              "module": "C3"
            },
            {
              "value": "6.21",
              "module": "C4"
            },
            {
              "value": "-0.0611",
              "module": "D"
            },
            {
              "name": "referenceToUnitGroupDataSet",
              "value": {
                "shortDescription": [
                  {
                    "value": "kg"
                  }
                ],
                "type": "unit group data set",
                "refObjectId": "ad38d542-3fe9-439d-9b95-2f5f7752acaf",
                "uri": "../unitgroups/ad38d542-3fe9-439d-9b95-2f5f7752acaf"
              }
            }
          ]
        },
        "flowProperties": [],
        "typeOfFlow": "Other flow",
        "classification": {
          "classHierarchy": "Gr\u00f6\u00dfen / Umweltliche Gr\u00f6\u00dfen / EPD EN 15804 / LCI Indikatoren",
          "name": "GaBiCategories"
        }
      },
      {
        "dataSetInternalID": 10,
        "referenceToFlowDataSet": {
          "shortDescription": [
            {
              "value": "Use of non renewable primary energy (PENRE)",
              "lang": "en"
            },
            {
              "value": "Nicht-erneuerbare Prim\u00e4renergie als Energietr\u00e4ger (PENRE)",
              "lang": "de"
            },
            {
              "value": "Uso de energ\u00eda primaria no renovable, excluyendo los recursos de energ\u00eda primaria no renovable utilizada como materia prima (PENRE)",
              "lang": "es"
            }
          ],
          "type": "flow data set",
          "refObjectId": "ac857178-2b45-46ec-892a-a9a4332f0372",
          "version": "30.00.000"
        },
        "exchange direction": "INPUT",
        "meanAmount": 0.0,
        "other": {
          "anies": [
            {
              "value": "296.0",
              "module": "A1"
            },
            {
              "value": "2.82",
              "module": "A2"
            },
            {
              "value": "4.54",
              "module": "A3"
            },
            {
              "module": "A1-A3"
            },
            {
              "value": "8.32",
              "module": "A4"
            },
            {
              "value": "3.49",
              "module": "A5"
            },
            {
              "module": "B1"
            },
            {
              "module": "B2"
            },
            {
              "module": "B3"
            },
            {
              "module": "B4"
            },
            {
              "module": "B5"
            },
            {
              "value": "276.0",
              "module": "B6"
            },
            {
              "module": "B7"
            },
            {
              "value": "2.26",
              "module": "C1"
            },
            {
              "value": "4.22",
              "module": "C2"
            },
            {
              "value": "67.3",
              "module": "C3"
            },
            {
              "value": "5.43",
              "module": "C4"
            },
            {
              "value": "-128.0",
              "module": "D"
            },
            {
              "name": "referenceToUnitGroupDataSet",
              "value": {
                "shortDescription": [
                  {
                    "value": "MJ"
                  }
                ],
                "type": "unit group data set",
                "refObjectId": "93a60a57-a3c8-11da-a746-0800200c9a66",
                "uri": "../unitgroups/93a60a57-a3c8-11da-a746-0800200c9a66"
              }
            }
          ]
        },
        "flowProperties": [],
        "typeOfFlow": "Other flow",
        "classification": {
          "classHierarchy": "Gr\u00f6\u00dfen / Umweltliche Gr\u00f6\u00dfen / EPD EN 15804 / LCI Indikatoren",
          "name": "GaBiCategories"
        }
      },
      {
        "dataSetInternalID": 11,
        "referenceToFlowDataSet": {
          "shortDescription": [
            {
              "value": "Use of non renewable primary energy resources used as raw materials (PENRM)",
              "lang": "en"
            },
            {
              "value": "Nicht-erneuerbare Prim\u00e4renergie zur stofflichen Nutzung (PENRM)",
              "lang": "de"
            },
            {
              "value": "Uso de la energ\u00eda primaria no renovable utilizada como materia prima (PENRM)",
              "lang": "es"
            }
          ],
          "type": "flow data set",
          "refObjectId": "1421caa0-679d-4bf4-b282-0eb850ccae27",
          "version": "30.00.000"
        },
        "exchange direction": "INPUT",
        "meanAmount": 0.0,
        "other": {
          "anies": [
            {
              "value": "340.0",
              "module": "A1"
            },
            {
              "value": "0.0",
              "module": "A2"
            },
            {
              "value": "7.58",
              "module": "A3"
            },
            {
              "module": "A1-A3"
            },
            {
              "value": "0.0",
              "module": "A4"
            },
            {
              "value": "0.571",
              "module": "A5"
            },
            {
              "module": "B1"
            },
            {
              "module": "B2"
            },
            {
              "module": "B3"
            },
            {
              "module": "B4"
            },
            {
              "module": "B5"
            },
            {
              "value": "0.0",
              "module": "B6"
            },
            {
              "module": "B7"
            },
            {
              "value": "0.0",
              "module": "C1"
            },
            {
              "value": "0.0",
              "module": "C2"
            },
            {
              "value": "-52.0",
              "module": "C3"
            },
            {
              "value": "0.0",
              "module": "C4"
            },
            {
              "value": "0.0",
              "module": "D"
            },
            {
              "name": "referenceToUnitGroupDataSet",
              "value": {
                "shortDescription": [
                  {
                    "value": "MJ"
                  }
                ],
                "type": "unit group data set",
                "refObjectId": "93a60a57-a3c8-11da-a746-0800200c9a66",
                "uri": "../unitgroups/93a60a57-a3c8-11da-a746-0800200c9a66"
              }
            }
          ]
        },
        "flowProperties": [],
        "typeOfFlow": "Other flow",
        "classification": {
          "classHierarchy": "Gr\u00f6\u00dfen / Umweltliche Gr\u00f6\u00dfen / EPD EN 15804 / LCI Indikatoren",
          "name": "GaBiCategories"
        }
      },
      {
        "dataSetInternalID": 12,
        "referenceToFlowDataSet": {
          "shortDescription": [
            {
              "value": "Use of non renewable secondary fuels (NRSF)",
              "lang": "en"
            },
            {
              "value": "Nicht erneuerbare Sekund\u00e4rbrennstoffe (NRSF)",
              "lang": "de"
            },
            {
              "value": "Uso de combustibles secundarios no renovables (NRSF)",
              "lang": "es"
            }
          ],
          "type": "flow data set",
          "refObjectId": "89def144-d39a-4287-b86f-efde453ddcb2",
          "version": "30.00.000"
        },
        "exchange direction": "INPUT",
        "meanAmount": 0.0,
        "other": {
          "anies": [
            {
              "value": "0.0",
              "module": "A1"
            },
            {
              "value": "0.0",
              "module": "A2"
            },
            {
              "value": "0.0",
              "module": "A3"
            },
            {
              "module": "A1-A3"
            },
            {
              "value": "0.0",
              "module": "A4"
            },
            {
              "value": "0.0",
              "module": "A5"
            },
            {
              "module": "B1"
            },
            {
              "module": "B2"
            },
            {
              "module": "B3"
            },
            {
              "module": "B4"
            },
            {
              "module": "B5"
            },
            {
              "value": "0.0",
              "module": "B6"
            },
            {
              "module": "B7"
            },
            {
              "value": "0.0",
              "module": "C1"
            },
            {
              "value": "0.0",
              "module": "C2"
            },
            {
              "value": "0.0",
              "module": "C3"
            },
            {
              "value": "0.0",
              "module": "C4"
            },
            {
              "value": "0.0",
              "module": "D"
            },
            {
              "name": "referenceToUnitGroupDataSet",
              "value": {
                "shortDescription": [
                  {
                    "value": "MJ"
                  }
                ],
                "type": "unit group data set",
                "refObjectId": "93a60a57-a3c8-11da-a746-0800200c9a66",
                "uri": "../unitgroups/93a60a57-a3c8-11da-a746-0800200c9a66"
              }
            }
          ]
        },
        "flowProperties": [],
        "typeOfFlow": "Other flow",
        "classification": {
          "classHierarchy": "Gr\u00f6\u00dfen / Umweltliche Gr\u00f6\u00dfen / EPD EN 15804 / LCI Indikatoren",
          "name": "GaBiCategories"
        }
      },
      {
        "dataSetInternalID": 13,
        "referenceToFlowDataSet": {
          "shortDescription": [
            {
              "value": "Radioactive waste disposed (RWD)",
              "lang": "en"
            },
            {
              "value": "Entsorgter radioaktiver Abfall (RWD)",
              "lang": "de"
            },
            {
              "value": "Residuos radiactivos eliminados (RWD)",
              "lang": "es"
            }
          ],
          "type": "flow data set",
          "refObjectId": "3449546e-52ad-4b39-b809-9fb77cea8ff6",
          "version": "30.00.000"
        },
        "exchange direction": "OUTPUT",
        "meanAmount": 0.0,
        "other": {
          "anies": [
            {
              "value": "0.014",
              "module": "A1"
            },
            {
              "value": "4.64E-6",
              "module": "A2"
            },
            {
              "value": "3.03E-4",
              "module": "A3"
            },
            {
              "module": "A1-A3"
            },
            {
              "value": "1.32E-5",
              "module": "A4"
            },
            {
              "value": "1.01E-4",
              "module": "A5"
            },
            {
              "module": "B1"
            },
            {
              "module": "B2"
            },
            {
              "module": "B3"
            },
            {
              "module": "B4"
            },
            {
              "module": "B5"
            },
            {
              "value": "0.0186",
              "module": "B6"
            },
            {
              "module": "B7"
            },
            {
              "value": "3.36E-4",
              "module": "C1"
            },
            {
              "value": "6.93E-6",
              "module": "C2"
            },
            {
              "value": "0.00101",
              "module": "C3"
            },
            {
              "value": "6.27E-5",
              "module": "C4"
            },
            {
              "value": "-0.00308",
              "module": "D"
            },
            {
              "name": "referenceToUnitGroupDataSet",
              "value": {
                "shortDescription": [
                  {
                    "value": "kg"
                  }
                ],
                "type": "unit group data set",
                "refObjectId": "ad38d542-3fe9-439d-9b95-2f5f7752acaf",
                "uri": "../unitgroups/ad38d542-3fe9-439d-9b95-2f5f7752acaf"
              }
            }
          ]
        },
        "flowProperties": [],
        "typeOfFlow": "Other flow",
        "classification": {
          "classHierarchy": "Gr\u00f6\u00dfen / Umweltliche Gr\u00f6\u00dfen / EPD EN 15804 / LCI Indikatoren",
          "name": "GaBiCategories"
        }
      },
      {
        "dataSetInternalID": 14,
        "referenceToFlowDataSet": {
          "shortDescription": [
            {
              "value": "Use of renewable primary energy (PERE)",
              "lang": "en"
            },
            {
              "value": "Erneuerbare Prim\u00e4renergie als Energietr\u00e4ger (PERE)",
              "lang": "de"
            },
            {
              "value": "Uso de energ\u00eda primaria renovable excluyendo los recursos de energ\u00eda primaria renovable utilizada como materia prima (PERE)",
              "lang": "es"
            }
          ],
          "type": "flow data set",
          "refObjectId": "20f32be5-0398-4288-9b6d-accddd195317",
          "version": "30.00.000"
        },
        "exchange direction": "INPUT",
        "meanAmount": 0.0,
        "other": {
          "anies": [
            {
              "value": "93.1",
              "module": "A1"
            },
            {
              "value": "0.015",
              "module": "A2"
            },
            {
              "value": "-20.3",
              "module": "A3"
            },
            {
              "module": "A1-A3"
            },
            {
              "value": "0.0425",
              "module": "A4"
            },
            {
              "value": "2.18",
              "module": "A5"
            },
            {
              "module": "B1"
            },
            {
              "module": "B2"
            },
            {
              "module": "B3"
            },
            {
              "module": "B4"
            },
            {
              "module": "B5"
            },
            {
              "value": "42.2",
              "module": "B6"
            },
            {
              "module": "B7"
            },
            {
              "value": "1.04",
              "module": "C1"
            },
            {
              "value": "0.0224",
              "module": "C2"
            },
            {
              "value": "2.14",
              "module": "C3"
            },
            {
              "value": "0.41",
              "module": "C4"
            },
            {
              "value": "-10.3",
              "module": "D"
            },
            {
              "name": "referenceToUnitGroupDataSet",
              "value": {
                "shortDescription": [
                  {
                    "value": "MJ"
                  }
                ],
                "type": "unit group data set",
                "refObjectId": "93a60a57-a3c8-11da-a746-0800200c9a66",
                "uri": "../unitgroups/93a60a57-a3c8-11da-a746-0800200c9a66"
              }
            }
          ]
        },
        "flowProperties": [],
        "typeOfFlow": "Other flow",
        "classification": {
          "classHierarchy": "Gr\u00f6\u00dfen / Umweltliche Gr\u00f6\u00dfen / EPD EN 15804 / LCI Indikatoren",
          "name": "GaBiCategories"
        }
      },
      {
        "dataSetInternalID": 15,
        "referenceToFlowDataSet": {
          "shortDescription": [
            {
              "value": "Use of renewable primary energy resources used as raw materials (PERM)",
              "lang": "en"
            },
            {
              "value": "Erneuerbare Prim\u00e4renergie zur stofflichen Nutzung (PERM)",
              "lang": "de"
            },
            {
              "value": "Uso de energ\u00eda primaria renovable utilizada como materia prima (PERM)",
              "lang": "es"
            }
          ],
          "type": "flow data set",
          "refObjectId": "fb3ec0de-548d-4508-aea5-00b73bf6f702",
          "version": "30.00.000"
        },
        "exchange direction": "INPUT",
        "meanAmount": 0.0,
        "other": {
          "anies": [
            {
              "value": "0.0",
              "module": "A1"
            },
            {
              "value": "0.0",
              "module": "A2"
            },
            {
              "value": "22.5",
              "module": "A3"
            },
            {
              "module": "A1-A3"
            },
            {
              "value": "0.0",
              "module": "A4"
            },
            {
              "value": "-1.63",
              "module": "A5"
            },
            {
              "module": "B1"
            },
            {
              "module": "B2"
            },
            {
              "module": "B3"
            },
            {
              "module": "B4"
            },
            {
              "module": "B5"
            },
            {
              "value": "0.0",
              "module": "B6"
            },
            {
              "module": "B7"
            },
            {
              "value": "0.0",
              "module": "C1"
            },
            {
              "value": "0.0",
              "module": "C2"
            },
            {
              "value": "0.0",
              "module": "C3"
            },
            {
              "value": "0.0",
              "module": "C4"
            },
            {
              "value": "0.0",
              "module": "D"
            },
            {
              "name": "referenceToUnitGroupDataSet",
              "value": {
                "shortDescription": [
                  {
                    "value": "MJ"
                  }
                ],
                "type": "unit group data set",
                "refObjectId": "93a60a57-a3c8-11da-a746-0800200c9a66",
                "uri": "../unitgroups/93a60a57-a3c8-11da-a746-0800200c9a66"
              }
            }
          ]
        },
        "flowProperties": [],
        "typeOfFlow": "Other flow",
        "classification": {
          "classHierarchy": "Gr\u00f6\u00dfen / Umweltliche Gr\u00f6\u00dfen / EPD EN 15804 / LCI Indikatoren",
          "name": "GaBiCategories"
        }
      },
      {
        "dataSetInternalID": 16,
        "referenceToFlowDataSet": {
          "shortDescription": [
            {
              "value": "Use of renewable secondary fuels (RSF)",
              "lang": "en"
            },
            {
              "value": "Erneuerbare Sekund\u00e4rbrennstoffe (RSF)",
              "lang": "de"
            },
            {
              "value": "Uso de combustibles secundarios renovables (RSF)",
              "lang": "es"
            }
          ],
          "type": "flow data set",
          "refObjectId": "64333088-a55f-4aa2-9a31-c10b07816787",
          "version": "30.00.000"
        },
        "exchange direction": "INPUT",
        "meanAmount": 0.0,
        "other": {
          "anies": [
            {
              "value": "0.0",
              "module": "A1"
            },
            {
              "value": "0.0",
              "module": "A2"
            },
            {
              "value": "0.0",
              "module": "A3"
            },
            {
              "module": "A1-A3"
            },
            {
              "value": "0.0",
              "module": "A4"
            },
            {
              "value": "0.0",
              "module": "A5"
            },
            {
              "module": "B1"
            },
            {
              "module": "B2"
            },
            {
              "module": "B3"
            },
            {
              "module": "B4"
            },
            {
              "module": "B5"
            },
            {
              "value": "0.0",
              "module": "B6"
            },
            {
              "module": "B7"
            },
            {
              "value": "0.0",
              "module": "C1"
            },
            {
              "value": "0.0",
              "module": "C2"
            },
            {
              "value": "0.0",
              "module": "C3"
            },
            {
              "value": "0.0",
              "module": "C4"
            },
            {
              "value": "0.0",
              "module": "D"
            },
            {
              "name": "referenceToUnitGroupDataSet",
              "value": {
                "shortDescription": [
                  {
                    "value": "MJ"
                  }
                ],
                "type": "unit group data set",
                "refObjectId": "93a60a57-a3c8-11da-a746-0800200c9a66",
                "uri": "../unitgroups/93a60a57-a3c8-11da-a746-0800200c9a66"
              }
            }
          ]
        },
        "flowProperties": [],
        "typeOfFlow": "Other flow",
        "classification": {
          "classHierarchy": "Gr\u00f6\u00dfen / Umweltliche Gr\u00f6\u00dfen / EPD EN 15804 / LCI Indikatoren",
          "name": "GaBiCategories"
        }
      },
      {
        "dataSetInternalID": 17,
        "referenceToFlowDataSet": {
          "shortDescription": [
            {
              "value": "Use of secondary material (SM)",
              "lang": "en"
            },
            {
              "value": "Einsatz von Sekund\u00e4rstoffen (SM)",
              "lang": "de"
            },
            {
              "value": "Uso de materiales secundarios (SM)",
              "lang": "es"
            }
          ],
          "type": "flow data set",
          "refObjectId": "c6a1f35f-2d09-4f54-8dfb-97e502e1ce92",
          "version": "30.00.000"
        },
        "exchange direction": "INPUT",
        "meanAmount": 0.0,
        "other": {
          "anies": [
            {
              "value": "4.52",
              "module": "A1"
            },
            {
              "value": "0.0",
              "module": "A2"
            },
            {
              "value": "1.57",
              "module": "A3"
            },
            {
              "module": "A1-A3"
            },
            {
              "value": "0.0",
              "module": "A4"
            },
            {
              "value": "0.0232",
              "module": "A5"
            },
            {
              "module": "B1"
            },
            {
              "module": "B2"
            },
            {
              "module": "B3"
            },
            {
              "module": "B4"
            },
            {
              "module": "B5"
            },
            {
              "value": "0.0",
              "module": "B6"
            },
            {
              "module": "B7"
            },
            {
              "value": "0.0",
              "module": "C1"
            },
            {
              "value": "0.0",
              "module": "C2"
            },
            {
              "value": "0.0",
              "module": "C3"
            },
            {
              "value": "0.0",
              "module": "C4"
            },
            {
              "value": "0.0",
              "module": "D"
            },
            {
              "name": "referenceToUnitGroupDataSet",
              "value": {
                "shortDescription": [
                  {
                    "value": "kg"
                  }
                ],
                "type": "unit group data set",
                "refObjectId": "ad38d542-3fe9-439d-9b95-2f5f7752acaf",
                "uri": "../unitgroups/ad38d542-3fe9-439d-9b95-2f5f7752acaf"
              }
            }
          ]
        },
        "flowProperties": [],
        "typeOfFlow": "Other flow",
        "classification": {
          "classHierarchy": "Gr\u00f6\u00dfen / Umweltliche Gr\u00f6\u00dfen / EPD EN 15804 / LCI Indikatoren",
          "name": "GaBiCategories"
        }
      },
      {
        "dataSetInternalID": 18,
        "referenceToFlowDataSet": {
          "shortDescription": [
            {
              "value": "Total use of non renewable primary energy resource (PENRT)",
              "lang": "en"
            },
            {
              "value": "Total nicht erneuerbare Prim\u00e4renergie (PENRT)",
              "lang": "de"
            },
            {
              "value": "Uso total de la energ\u00eda primaria no renovable (energ\u00eda primaria y recursos de energ\u00eda primaria renovable utilizada como materia prima) (PENRT)",
              "lang": "es"
            }
          ],
          "type": "flow data set",
          "refObjectId": "06159210-646b-4c8d-8583-da9b3b95a6c1",
          "version": "30.00.000"
        },
        "exchange direction": "INPUT",
        "meanAmount": 0.0,
        "other": {
          "anies": [
            {
              "value": "636.0",
              "module": "A1"
            },
            {
              "value": "2.82",
              "module": "A2"
            },
            {
              "value": "12.1",
              "module": "A3"
            },
            {
              "module": "A1-A3"
            },
            {
              "value": "8.32",
              "module": "A4"
            },
            {
              "value": "4.06",
              "module": "A5"
            },
            {
              "module": "B1"
            },
            {
              "module": "B2"
            },
            {
              "module": "B3"
            },
            {
              "module": "B4"
            },
            {
              "module": "B5"
            },
            {
              "value": "276.0",
              "module": "B6"
            },
            {
              "module": "B7"
            },
            {
              "value": "2.26",
              "module": "C1"
            },
            {
              "value": "4.22",
              "module": "C2"
            },
            {
              "value": "15.2",
              "module": "C3"
            },
            {
              "value": "5.43",
              "module": "C4"
            },
            {
              "value": "-128.0",
              "module": "D"
            },
            {
              "name": "referenceToUnitGroupDataSet",
              "value": {
                "shortDescription": [
                  {
                    "value": "MJ"
                  }
                ],
                "type": "unit group data set",
                "refObjectId": "93a60a57-a3c8-11da-a746-0800200c9a66",
                "uri": "../unitgroups/93a60a57-a3c8-11da-a746-0800200c9a66"
              }
            }
          ]
        },
        "flowProperties": [],
        "typeOfFlow": "Other flow",
        "classification": {
          "classHierarchy": "Gr\u00f6\u00dfen / Umweltliche Gr\u00f6\u00dfen / EPD EN 15804 / LCI Indikatoren",
          "name": "GaBiCategories"
        }
      },
      {
        "dataSetInternalID": 19,
        "referenceToFlowDataSet": {
          "shortDescription": [
            {
              "value": "Total use of renewable primary energy resources (PERT)",
              "lang": "en"
            },
            {
              "value": "Total erneuerbare Prim\u00e4renergie (PERT)",
              "lang": "de"
            },
            {
              "value": "Uso total de la energ\u00eda primaria renovable (energ\u00eda primaria y recursos de energ\u00eda primaria renovable utilizada como materia prima) (PERT)",
              "lang": "es"
            }
          ],
          "type": "flow data set",
          "refObjectId": "53f97275-fa8a-4cdd-9024-65936002acd0",
          "version": "30.00.000"
        },
        "exchange direction": "INPUT",
        "meanAmount": 0.0,
        "other": {
          "anies": [
            {
              "value": "93.1",
              "module": "A1"
            },
            {
              "value": "0.015",
              "module": "A2"
            },
            {
              "value": "2.21",
              "module": "A3"
            },
            {
              "module": "A1-A3"
            },
            {
              "value": "0.0425",
              "module": "A4"
            },
            {
              "value": "0.549",
              "module": "A5"
            },
            {
              "module": "B1"
            },
            {
              "module": "B2"
            },
            {
              "module": "B3"
            },
            {
              "module": "B4"
            },
            {
              "module": "B5"
            },
            {
              "value": "42.2",
              "module": "B6"
            },
            {
              "module": "B7"
            },
            {
              "value": "1.04",
              "module": "C1"
            },
            {
              "value": "0.0224",
              "module": "C2"
            },
            {
              "value": "2.14",
              "module": "C3"
            },
            {
              "value": "0.41",
              "module": "C4"
            },
            {
              "value": "-10.3",
              "module": "D"
            },
            {
              "name": "referenceToUnitGroupDataSet",
              "value": {
                "shortDescription": [
                  {
                    "value": "MJ"
                  }
                ],
                "type": "unit group data set",
                "refObjectId": "93a60a57-a3c8-11da-a746-0800200c9a66",
                "uri": "../unitgroups/93a60a57-a3c8-11da-a746-0800200c9a66"
              }
            }
          ]
        },
        "flowProperties": [],
        "typeOfFlow": "Other flow",
        "classification": {
          "classHierarchy": "Gr\u00f6\u00dfen / Umweltliche Gr\u00f6\u00dfen / EPD EN 15804 / LCI Indikatoren",
          "name": "GaBiCategories"
        }
      }
    ]
  },
  "LCIAResults": {
    "LCIAResult": [
      {
        "referenceToLCIAMethodDataSet": {
          "shortDescription": [
            {
              "value": "Abiotic depletion potential - non-fossil resources (ADPE)",
              "lang": "en"
            },
            {
              "value": "Potenzial f\u00fcr die Verknappung abiotischer Ressourcen \u2013 nicht fossile Ressourcen (ADPE)",
              "lang": "de"
            }
          ],
          "type": "LCIA method data set",
          "refObjectId": "b2ad6494-c78d-11e6-9d9d-cec0c932ce01",
          "version": "01.00.011"
        },
        "meanAmount": 0.0,
        "other": {
          "anies": [
            {
              "value": "4.85E-4",
              "module": "A1"
            },
            {
              "value": "9.67E-9",
              "module": "A2"
            },
            {
              "value": "1.13E-5",
              "module": "A3"
            },
            {
              "module": "A1-A3"
            },
            {
              "value": "2.76E-8",
              "module": "A4"
            },
            {
              "value": "3.12E-6",
              "module": "A5"
            },
            {
              "module": "B1"
            },
            {
              "module": "B2"
            },
            {
              "module": "B3"
            },
            {
              "module": "B4"
            },
            {
              "module": "B5"
            },
            {
              "value": "2.93E-6",
              "module": "B6"
            },
            {
              "module": "B7"
            },
            {
              "value": "3.73E-8",
              "module": "C1"
            },
            {
              "value": "1.44E-8",
              "module": "C2"
            },
            {
              "value": "-1.34E-5",
              "module": "C3"
            },
            {
              "value": "2.62E-8",
              "module": "C4"
            },
            {
              "value": "-1.12E-6",
              "module": "D"
            },
            {
              "name": "referenceToUnitGroupDataSet",
              "value": {
                "shortDescription": [
                  {
                    "value": "kg Sb-\u00c4qv."
                  }
                ],
                "type": "unit group data set",
                "refObjectId": "54ccd2d9-a32a-4fc2-923d-f2c8c93e89d4",
                "uri": "../unitgroups/54ccd2d9-a32a-4fc2-923d-f2c8c93e89d4"
              }
            }
          ]
        }
      },
      {
        "referenceToLCIAMethodDataSet": {
          "shortDescription": [
            {
              "value": "Abiotic depletion potential - fossil resources (ADPF)",
              "lang": "en"
            },
            {
              "value": "Potenzial f\u00fcr die Verknappung abiotischer Ressourcen \u2013 fossile Brennstoffe (ADPF)",
              "lang": "de"
            }
          ],
          "type": "LCIA method data set",
          "refObjectId": "b2ad6110-c78d-11e6-9d9d-cec0c932ce01",
          "version": "01.00.011"
        },
        "meanAmount": 0.0,
        "other": {
          "anies": [
            {
              "value": "636.0",
              "module": "A1"
            },
            {
              "value": "2.81",
              "module": "A2"
            },
            {
              "value": "12.1",
              "module": "A3"
            },
            {
              "module": "A1-A3"
            },
            {
              "value": "8.29",
              "module": "A4"
            },
            {
              "value": "4.06",
              "module": "A5"
            },
            {
              "module": "B1"
            },
            {
              "module": "B2"
            },
            {
              "module": "B3"
            },
            {
              "module": "B4"
            },
            {
              "module": "B5"
            },
            {
              "value": "276.0",
              "module": "B6"
            },
            {
              "module": "B7"
            },
            {
              "value": "2.26",
              "module": "C1"
            },
            {
              "value": "4.2",
              "module": "C2"
            },
            {
              "value": "15.2",
              "module": "C3"
            },
            {
              "value": "5.43",
              "module": "C4"
            },
            {
              "value": "-128.0",
              "module": "D"
            },
            {
              "name": "referenceToUnitGroupDataSet",
              "value": {
                "shortDescription": [
                  {
                    "value": "MJ"
                  }
                ],
                "type": "unit group data set",
                "refObjectId": "93a60a57-a3c8-11da-a746-0800200c9a66",
                "uri": "../unitgroups/93a60a57-a3c8-11da-a746-0800200c9a66"
              }
            }
          ]
        }
      },
      {
        "referenceToLCIAMethodDataSet": {
          "shortDescription": [
            {
              "value": "Acidification potential, Accumulated Exceedance (AP)",
              "lang": "en"
            },
            {
              "value": "Versauerungspotenzial, kumulierte \u00dcberschreitung (AP)",
              "lang": "de"
            }
          ],
          "type": "LCIA method data set",
          "refObjectId": "b5c611c6-def3-11e6-bf01-fe55135034f3",
          "version": "01.03.010",
          "uri": "http://lca.jrc.ec.europa.eu/lcainfohub/datasets/elcd/lciamethods/f6cbd466-253f-4145-a4bb-8dae7d266e89.xml"
        },
        "meanAmount": 0.0,
        "other": {
          "anies": [
            {
              "value": "0.0795",
              "module": "A1"
            },
            {
              "value": "2.03E-4",
              "module": "A2"
            },
            {
              "value": "0.0055",
              "module": "A3"
            },
            {
              "module": "A1-A3"
            },
            {
              "value": "0.00327",
              "module": "A4"
            },
            {
              "value": "6.47E-4",
              "module": "A5"
            },
            {
              "module": "B1"
            },
            {
              "module": "B2"
            },
            {
              "module": "B3"
            },
            {
              "module": "B4"
            },
            {
              "module": "B5"
            },
            {
              "value": "0.0186",
              "module": "B6"
            },
            {
              "module": "B7"
            },
            {
              "value": "2.64E-4",
              "module": "C1"
            },
            {
              "value": "2.71E-4",
              "module": "C2"
            },
            {
              "value": "0.00151",
              "module": "C3"
            },
            {
              "value": "0.0012",
              "module": "C4"
            },
            {
              "value": "-0.0097",
              "module": "D"
            },
            {
              "name": "referenceToUnitGroupDataSet",
              "value": {
                "shortDescription": [
                  {
                    "value": "mol H+ eqv."
                  }
                ],
                "type": "unit group data set",
                "refObjectId": "42e089ac-92bf-4bf2-8ca1-5fc40d18f2ed",
                "uri": "../unitgroups/42e089ac-92bf-4bf2-8ca1-5fc40d18f2ed"
              }
            }
          ]
        }
      },
      {
        "referenceToLCIAMethodDataSet": {
          "shortDescription": [
            {
              "value": "Eutrophication potential - freshwater (EP-freshwater)",
              "lang": "en"
            },
            {
              "value": "Eutrophierungspotenzial - S\u00fc\u00dfwasser (EP-freshwater)",
              "lang": "de"
            }
          ],
          "type": "LCIA method data set",
          "refObjectId": "b53ec18f-7377-4ad3-86eb-cc3f4f276b2b",
          "version": "01.00.011",
          "uri": "http://lca.jrc.ec.europa.eu/lcainfohub/datasets/elcd/lciamethods/a4630d5b-df2f-48ae-b3f2-5e5257606d68.xml"
        },
        "meanAmount": 0.0,
        "other": {
          "anies": [
            {
              "value": "5.76E-5",
              "module": "A1"
            },
            {
              "value": "4.67E-8",
              "module": "A2"
            },
            {
              "value": "9.41E-5",
              "module": "A3"
            },
            {
              "module": "A1-A3"
            },
            {
              "value": "1.39E-7",
              "module": "A4"
            },
            {
              "value": "8.51E-6",
              "module": "A5"
            },
            {
              "module": "B1"
            },
            {
              "module": "B2"
            },
            {
              "module": "B3"
            },
            {
              "module": "B4"
            },
            {
              "module": "B5"
            },
            {
              "value": "7.11E-6",
              "module": "B6"
            },
            {
              "module": "B7"
            },
            {
              "value": "3.4E-7",
              "module": "C1"
            },
            {
              "value": "6.98E-8",
              "module": "C2"
            },
            {
              "value": "1.58E-5",
              "module": "C3"
            },
            {
              "value": "6.56E-5",
              "module": "C4"
            },
            {
              "value": "-6.59E-6",
              "module": "D"
            },
            {
              "name": "referenceToUnitGroupDataSet",
              "value": {
                "shortDescription": [
                  {
                    "value": "kg P eqv."
                  }
                ],
                "type": "unit group data set",
                "refObjectId": "0429039d-a61d-4590-ba67-aa4a20a810a1",
                "uri": "../unitgroups/0429039d-a61d-4590-ba67-aa4a20a810a1"
              }
            }
          ]
        }
      },
      {
        "referenceToLCIAMethodDataSet": {
          "shortDescription": [
            {
              "value": "Eutrophication potential - marine (EP-marine)",
              "lang": "en"
            },
            {
              "value": "Eutrophierungspotenzial - Salzwasser (EP-marine)",
              "lang": "de"
            }
          ],
          "type": "LCIA method data set",
          "refObjectId": "b5c619fa-def3-11e6-bf01-fe55135034f3",
          "version": "02.00.011",
          "uri": "http://lca.jrc.ec.europa.eu/lcainfohub/datasets/elcd/lciamethods/5296e2be-060b-4e50-b033-d45f85f6ac92.xml"
        },
        "meanAmount": 0.0,
        "other": {
          "anies": [
            {
              "value": "0.0169",
              "module": "A1"
            },
            {
              "value": "6.93E-5",
              "module": "A2"
            },
            {
              "value": "0.00175",
              "module": "A3"
            },
            {
              "module": "A1-A3"
            },
            {
              "value": "8.65E-4",
              "module": "A4"
            },
            {
              "value": "1.94E-4",
              "module": "A5"
            },
            {
              "module": "B1"
            },
            {
              "module": "B2"
            },
            {
              "module": "B3"
            },
            {
              "module": "B4"
            },
            {
              "module": "B5"
            },
            {
              "value": "0.00568",
              "module": "B6"
            },
            {
              "module": "B7"
            },
            {
              "value": "6.27E-5",
              "module": "C1"
            },
            {
              "value": "8.45E-5",
              "module": "C2"
            },
            {
              "value": "5.43E-4",
              "module": "C3"
            },
            {
              "value": "2.77E-4",
              "module": "C4"
            },
            {
              "value": "-0.00254",
              "module": "D"
            },
            {
              "name": "referenceToUnitGroupDataSet",
              "value": {
                "shortDescription": [
                  {
                    "value": "kg N eqv."
                  }
                ],
                "type": "unit group data set",
                "refObjectId": "d05bb823-ecdf-4686-8c40-bf1d9257859f",
                "uri": "../unitgroups/d05bb823-ecdf-4686-8c40-bf1d9257859f"
              }
            }
          ]
        }
      },
      {
        "referenceToLCIAMethodDataSet": {
          "shortDescription": [
            {
              "value": "Eutrophication potential - terrestrial (EP-terrestrial)",
              "lang": "en"
            },
            {
              "value": "Eutrophierungspotenzial - Land (EP-terrestrial)",
              "lang": "de"
            }
          ],
          "type": "LCIA method data set",
          "refObjectId": "b5c614d2-def3-11e6-bf01-fe55135034f3",
          "version": "01.02.010",
          "uri": "http://lca.jrc.ec.europa.eu/lcainfohub/datasets/elcd/lciamethods/40054970-5936-477c-9bec-29fa23b1cb77.xml"
        },
        "meanAmount": 0.0,
        "other": {
          "anies": [
            {
              "value": "0.181",
              "module": "A1"
            },
            {
              "value": "7.69E-4",
              "module": "A2"
            },
            {
              "value": "0.0212",
              "module": "A3"
            },
            {
              "module": "A1-A3"
            },
            {
              "value": "0.00949",
              "module": "A4"
            },
            {
              "value": "0.00177",
              "module": "A5"
            },
            {
              "module": "B1"
            },
            {
              "module": "B2"
            },
            {
              "module": "B3"
            },
            {
              "module": "B4"
            },
            {
              "module": "B5"
            },
            {
              "value": "0.0615",
              "module": "B6"
            },
            {
              "module": "B7"
            },
            {
              "value": "6.58E-4",
              "module": "C1"
            },
            {
              "value": "9.54E-4",
              "module": "C2"
            },
            {
              "value": "0.00683",
              "module": "C3"
            },
            {
              "value": "0.00304",
              "module": "C4"
            },
            {
              "value": "-0.0272",
              "module": "D"
            },
            {
              "name": "referenceToUnitGroupDataSet",
              "value": {
                "shortDescription": [
                  {
                    "value": "mol N eqv."
                  }
                ],
                "type": "unit group data set",
                "refObjectId": "71b4d617-0ec9-4d3f-b65e-e438940c2401",
                "uri": "../unitgroups/71b4d617-0ec9-4d3f-b65e-e438940c2401"
              }
            }
          ]
        }
      },
      {
        "referenceToLCIAMethodDataSet": {
          "shortDescription": [
            {
              "value": "Global Warming Potential - total (GWP-total)",
              "lang": "en"
            },
            {
              "value": "Globales Erw\u00e4rmungspotenzial - total (GWP-total)",
              "lang": "de"
            }
          ],
          "type": "LCIA method data set",
          "refObjectId": "6a37f984-a4b3-458a-a20a-64418c145fa2",
          "version": "04.00.017"
        },
        "meanAmount": 0.0,
        "other": {
          "anies": [
            {
              "value": "32.3",
              "module": "A1"
            },
            {
              "value": "0.208",
              "module": "A2"
            },
            {
              "value": "-1.06",
              "module": "A3"
            },
            {
              "module": "A1-A3"
            },
            {
              "value": "0.62",
              "module": "A4"
            },
            {
              "value": "2.9",
              "module": "A5"
            },
            {
              "module": "B1"
            },
            {
              "module": "B2"
            },
            {
              "module": "B3"
            },
            {
              "module": "B4"
            },
            {
              "module": "B5"
            },
            {
              "value": "17.2",
              "module": "B6"
            },
            {
              "module": "B7"
            },
            {
              "value": "0.128",
              "module": "C1"
            },
            {
              "value": "0.311",
              "module": "C2"
            },
            {
              "value": "4.46",
              "module": "C3"
            },
            {
              "value": "0.371",
              "module": "C4"
            },
            {
              "value": "-5.71",
              "module": "D"
            },
            {
              "name": "referenceToUnitGroupDataSet",
              "value": {
                "shortDescription": [
                  {
                    "value": "kg CO2-\u00c4qv."
                  }
                ],
                "type": "unit group data set",
                "refObjectId": "1ebf3012-d0db-4de2-aefd-ef30cedb0be1",
                "uri": "../unitgroups/1ebf3012-d0db-4de2-aefd-ef30cedb0be1"
              }
            }
          ]
        }
      },
      {
        "referenceToLCIAMethodDataSet": {
          "shortDescription": [
            {
              "value": "Global Warming Potential - fossil fuels (GWP-fossil)",
              "lang": "en"
            },
            {
              "value": "Globales Erw\u00e4rmungspotenzial - fossil (GWP-fossil)",
              "lang": "de"
            }
          ],
          "type": "LCIA method data set",
          "refObjectId": "5f635281-343e-44fb-83df-1971b155e6b6",
          "version": "01.00.009"
        },
        "meanAmount": 0.0,
        "other": {
          "anies": [
            {
              "value": "32.1",
              "module": "A1"
            },
            {
              "value": "0.208",
              "module": "A2"
            },
            {
              "value": "1.31",
              "module": "A3"
            },
            {
              "module": "A1-A3"
            },
            {
              "value": "0.619",
              "module": "A4"
            },
            {
              "value": "0.32",
              "module": "A5"
            },
            {
              "module": "B1"
            },
            {
              "module": "B2"
            },
            {
              "module": "B3"
            },
            {
              "module": "B4"
            },
            {
              "module": "B5"
            },
            {
              "value": "17.2",
              "module": "B6"
            },
            {
              "module": "B7"
            },
            {
              "value": "0.127",
              "module": "C1"
            },
            {
              "value": "0.311",
              "module": "C2"
            },
            {
              "value": "4.46",
              "module": "C3"
            },
            {
              "value": "0.374",
              "module": "C4"
            },
            {
              "value": "-5.68",
              "module": "D"
            },
            {
              "name": "referenceToUnitGroupDataSet",
              "value": {
                "shortDescription": [
                  {
                    "value": "kg CO2-\u00c4qv."
                  }
                ],
                "type": "unit group data set",
                "refObjectId": "1ebf3012-d0db-4de2-aefd-ef30cedb0be1",
                "uri": "../unitgroups/1ebf3012-d0db-4de2-aefd-ef30cedb0be1"
              }
            }
          ]
        }
      },
      {
        "referenceToLCIAMethodDataSet": {
          "shortDescription": [
            {
              "value": "Global Warming Potential - biogenic (GWP-biogenic)",
              "lang": "en"
            },
            {
              "value": "Globales Erw\u00e4rmungspotenzial - biogen (GWP-biogenic)",
              "lang": "de"
            }
          ],
          "type": "LCIA method data set",
          "refObjectId": "2356e1ab-0185-4db5-86e5-16de51c7485c",
          "version": "01.00.006"
        },
        "meanAmount": 0.0,
        "other": {
          "anies": [
            {
              "value": "0.148",
              "module": "A1"
            },
            {
              "value": "3.13E-4",
              "module": "A2"
            },
            {
              "value": "-2.37",
              "module": "A3"
            },
            {
              "module": "A1-A3"
            },
            {
              "value": "9.19E-4",
              "module": "A4"
            },
            {
              "value": "2.58",
              "module": "A5"
            },
            {
              "module": "B1"
            },
            {
              "module": "B2"
            },
            {
              "module": "B3"
            },
            {
              "module": "B4"
            },
            {
              "module": "B5"
            },
            {
              "value": "0.0196",
              "module": "B6"
            },
            {
              "module": "B7"
            },
            {
              "value": "0.00108",
              "module": "C1"
            },
            {
              "value": "4.68E-4",
              "module": "C2"
            },
            {
              "value": "0.00398",
              "module": "C3"
            },
            {
              "value": "-0.00372",
              "module": "C4"
            },
            {
              "value": "-0.0256",
              "module": "D"
            },
            {
              "name": "referenceToUnitGroupDataSet",
              "value": {
                "shortDescription": [
                  {
                    "value": "kg CO2-\u00c4qv."
                  }
                ],
                "type": "unit group data set",
                "refObjectId": "1ebf3012-d0db-4de2-aefd-ef30cedb0be1",
                "uri": "../unitgroups/1ebf3012-d0db-4de2-aefd-ef30cedb0be1"
              }
            }
          ]
        }
      },
      {
        "referenceToLCIAMethodDataSet": {
          "shortDescription": [
            {
              "value": "Global Warming Potential - land use and land use change (GWP-luluc)",
              "lang": "en"
            },
            {
              "value": "Globales Erw\u00e4rmungspotenzial - luluc (GWP-luluc)",
              "lang": "de"
            }
          ],
          "type": "LCIA method data set",
          "refObjectId": "4331bbdb-978a-490d-8707-eeb047f01a55",
          "version": "01.00.006"
        },
        "meanAmount": 0.0,
        "other": {
          "anies": [
            {
              "value": "0.0345",
              "module": "A1"
            },
            {
              "value": "1.36E-5",
              "module": "A2"
            },
            {
              "value": "0.0019",
              "module": "A3"
            },
            {
              "module": "A1-A3"
            },
            {
              "value": "3.72E-5",
              "module": "A4"
            },
            {
              "value": "2.11E-4",
              "module": "A5"
            },
            {
              "module": "B1"
            },
            {
              "module": "B2"
            },
            {
              "module": "B3"
            },
            {
              "module": "B4"
            },
            {
              "module": "B5"
            },
            {
              "value": "0.00327",
              "module": "B6"
            },
            {
              "module": "B7"
            },
            {
              "value": "1.8E-4",
              "module": "C1"
            },
            {
              "value": "2.03E-5",
              "module": "C2"
            },
            {
              "value": "2.56E-4",
              "module": "C3"
            },
            {
              "value": "3.53E-4",
              "module": "C4"
            },
            {
              "value": "-0.0025",
              "module": "D"
            },
            {
              "name": "referenceToUnitGroupDataSet",
              "value": {
                "shortDescription": [
                  {
                    "value": "kg CO2-\u00c4qv."
                  }
                ],
                "type": "unit group data set",
                "refObjectId": "1ebf3012-d0db-4de2-aefd-ef30cedb0be1",
                "uri": "../unitgroups/1ebf3012-d0db-4de2-aefd-ef30cedb0be1"
              }
            }
          ]
        }
      },
      {
        "referenceToLCIAMethodDataSet": {
          "shortDescription": [
            {
              "value": "Depletion potential of the stratospheric ozone layer (ODP)",
              "lang": "en"
            },
            {
              "value": "Abbaupotenzial der stratosph\u00e4rischen Ozonschicht (ODP)",
              "lang": "de"
            }
          ],
          "type": "LCIA method data set",
          "refObjectId": "b5c629d6-def3-11e6-bf01-fe55135034f3",
          "version": "02.00.013",
          "uri": "http://lca.jrc.ec.europa.eu/lcainfohub/datasets/elcd/lciamethods/8b723200-3d8f-4eec-9e10-444edb029476.xml"
        },
        "meanAmount": 0.0,
        "other": {
          "anies": [
            {
              "value": "3.78E-9",
              "module": "A1"
            },
            {
              "value": "3.66E-17",
              "module": "A2"
            },
            {
              "value": "1.76E-13",
              "module": "A3"
            },
            {
              "module": "A1-A3"
            },
            {
              "value": "1.04E-16",
              "module": "A4"
            },
            {
              "value": "1.89E-11",
              "module": "A5"
            },
            {
              "module": "B1"
            },
            {
              "module": "B2"
            },
            {
              "module": "B3"
            },
            {
              "module": "B4"
            },
            {
              "module": "B5"
            },
            {
              "value": "2.68E-13",
              "module": "B6"
            },
            {
              "module": "B7"
            },
            {
              "value": "3.04E-15",
              "module": "C1"
            },
            {
              "value": "5.47E-17",
              "module": "C2"
            },
            {
              "value": "4.63E-15",
              "module": "C3"
            },
            {
              "value": "9.31E-16",
              "module": "C4"
            },
            {
              "value": "-3.14E-10",
              "module": "D"
            },
            {
              "name": "referenceToUnitGroupDataSet",
              "value": {
                "shortDescription": [
                  {
                    "value": "kg CFC 11-\u00c4quiv."
                  }
                ],
                "type": "unit group data set",
                "refObjectId": "d9e957c9-7309-4474-bf3a-7777df6c4e5b",
                "uri": "../unitgroups/d9e957c9-7309-4474-bf3a-7777df6c4e5b"
              }
            }
          ]
        }
      },
      {
        "referenceToLCIAMethodDataSet": {
          "shortDescription": [
            {
              "value": "Versauerungspotenzial, kumulierte \u00dcberschreitung (AP)",
              "lang": "en"
            },
            {
              "value": "Bildungspotenzial f\u00fcr troposph\u00e4risches Ozon (POCP)",
              "lang": "de"
            }
          ],
          "type": "LCIA method data set",
          "refObjectId": "b5c610fe-def3-11e6-bf01-fe55135034f3",
          "version": "02.00.014",
          "uri": "http://lca.jrc.ec.europa.eu/lcainfohub/datasets/elcd/lciamethods/ec7836be-83eb-41da-bcda-1a6a3fe2d149.xml"
        },
        "meanAmount": 0.0,
        "other": {
          "anies": [
            {
              "value": "0.0558",
              "module": "A1"
            },
            {
              "value": "1.94E-4",
              "module": "A2"
            },
            {
              "value": "0.00583",
              "module": "A3"
            },
            {
              "module": "A1-A3"
            },
            {
              "value": "0.00245",
              "module": "A4"
            },
            {
              "value": "5.88E-4",
              "module": "A5"
            },
            {
              "module": "B1"
            },
            {
              "module": "B2"
            },
            {
              "module": "B3"
            },
            {
              "module": "B4"
            },
            {
              "module": "B5"
            },
            {
              "value": "0.0168",
              "module": "B6"
            },
            {
              "module": "B7"
            },
            {
              "value": "1.7E-4",
              "module": "C1"
            },
            {
              "value": "2.52E-4",
              "module": "C2"
            },
            {
              "value": "0.00143",
              "module": "C3"
            },
            {
              "value": "8.8E-4",
              "module": "C4"
            },
            {
              "value": "-0.00896",
              "module": "D"
            },
            {
              "name": "referenceToUnitGroupDataSet",
              "value": {
                "shortDescription": [
                  {
                    "value": "kg NMVOC eqv."
                  }
                ],
                "type": "unit group data set",
                "refObjectId": "d27c25f8-fbc1-44c6-b47b-4adbae4199c6",
                "uri": "../unitgroups/d27c25f8-fbc1-44c6-b47b-4adbae4199c6"
              }
            }
          ]
        }
      },
      {
        "referenceToLCIAMethodDataSet": {
          "shortDescription": [
            {
              "value": "Water (user) deprivation potential (WDP)",
              "lang": "en"
            },
            {
              "value": "Wasser-Entzugspotenzial (Benutzer) (WDP)",
              "lang": "de"
            }
          ],
          "type": "LCIA method data set",
          "refObjectId": "b2ad66ce-c78d-11e6-9d9d-cec0c932ce01",
          "version": "03.00.015"
        },
        "meanAmount": 0.0,
        "other": {
          "anies": [
            {
              "value": "3.56",
              "module": "A1"
            },
            {
              "value": "4.6E-4",
              "module": "A2"
            },
            {
              "value": "2.11",
              "module": "A3"
            },
            {
              "module": "A1-A3"
            },
            {
              "value": "0.00132",
              "module": "A4"
            },
            {
              "value": "0.0575",
              "module": "A5"
            },
            {
              "module": "B1"
            },
            {
              "module": "B2"
            },
            {
              "module": "B3"
            },
            {
              "module": "B4"
            },
            {
              "module": "B5"
            },
            {
              "value": "1.83",
              "module": "B6"
            },
            {
              "module": "B7"
            },
            {
              "value": "0.0203",
              "module": "C1"
            },
            {
              "value": "6.87E-4",
              "module": "C2"
            },
            {
              "value": "0.493",
              "module": "C3"
            },
            {
              "value": "-0.0023",
              "module": "C4"
            },
            {
              "value": "-0.437",
              "module": "D"
            },
            {
              "name": "referenceToUnitGroupDataSet",
              "value": {
                "shortDescription": [
                  {
                    "value": "m3 world eqv."
                  }
                ],
                "type": "unit group data set",
                "refObjectId": "6ae2df01-888e-46c8-b17d-49fa3869b476",
                "uri": "../unitgroups/6ae2df01-888e-46c8-b17d-49fa3869b476"
              }
            }
          ]
        }
      },
      {
        "referenceToLCIAMethodDataSet": {
          "shortDescription": [
            {
              "value": "Potential incidence of disease due to PM emissions (PM)",
              "lang": "en"
            },
            {
              "value": "Potenzielles Auftreten von Krankheiten aufgrund von Feinstaubemissionen (PM)",
              "lang": "de"
            }
          ],
          "type": "LCIA method data set",
          "refObjectId": "b5c602c6-def3-11e6-bf01-fe55135034f3",
          "version": "02.00.012",
          "uri": "http://lca.jrc.ec.europa.eu/lcainfohub/datasets/elcd/lciamethods/72ce3013-f678-4c6a-935b-f4752ff8901b.xml"
        },
        "meanAmount": 0.0,
        "other": {
          "anies": [
            {
              "module": "A1"
            },
            {
              "module": "A2"
            },
            {
              "module": "A3"
            },
            {
              "module": "A1-A3"
            },
            {
              "module": "A4"
            },
            {
              "module": "A5"
            },
            {
              "module": "B1"
            },
            {
              "module": "B2"
            },
            {
              "module": "B3"
            },
            {
              "module": "B4"
            },
            {
              "module": "B5"
            },
            {
              "module": "B6"
            },
            {
              "module": "B7"
            },
            {
              "module": "C1"
            },
            {
              "module": "C2"
            },
            {
              "module": "C3"
            },
            {
              "module": "C4"
            },
            {
              "module": "D"
            },
            {
              "name": "referenceToUnitGroupDataSet",
              "value": {
                "shortDescription": [
                  {
                    "value": "disease incidence"
                  }
                ],
                "type": "unit group data set",
                "refObjectId": "3883559b-648f-4afc-8ba2-0bd24f3affa3",
                "uri": "../unitgroups/3883559b-648f-4afc-8ba2-0bd24f3affa3"
              }
            }
          ]
        }
      },
      {
        "referenceToLCIAMethodDataSet": {
          "shortDescription": [
            {
              "value": "Potential Human exposure efficiency relative to U235 (IRP)",
              "lang": "en"
            },
            {
              "value": "Potenzielle Wirkung durch Exposition des Menschen mit U235 (IRP)",
              "lang": "de"
            }
          ],
          "type": "LCIA method data set",
          "refObjectId": "b5c632be-def3-11e6-bf01-fe55135034f3",
          "version": "01.00.012",
          "uri": "http://lca.jrc.ec.europa.eu/lcainfohub/datasets/elcd/lciamethods/a6f4cbc8-5388-44d6-9a67-53d05684f93e.xml"
        },
        "meanAmount": 0.0,
        "other": {
          "anies": [
            {
              "module": "A1"
            },
            {
              "module": "A2"
            },
            {
              "module": "A3"
            },
            {
              "module": "A1-A3"
            },
            {
              "module": "A4"
            },
            {
              "module": "A5"
            },
            {
              "module": "B1"
            },
            {
              "module": "B2"
            },
            {
              "module": "B3"
            },
            {
              "module": "B4"
            },
            {
              "module": "B5"
            },
            {
              "module": "B6"
            },
            {
              "module": "B7"
            },
            {
              "module": "C1"
            },
            {
              "module": "C2"
            },
            {
              "module": "C3"
            },
            {
              "module": "C4"
            },
            {
              "module": "D"
            },
            {
              "name": "referenceToUnitGroupDataSet",
              "value": {
                "shortDescription": [
                  {
                    "value": "kBq U235 eqv."
                  }
                ],
                "type": "unit group data set",
                "refObjectId": "456b05bf-1415-44a9-9993-02452f554c09",
                "uri": "../unitgroups/456b05bf-1415-44a9-9993-02452f554c09"
              }
            }
          ]
        }
      },
      {
        "referenceToLCIAMethodDataSet": {
          "shortDescription": [
            {
              "value": "Potential Comparative Toxic Unit for ecosystems (ETP-fw)",
              "lang": "en"
            },
            {
              "value": "Potenzielle Toxizit\u00e4tsvergleichseinheit f\u00fcr \u00d6kosysteme (ETP-fw)",
              "lang": "de"
            }
          ],
          "type": "LCIA method data set",
          "refObjectId": "ee1082d1-b0f7-43ca-a1f0-21e2a4a74511",
          "version": "01.00.003",
          "uri": "http://lca.jrc.ec.europa.eu/lcainfohub/datasets/elcd/lciamethods/ee1082d1-b0f7-43ca-a1f0-21e2a4a74511.xml"
        },
        "meanAmount": 0.0,
        "other": {
          "anies": [
            {
              "module": "A1"
            },
            {
              "module": "A2"
            },
            {
              "module": "A3"
            },
            {
              "module": "A1-A3"
            },
            {
              "module": "A4"
            },
            {
              "module": "A5"
            },
            {
              "module": "B1"
            },
            {
              "module": "B2"
            },
            {
              "module": "B3"
            },
            {
              "module": "B4"
            },
            {
              "module": "B5"
            },
            {
              "module": "B6"
            },
            {
              "module": "B7"
            },
            {
              "module": "C1"
            },
            {
              "module": "C2"
            },
            {
              "module": "C3"
            },
            {
              "module": "C4"
            },
            {
              "module": "D"
            },
            {
              "name": "referenceToUnitGroupDataSet",
              "value": {
                "shortDescription": [
                  {
                    "value": "CTUe"
                  }
                ],
                "type": "unit group data set",
                "refObjectId": "aa959ded-f1eb-4efb-9c5c-2d60be36b3e6",
                "uri": "../unitgroups/aa959ded-f1eb-4efb-9c5c-2d60be36b3e6"
              }
            }
          ]
        }
      },
      {
        "referenceToLCIAMethodDataSet": {
          "shortDescription": [
            {
              "value": "Potential Comparative Toxic Unit for humans - cancer effects (HTP-c)",
              "lang": "en"
            },
            {
              "value": "Potenzielle Toxizit\u00e4tsvergleichseinheit f\u00fcr den Menschen - kanzerogene Wirkung (HTP-c)",
              "lang": "de"
            }
          ],
          "type": "LCIA method data set",
          "refObjectId": "2299222a-bbd8-474f-9d4f-4dd1f18aea7c",
          "version": "01.00.004",
          "uri": "http://lca.jrc.ec.europa.eu/lcainfohub/datasets/elcd/lciamethods/2299222a-bbd8-474f-9d4f-4dd1f18aea7c.xml"
        },
        "meanAmount": 0.0,
        "other": {
          "anies": [
            {
              "module": "A1"
            },
            {
              "module": "A2"
            },
            {
              "module": "A3"
            },
            {
              "module": "A1-A3"
            },
            {
              "module": "A4"
            },
            {
              "module": "A5"
            },
            {
              "module": "B1"
            },
            {
              "module": "B2"
            },
            {
              "module": "B3"
            },
            {
              "module": "B4"
            },
            {
              "module": "B5"
            },
            {
              "module": "B6"
            },
            {
              "module": "B7"
            },
            {
              "module": "C1"
            },
            {
              "module": "C2"
            },
            {
              "module": "C3"
            },
            {
              "module": "C4"
            },
            {
              "module": "D"
            },
            {
              "name": "referenceToUnitGroupDataSet",
              "value": {
                "shortDescription": [
                  {
                    "value": "CTUh"
                  }
                ],
                "type": "unit group data set",
                "refObjectId": "d4c9523e-2d7e-49fd-8469-998f547d3a70",
                "uri": "../unitgroups/d4c9523e-2d7e-49fd-8469-998f547d3a70"
              }
            }
          ]
        }
      },
      {
        "referenceToLCIAMethodDataSet": {
          "shortDescription": [
            {
              "value": "Potential Comparative Toxic Unit for humans - non-cancer effects (HTP-nc)",
              "lang": "en"
            },
            {
              "value": "Potenzielle Toxizit\u00e4tsvergleichseinheit f\u00fcr den Menschen - nicht kanzerogene Wirkung (HTP-nc)",
              "lang": "de"
            }
          ],
          "type": "LCIA method data set",
          "refObjectId": "3af763a5-b7a1-48c9-9cee-1f223481fcef",
          "version": "01.00.003",
          "uri": "http://lca.jrc.ec.europa.eu/lcainfohub/datasets/elcd/lciamethods/3af763a5-b7a1-48c9-9cee-1f223481fcef.xml"
        },
        "meanAmount": 0.0,
        "other": {
          "anies": [
            {
              "module": "A1"
            },
            {
              "module": "A2"
            },
            {
              "module": "A3"
            },
            {
              "module": "A1-A3"
            },
            {
              "module": "A4"
            },
            {
              "module": "A5"
            },
            {
              "module": "B1"
            },
            {
              "module": "B2"
            },
            {
              "module": "B3"
            },
            {
              "module": "B4"
            },
            {
              "module": "B5"
            },
            {
              "module": "B6"
            },
            {
              "module": "B7"
            },
            {
              "module": "C1"
            },
            {
              "module": "C2"
            },
            {
              "module": "C3"
            },
            {
              "module": "C4"
            },
            {
              "module": "D"
            },
            {
              "name": "referenceToUnitGroupDataSet",
              "value": {
                "shortDescription": [
                  {
                    "value": "CTUh"
                  }
                ],
                "type": "unit group data set",
                "refObjectId": "d4c9523e-2d7e-49fd-8469-998f547d3a70",
                "uri": "../unitgroups/d4c9523e-2d7e-49fd-8469-998f547d3a70"
              }
            }
          ]
        }
      },
      {
        "referenceToLCIAMethodDataSet": {
          "shortDescription": [
            {
              "value": "Potential Soil quality index (SQP)",
              "lang": "en"
            },
            {
              "value": "Potenzieller Bodenqualit\u00e4tsindex (SQP)",
              "lang": "de"
            }
          ],
          "type": "LCIA method data set",
          "refObjectId": "b2ad6890-c78d-11e6-9d9d-cec0c932ce01",
          "version": "01.00.011"
        },
        "meanAmount": 0.0,
        "other": {
          "anies": [
            {
              "module": "A1"
            },
            {
              "module": "A2"
            },
            {
              "module": "A3"
            },
            {
              "module": "A1-A3"
            },
            {
              "module": "A4"
            },
            {
              "module": "A5"
            },
            {
              "module": "B1"
            },
            {
              "module": "B2"
            },
            {
              "module": "B3"
            },
            {
              "module": "B4"
            },
            {
              "module": "B5"
            },
            {
              "module": "B6"
            },
            {
              "module": "B7"
            },
            {
              "module": "C1"
            },
            {
              "module": "C2"
            },
            {
              "module": "C3"
            },
            {
              "module": "C4"
            },
            {
              "module": "D"
            },
            {
              "name": "referenceToUnitGroupDataSet",
              "value": {
                "shortDescription": [
                  {
                    "value": "dimensionless"
                  }
                ],
                "type": "unit group data set",
                "refObjectId": "f130951c-e67f-4f7f-8dd4-665de3974e18",
                "uri": "../unitgroups/f130951c-e67f-4f7f-8dd4-665de3974e18"
              }
            }
          ]
        }
      }
    ]
  },
  "otherAttributes": {
    "{http://www.indata.network/EPD/2019}epd-version": "1.2",
    "{http://www.okworx.com/ILCD/Extensions/2018/Profile}profile": "EN_15804_A2"
  },
  "version": "1.1",
  "source": "https://node.epditaly.it/resource/datastocks/24493f94-1ca8-4cc7-a056-67cbe25aef5a/processes/073460b5-315d-4480-af0f-e54b496204cd"
}