{
  "processInformation": {
    "dataSetInformation": {
      "UUID": "0b18264c-993d-4a53-8e09-2eb44d178231",
      "name": {
        "baseName": [
          {
            "value": "Air, wind and water barrier membranes and Vapor control layers: TRASPIR EVO 160",
            "lang": "en"
          }
        ]
      },
      "generalComment": [
        {
          "value": "The data quality can be considered as good. The LCA models have been checked and most relevant flows were considered. Technological  geographical and temporal representativeness is appropriate.\n\nInformation about single datasets is documented in http://database-documentation.gabisoftware.com/support/gabi/.\n\nEN 15804 requires that in case of data discrepancies or insufficient input data for a unit process. the cutoff criteria shall be 1% of renewable and non-renewable primary energy usage and 1% of the total mass\nof this unit process. The total neglected flows from a product stage must be no more than 5% of product\ninputs by mass or 5% of primary energy contribution.\nProduction of capital equipment facilities and infrastructure required for manufacture are outside the scope of this assessment.\n\n",
          "lang": "en"
        }
      ]
    },
    "quantitativeReference": {
      "referenceToReferenceFlow": [
        1
      ],
      "type": "Reference flow(s)"
    },
    "time": {
      "referenceYear": 2021,
      "dataSetValidUntil": 2026,
      "other": {
        "anies": [
          {
            "name": "publicationDateOfEPD",
            "value": 1626912000000
          }
        ]
      }
    },
    "geography": {
      "locationOfOperationSupplyOrProduction": {
        "descriptionOfRestrictions": [
          {
            "value": "global",
            "lang": "en"
          }
        ],
        "location": "IT"
      }
    },
    "technology": {
      "technologyDescriptionAndIncludedProcesses": [
        {
          "value": "Mass per unit area: 160 g/m2\nWater vapour transmission (Sd): 0,1 m\nReaction to fire (steel): B-s1,d2\nMaximun tensile force MD/CD: 280-220 N/50mm\nElongation MD/CD: 50-60 %\nResistance to nail tearing MD/CD: 180-200 N",
          "lang": "en"
        }
      ],
      "technologicalApplicability": [
        {
          "value": "The monolithic structure of the membrane guarantees excellent durability over time, thanks to the special polymers used. This Environmental Product Declaration (EPD) is valid for Air, wind and water barrier membranes and Vapor control layers designed by Rothoblass in Europe. MONOLITHIC\nThe monolithic structure of the membrane guarantees excellent durability over time, thanks to the special polymers used.\nREACTION TO FIRE B-s1,d2\nSelf-extinguishing membrane which does not spread the flame in case of fire, contributing to the protection of the structure.\nHIGH UV STABILITY\nIt passed the artificial ageing test involving exposure to UV light for 1000 hours.\nComposition: \ntop layer - non-woven PP fabric\nmiddle layer - breathable monolithic TPE film\nbottom layer - non-woven PP fabric",
          "lang": "en"
        }
      ]
    }
  },
  "modellingAndValidation": {
    "LCIMethodAndAllocation": {
      "typeOfDataSet": "EPD",
      "referenceToLCAMethodDetails": [
        {
          "shortDescription": [
            {
              "value": "PCR ICMQ 3.0 - rev. 3.0 - Products and services for construction",
              "lang": "en"
            }
          ],
          "type": "source data set",
          "refObjectId": "ef443a4d-f05e-423e-89a7-a43134ef23b2",
          "version": "00.00.000"
        }
      ],
      "other": {
        "anies": [
          {
            "name": "subType",
            "value": "specific dataset"
          }
        ]
      }
    },
    "dataSourcesTreatmentAndRepresentativeness": {
      "referenceToDataSource": [
        {
          "shortDescription": [
            {
              "value": "ecoinvent database (all versions)",
              "lang": "en"
            }
          ],
          "type": "source data set",
          "refObjectId": "b497a91f-e14b-4b69-8f28-f50eb1576766",
          "version": "00.03.001",
          "uri": "http://openlca.org/ilcd/resource/sources/b497a91f-e14b-4b69-8f28-f50eb1576766"
        }
      ],
      "useAdviceForDataSet": [
        {
          "value": "cradle to grave: A1, A2, A3, A4, A5, B1, B2, B3, B4, B5, B6, B7, C1, C2, C3, C4, D",
          "lang": "en"
        }
      ],
      "other": {
        "anies": [
          {
            "name": "referenceToOriginalEPD",
            "value": {
              "shortDescription": {},
              "version": {
                "version": 0,
                "majorVersion": 0,
                "minorVersion": 0,
                "subMinorVersion": 0,
                "zero": true,
                "versionString": "00.00.000"
              },
              "type": "source data set",
              "uuid": {
                "uuid": "7dc7317d-fe77-4670-a3dc-e16f9b4086f4"
              },
              "refObjectId": "7dc7317d-fe77-4670-a3dc-e16f9b4086f4",
              "versionAsString": "00.00.000",
              "resourceURLs": [
                "https://node.epditaly.it/resource/sources/7dc7317d-fe77-4670-a3dc-e16f9b4086f4/https://www.epditaly.it/wp-content/uploads/2021/08/RB_EPD2-19-07-2021-v2.pdf?version=00.00.000"
              ]
            }
          }
        ]
      }
    },
    "validation": {
      "review": [
        {
          "referenceToNameOfReviewerAndInstitution": [
            {
              "shortDescription": [
                {
                  "value": "ICMQ spa",
                  "lang": "en"
                }
              ],
              "type": "contact data set",
              "refObjectId": "cbb9d118-f872-4b99-920a-b1078fce25da",
              "version": "00.00.001"
            }
          ],
          "type": "Independent external review"
        }
      ]
    },
    "complianceDeclarations": {
      "compliance": [
        {
          "referenceToComplianceSystem": {
            "shortDescription": [
              {
                "value": "EN 15804+A2",
                "lang": "en"
              }
            ],
            "type": "source data set",
            "refObjectId": "c0016b33-8cf7-415c-ac6e-deba0d21440d",
            "version": "00.02.000"
          },
          "approvalOfOverallCompliance": "Fully compliant",
          "nomenclatureCompliance": "Fully compliant",
          "methodologicalCompliance": "Fully compliant",
          "reviewCompliance": "Fully compliant",
          "documentationCompliance": "Fully compliant",
          "qualityCompliance": "Fully compliant"
        },
        {
          "referenceToComplianceSystem": {
            "shortDescription": [
              {
                "value": "ISO 14025",
                "lang": "en"
              }
            ],
            "type": "source data set",
            "refObjectId": "4f2eb655-6e44-4874-a95a-e28f5442cd4d",
            "version": "00.00.001"
          },
          "approvalOfOverallCompliance": "Fully compliant",
          "nomenclatureCompliance": "Fully compliant",
          "methodologicalCompliance": "Fully compliant",
          "reviewCompliance": "Fully compliant",
          "documentationCompliance": "Fully compliant",
          "qualityCompliance": "Fully compliant"
        },
        {
          "referenceToComplianceSystem": {
            "shortDescription": [
              {
                "value": "ISO 21930",
                "lang": "en"
              }
            ],
            "type": "source data set",
            "refObjectId": "9c1e8451-2321-4498-b459-b6568b6b6547",
            "version": "00.00.001"
          },
          "approvalOfOverallCompliance": "Fully compliant",
          "nomenclatureCompliance": "Fully compliant",
          "methodologicalCompliance": "Fully compliant",
          "reviewCompliance": "Fully compliant",
          "documentationCompliance": "Fully compliant",
          "qualityCompliance": "Fully compliant"
        }
      ]
    }
  },
  "administrativeInformation": {
    "dataGenerator": {
      "referenceToPersonOrEntityGeneratingTheDataSet": [
        {
          "shortDescription": [
            {
              "value": "LCA.no AS",
              "lang": "en"
            }
          ],
          "type": "contact data set",
          "refObjectId": "77a6868e-b256-47c8-a410-32706b6e1814",
          "version": "00.00.001"
        }
      ]
    },
    "dataEntryBy": {
      "timeStamp": 1692724943000,
      "referenceToDataSetFormat": [
        {
          "shortDescription": [
            {
              "value": "ILCD format",
              "lang": "en"
            }
          ],
          "type": "source data set",
          "refObjectId": "a97a0155-0234-4b87-b4ce-a45da52f2a40",
          "version": "01.00.000",
          "uri": "http://lca.jrc.ec.europa.eu/lcainfohub/sample_data/ilcd/sources/ILCD_Format_a97a0155-0234-4b87-b4ce-a45da52f2a40_01.00.000.xml"
        },
        {
          "shortDescription": [
            {
              "value": "EPD Data Format Extensions v1.2",
              "lang": "no"
            },
            {
              "value": "EPD Data Format Extensions v1.2",
              "lang": "en"
            },
            {
              "value": "EPD-Datenformaterweiterungen v1.2",
              "lang": "de"
            }
          ],
          "type": "source data set",
          "refObjectId": "a29449fd-aa2f-4de8-b5d7-4b06b43c6fde",
          "version": "00.01.000"
        }
      ]
    },
    "publicationAndOwnership": {
      "dataSetVersion": "00.03.000",
      "dateOfLastRevision": 1692717259270,
      "referenceToRegistrationAuthority": {
        "shortDescription": [
          {
            "value": "EPDItaly",
            "lang": "en"
          }
        ],
        "type": "contact data set",
        "refObjectId": "9433b9cf-1d4a-420f-8c09-88d2472225b9",
        "version": "00.00.004"
      },
      "registrationNumber": "EPDITALY0141",
      "referenceToOwnershipOfDataSet": {
        "shortDescription": [
          {
            "value": "ROTHO BLAAS SRL",
            "lang": "en"
          }
        ],
        "type": "contact data set",
        "refObjectId": "f20012c7-12e2-446f-b704-48987359f415",
        "version": "00.00.000"
      },
      "copyright": true,
      "licenseType": "Free of charge for all users and uses",
      "accessRestrictions": [
        {
          "value": "None",
          "lang": "en"
        }
      ],
      "other": {
        "anies": [
          {
            "name": "referenceToPublisher",
            "value": {
              "shortDescription": [
                {
                  "value": "EPDItaly",
                  "lang": "en"
                }
              ],
              "type": "contact data set",
              "refObjectId": "9433b9cf-1d4a-420f-8c09-88d2472225b9",
              "version": "00.00.004"
            }
          }
        ]
      }
    }
  },
  "exchanges": {
    "exchange": [
      {
        "dataSetInternalID": 1,
        "referenceToFlowDataSet": {
          "shortDescription": [
            {
              "value": "Air, wind and water barrier membranes and Vapor control layers: TRASPIR EVO 160",
              "lang": "en"
            }
          ],
          "type": "flow data set",
          "refObjectId": "c5076b81-e97e-4d2f-905d-19af725b5349",
          "version": "00.01.000"
        },
        "exchange direction": "OUTPUT",
        "meanAmount": 1.0,
        "resultingAmount": 1.0,
        "minimumAmount": 0.0,
        "maximumAmount": 0.0,
        "uncertaintyDistributionType": "UNDEFINED",
        "relativeStandardDeviation95In": "0",
        "dataSourceType": "Primary",
        "dataDerivationTypeStatus": "MEASURED",
        "referenceFlow": true,
        "resultingflowAmount": 1.0,
        "flowProperties": [
          {
            "name": [
              {
                "lang": "no",
                "value": "Masse"
              },
              {
                "lang": "en",
                "value": "Mass"
              }
            ],
            "uuid": "93a60a56-a3c8-11da-a746-0800200b9a66",
            "meanValue": 0.0
          },
          {
            "name": [
              {
                "lang": "no",
                "value": "Innhold av biogent karbon i produkt"
              },
              {
                "lang": "en",
                "value": "Carbon content (biogenic)"
              }
            ],
            "uuid": "62e503ce-544a-4599-b2ad-bcea15a7bf20",
            "meanValue": 0.0
          },
          {
            "name": [
              {
                "lang": "en",
                "value": "Area"
              },
              {
                "lang": "de",
                "value": "Fl\u00e4che"
              }
            ],
            "uuid": "93a60a56-a3c8-19da-a746-0800200c9a66",
            "referenceFlowProperty": true,
            "meanValue": 1.0,
            "referenceUnit": "qm",
            "unitGroupUUID": "c20a03d7-bd90-4569-bc94-66cfd364dfc8"
          },
          {
            "name": [
              {
                "lang": "no",
                "value": "Innhold av biogent karbon i emballasjen"
              },
              {
                "lang": "en",
                "value": "Carbon content (biogenic) - packaging"
              }
            ],
            "uuid": "262a541b-209e-44cc-a426-33bce30de7b1",
            "meanValue": 0.00378
          }
        ],
        "typeOfFlow": "Product flow"
      },
      {
        "dataSetInternalID": 2,
        "referenceToFlowDataSet": {
          "shortDescription": [
            {
              "value": "Use of renewable primary energy (PERE)",
              "lang": "en"
            },
            {
              "value": "Fornybar prim\u00e6renergi brukt som energib\u00e6rer (RPEE)",
              "lang": "no"
            }
          ],
          "type": "flow data set",
          "refObjectId": "20f32be5-0398-4288-9b6d-accddd195317",
          "version": "30.00.000"
        },
        "exchange direction": "INPUT",
        "meanAmount": 0.0,
        "resultingAmount": 0.0,
        "minimumAmount": 0.0,
        "maximumAmount": 0.0,
        "uncertaintyDistributionType": "UNDEFINED",
        "relativeStandardDeviation95In": "0",
        "dataSourceType": "Primary",
        "dataDerivationTypeStatus": "MEASURED",
        "other": {
          "anies": [
            {
              "value": "0.988000000000",
              "module": "A1"
            },
            {
              "value": "0.007920000000",
              "module": "A2"
            },
            {
              "value": "-0.000089000000",
              "module": "A3"
            },
            {
              "value": "0.014900000000",
              "module": "A4"
            },
            {
              "value": "0.113000000000",
              "module": "A5"
            },
            {
              "value": "0.000000000000",
              "module": "B1"
            },
            {
              "value": "0.000000000000",
              "module": "B2"
            },
            {
              "value": "0.000000000000",
              "module": "B3"
            },
            {
              "value": "0.000000000000",
              "module": "B4"
            },
            {
              "value": "0.000000000000",
              "module": "B5"
            },
            {
              "value": "0.000000000000",
              "module": "B6"
            },
            {
              "value": "0.000000000000",
              "module": "B7"
            },
            {
              "value": "0.017000000000",
              "module": "C1"
            },
            {
              "value": "0.003860000000",
              "module": "C2"
            },
            {
              "value": "0.046200000000",
              "module": "C3"
            },
            {
              "value": "0.008820000000",
              "module": "C4"
            },
            {
              "value": "-0.237000000000",
              "module": "D"
            },
            {
              "name": "referenceToUnitGroupDataSet",
              "value": {
                "shortDescription": [
                  {
                    "value": "MJ"
                  }
                ],
                "type": "unit group data set",
                "refObjectId": "93a60a57-a3c8-11da-a746-0800200c9a66",
                "uri": "../unitgroups/93a60a57-a3c8-11da-a746-0800200c9a66"
              }
            }
          ]
        },
        "flowProperties": [],
        "typeOfFlow": "Other flow",
        "classification": {
          "classHierarchy": "Gr\u00f6\u00dfen / Umweltliche Gr\u00f6\u00dfen / EPD EN 15804 / LCI Indikatoren",
          "name": "GaBiCategories"
        }
      },
      {
        "dataSetInternalID": 3,
        "referenceToFlowDataSet": {
          "shortDescription": [
            {
              "value": "Use of renewable primary energy resources used as raw materials (PERM)",
              "lang": "en"
            },
            {
              "value": "Fornybar prim\u00e6renergi brukt som energib\u00e6rer (RPEE)",
              "lang": "no"
            }
          ],
          "type": "flow data set",
          "refObjectId": "fb3ec0de-548d-4508-aea5-00b73bf6f702",
          "version": "30.00.000"
        },
        "exchange direction": "INPUT",
        "meanAmount": 0.0,
        "resultingAmount": 0.0,
        "minimumAmount": 0.0,
        "maximumAmount": 0.0,
        "uncertaintyDistributionType": "UNDEFINED",
        "relativeStandardDeviation95In": "0",
        "dataSourceType": "Primary",
        "dataDerivationTypeStatus": "MEASURED",
        "other": {
          "anies": [
            {
              "value": "0.138000000000",
              "module": "A1"
            },
            {
              "value": "0.000000000000",
              "module": "A2"
            },
            {
              "value": "0.020100000000",
              "module": "A3"
            },
            {
              "value": "0.000000000000",
              "module": "A4"
            },
            {
              "value": "0.006510000000",
              "module": "A5"
            },
            {
              "value": "0.000000000000",
              "module": "B1"
            },
            {
              "value": "0.000000000000",
              "module": "B2"
            },
            {
              "value": "0.000000000000",
              "module": "B3"
            },
            {
              "value": "0.000000000000",
              "module": "B4"
            },
            {
              "value": "0.000000000000",
              "module": "B5"
            },
            {
              "value": "0.000000000000",
              "module": "B6"
            },
            {
              "value": "0.000000000000",
              "module": "B7"
            },
            {
              "value": "0.000000000000",
              "module": "C1"
            },
            {
              "value": "0.000000000000",
              "module": "C2"
            },
            {
              "value": "0.000000000000",
              "module": "C3"
            },
            {
              "value": "0.000000000000",
              "module": "C4"
            },
            {
              "value": "0.000000000000",
              "module": "D"
            },
            {
              "name": "referenceToUnitGroupDataSet",
              "value": {
                "shortDescription": [
                  {
                    "value": "MJ"
                  }
                ],
                "type": "unit group data set",
                "refObjectId": "93a60a57-a3c8-11da-a746-0800200c9a66",
                "uri": "../unitgroups/93a60a57-a3c8-11da-a746-0800200c9a66"
              }
            }
          ]
        },
        "flowProperties": [],
        "typeOfFlow": "Other flow",
        "classification": {
          "classHierarchy": "Gr\u00f6\u00dfen / Umweltliche Gr\u00f6\u00dfen / EPD EN 15804 / LCI Indikatoren",
          "name": "GaBiCategories"
        }
      },
      {
        "dataSetInternalID": 4,
        "referenceToFlowDataSet": {
          "shortDescription": [
            {
              "value": "Total use of renewable primary energy resource (PERT)",
              "lang": "en"
            },
            {
              "value": "Total bruk av fornybar prim\u00e6renergi (TPE)",
              "lang": "no"
            }
          ],
          "type": "flow data set",
          "refObjectId": "53f97275-fa8a-4cdd-9024-65936002acd0",
          "version": "30.00.000"
        },
        "exchange direction": "INPUT",
        "meanAmount": 0.0,
        "resultingAmount": 0.0,
        "minimumAmount": 0.0,
        "maximumAmount": 0.0,
        "uncertaintyDistributionType": "UNDEFINED",
        "relativeStandardDeviation95In": "0",
        "dataSourceType": "Primary",
        "dataDerivationTypeStatus": "MEASURED",
        "other": {
          "anies": [
            {
              "value": "1.130000000000",
              "module": "A1"
            },
            {
              "value": "0.007920000000",
              "module": "A2"
            },
            {
              "value": "0.020000000000",
              "module": "A3"
            },
            {
              "value": "0.014900000000",
              "module": "A4"
            },
            {
              "value": "0.119000000000",
              "module": "A5"
            },
            {
              "value": "0.000000000000",
              "module": "B1"
            },
            {
              "value": "0.000000000000",
              "module": "B2"
            },
            {
              "value": "0.000000000000",
              "module": "B3"
            },
            {
              "value": "0.000000000000",
              "module": "B4"
            },
            {
              "value": "0.000000000000",
              "module": "B5"
            },
            {
              "value": "0.000000000000",
              "module": "B6"
            },
            {
              "value": "0.000000000000",
              "module": "B7"
            },
            {
              "value": "0.017000000000",
              "module": "C1"
            },
            {
              "value": "0.003860000000",
              "module": "C2"
            },
            {
              "value": "0.046200000000",
              "module": "C3"
            },
            {
              "value": "0.008820000000",
              "module": "C4"
            },
            {
              "value": "0.237000000000",
              "module": "D"
            },
            {
              "name": "referenceToUnitGroupDataSet",
              "value": {
                "shortDescription": [
                  {
                    "value": "MJ"
                  }
                ],
                "type": "unit group data set",
                "refObjectId": "93a60a57-a3c8-11da-a746-0800200c9a66",
                "uri": "../unitgroups/93a60a57-a3c8-11da-a746-0800200c9a66"
              }
            }
          ]
        },
        "flowProperties": [],
        "typeOfFlow": "Other flow",
        "classification": {
          "classHierarchy": "Gr\u00f6\u00dfen / Umweltliche Gr\u00f6\u00dfen / EPD EN 15804 / LCI Indikatoren",
          "name": "GaBiCategories"
        }
      },
      {
        "dataSetInternalID": 5,
        "referenceToFlowDataSet": {
          "shortDescription": [
            {
              "value": "Use of non renewable primary energy (PENRE)",
              "lang": "en"
            },
            {
              "value": "Ikke fornybar prim\u00e6renergi brukt som energib\u00e6rer (NRPE)",
              "lang": "no"
            }
          ],
          "type": "flow data set",
          "refObjectId": "ac857178-2b45-46ec-892a-a9a4332f0372",
          "version": "30.00.000"
        },
        "exchange direction": "INPUT",
        "meanAmount": 0.0,
        "resultingAmount": 0.0,
        "minimumAmount": 0.0,
        "maximumAmount": 0.0,
        "uncertaintyDistributionType": "UNDEFINED",
        "relativeStandardDeviation95In": "0",
        "dataSourceType": "Primary",
        "dataDerivationTypeStatus": "MEASURED",
        "other": {
          "anies": [
            {
              "value": "9.910000000000",
              "module": "A1"
            },
            {
              "value": "0.138000000000",
              "module": "A2"
            },
            {
              "value": "0.009330000000",
              "module": "A3"
            },
            {
              "value": "0.318000000000",
              "module": "A4"
            },
            {
              "value": "1.120000000000",
              "module": "A5"
            },
            {
              "value": "0.000000000000",
              "module": "B1"
            },
            {
              "value": "0.000000000000",
              "module": "B2"
            },
            {
              "value": "0.000000000000",
              "module": "B3"
            },
            {
              "value": "0.000000000000",
              "module": "B4"
            },
            {
              "value": "0.000000000000",
              "module": "B5"
            },
            {
              "value": "0.000000000000",
              "module": "B6"
            },
            {
              "value": "0.000000000000",
              "module": "B7"
            },
            {
              "value": "0.036800000000",
              "module": "C1"
            },
            {
              "value": "0.069200000000",
              "module": "C2"
            },
            {
              "value": "1.260000000000",
              "module": "C3"
            },
            {
              "value": "0.121000000000",
              "module": "C4"
            },
            {
              "value": "-2.760000000000",
              "module": "D"
            },
            {
              "name": "referenceToUnitGroupDataSet",
              "value": {
                "shortDescription": [
                  {
                    "value": "MJ"
                  }
                ],
                "type": "unit group data set",
                "refObjectId": "93a60a57-a3c8-11da-a746-0800200c9a66",
                "uri": "../unitgroups/93a60a57-a3c8-11da-a746-0800200c9a66"
              }
            }
          ]
        },
        "flowProperties": [],
        "typeOfFlow": "Other flow",
        "classification": {
          "classHierarchy": "Gr\u00f6\u00dfen / Umweltliche Gr\u00f6\u00dfen / EPD EN 15804 / LCI Indikatoren",
          "name": "GaBiCategories"
        }
      },
      {
        "dataSetInternalID": 6,
        "referenceToFlowDataSet": {
          "shortDescription": [
            {
              "value": "Use of non renewable primary energy resources used as raw materials (PENRM)",
              "lang": "en"
            },
            {
              "value": "Ikke fornybar prim\u00e6renergi brukt som r\u00e5materiale (NRPM)",
              "lang": "no"
            }
          ],
          "type": "flow data set",
          "refObjectId": "1421caa0-679d-4bf4-b282-0eb850ccae27",
          "version": "30.00.000"
        },
        "exchange direction": "INPUT",
        "meanAmount": 0.0,
        "resultingAmount": 0.0,
        "minimumAmount": 0.0,
        "maximumAmount": 0.0,
        "uncertaintyDistributionType": "UNDEFINED",
        "relativeStandardDeviation95In": "0",
        "dataSourceType": "Primary",
        "dataDerivationTypeStatus": "MEASURED",
        "other": {
          "anies": [
            {
              "value": "7.280000000000",
              "module": "A1"
            },
            {
              "value": "0.000000000000",
              "module": "A2"
            },
            {
              "value": "0.003360000000",
              "module": "A3"
            },
            {
              "value": "0.000000000000",
              "module": "A4"
            },
            {
              "value": "0.606000000000",
              "module": "A5"
            },
            {
              "value": "0.000000000000",
              "module": "B1"
            },
            {
              "value": "0.000000000000",
              "module": "B2"
            },
            {
              "value": "0.000000000000",
              "module": "B3"
            },
            {
              "value": "0.000000000000",
              "module": "B4"
            },
            {
              "value": "0.000000000000",
              "module": "B5"
            },
            {
              "value": "0.000000000000",
              "module": "B6"
            },
            {
              "value": "0.000000000000",
              "module": "B7"
            },
            {
              "value": "0.000000000000",
              "module": "C1"
            },
            {
              "value": "0.000000000000",
              "module": "C2"
            },
            {
              "value": "-1.090000000000",
              "module": "C3"
            },
            {
              "value": "0.000000000000",
              "module": "C4"
            },
            {
              "value": "0.000000000000",
              "module": "D"
            },
            {
              "name": "referenceToUnitGroupDataSet",
              "value": {
                "shortDescription": [
                  {
                    "value": "MJ"
                  }
                ],
                "type": "unit group data set",
                "refObjectId": "93a60a57-a3c8-11da-a746-0800200c9a66",
                "uri": "../unitgroups/93a60a57-a3c8-11da-a746-0800200c9a66"
              }
            }
          ]
        },
        "flowProperties": [],
        "typeOfFlow": "Other flow",
        "classification": {
          "classHierarchy": "Gr\u00f6\u00dfen / Umweltliche Gr\u00f6\u00dfen / EPD EN 15804 / LCI Indikatoren",
          "name": "GaBiCategories"
        }
      },
      {
        "dataSetInternalID": 7,
        "referenceToFlowDataSet": {
          "shortDescription": [
            {
              "value": "Total use of non renewable primary energy resource (PENRT)",
              "lang": "en"
            },
            {
              "value": "Total nicht erneuerbare Prim\u00e4renergie (PENRT)",
              "lang": "no"
            }
          ],
          "type": "flow data set",
          "refObjectId": "06159210-646b-4c8d-8583-da9b3b95a6c1",
          "version": "30.00.000"
        },
        "exchange direction": "INPUT",
        "meanAmount": 0.0,
        "resultingAmount": 0.0,
        "minimumAmount": 0.0,
        "maximumAmount": 0.0,
        "uncertaintyDistributionType": "UNDEFINED",
        "relativeStandardDeviation95In": "0",
        "dataSourceType": "Primary",
        "dataDerivationTypeStatus": "MEASURED",
        "other": {
          "anies": [
            {
              "value": "17.200000000000",
              "module": "A1"
            },
            {
              "value": "0.138000000000",
              "module": "A2"
            },
            {
              "value": "0.012700000000",
              "module": "A3"
            },
            {
              "value": "0.318000000000",
              "module": "A4"
            },
            {
              "value": "1.730000000000",
              "module": "A5"
            },
            {
              "value": "0.000000000000",
              "module": "B1"
            },
            {
              "value": "0.000000000000",
              "module": "B2"
            },
            {
              "value": "0.000000000000",
              "module": "B3"
            },
            {
              "value": "0.000000000000",
              "module": "B4"
            },
            {
              "value": "0.000000000000",
              "module": "B5"
            },
            {
              "value": "0.000000000000",
              "module": "B6"
            },
            {
              "value": "0.000000000000",
              "module": "B7"
            },
            {
              "value": "0.036800000000",
              "module": "C1"
            },
            {
              "value": "0.069200000000",
              "module": "C2"
            },
            {
              "value": "0.168000000000",
              "module": "C3"
            },
            {
              "value": "0.121000000000",
              "module": "C4"
            },
            {
              "value": "-2.760000000000",
              "module": "D"
            },
            {
              "name": "referenceToUnitGroupDataSet",
              "value": {
                "shortDescription": [
                  {
                    "value": "MJ"
                  }
                ],
                "type": "unit group data set",
                "refObjectId": "93a60a57-a3c8-11da-a746-0800200c9a66",
                "uri": "../unitgroups/93a60a57-a3c8-11da-a746-0800200c9a66"
              }
            }
          ]
        },
        "flowProperties": [],
        "typeOfFlow": "Other flow",
        "classification": {
          "classHierarchy": "Gr\u00f6\u00dfen / Umweltliche Gr\u00f6\u00dfen / EPD EN 15804 / LCI Indikatoren",
          "name": "GaBiCategories"
        }
      },
      {
        "dataSetInternalID": 8,
        "referenceToFlowDataSet": {
          "shortDescription": [
            {
              "value": "Use of secondary material (SM)",
              "lang": "en"
            },
            {
              "value": "Bruk av sekund\u00e6re materialer (SM)",
              "lang": "no"
            }
          ],
          "type": "flow data set",
          "refObjectId": "c6a1f35f-2d09-4f54-8dfb-97e502e1ce92",
          "version": "30.00.000"
        },
        "exchange direction": "INPUT",
        "meanAmount": 0.0,
        "resultingAmount": 0.0,
        "minimumAmount": 0.0,
        "maximumAmount": 0.0,
        "uncertaintyDistributionType": "UNDEFINED",
        "relativeStandardDeviation95In": "0",
        "dataSourceType": "Primary",
        "dataDerivationTypeStatus": "MEASURED",
        "other": {
          "anies": [
            {
              "value": "0.003080000000",
              "module": "A1"
            },
            {
              "value": "0.000000000000",
              "module": "A2"
            },
            {
              "value": "0.000000000000",
              "module": "A3"
            },
            {
              "value": "0.000000000000",
              "module": "A4"
            },
            {
              "value": "0.000385000000",
              "module": "A5"
            },
            {
              "value": "0.000000000000",
              "module": "B1"
            },
            {
              "value": "0.000000000000",
              "module": "B2"
            },
            {
              "value": "0.000000000000",
              "module": "B3"
            },
            {
              "value": "0.000000000000",
              "module": "B4"
            },
            {
              "value": "0.000000000000",
              "module": "B5"
            },
            {
              "value": "0.000000000000",
              "module": "B6"
            },
            {
              "value": "0.000000000000",
              "module": "B7"
            },
            {
              "value": "0.000000000000",
              "module": "C1"
            },
            {
              "value": "0.000000000000",
              "module": "C2"
            },
            {
              "value": "0.000000000000",
              "module": "C3"
            },
            {
              "value": "0.000000000000",
              "module": "C4"
            },
            {
              "value": "0.000000000000",
              "module": "D"
            },
            {
              "name": "referenceToUnitGroupDataSet",
              "value": {
                "shortDescription": [
                  {
                    "value": "kg"
                  }
                ],
                "type": "unit group data set",
                "refObjectId": "ad38d542-3fe9-439d-9b95-2f5f7752acaf",
                "uri": "../unitgroups/ad38d542-3fe9-439d-9b95-2f5f7752acaf"
              }
            }
          ]
        },
        "flowProperties": [],
        "typeOfFlow": "Other flow",
        "classification": {
          "classHierarchy": "Gr\u00f6\u00dfen / Umweltliche Gr\u00f6\u00dfen / EPD EN 15804 / LCI Indikatoren",
          "name": "GaBiCategories"
        }
      },
      {
        "dataSetInternalID": 9,
        "referenceToFlowDataSet": {
          "shortDescription": [
            {
              "value": "Use of renewable secondary fuels (RSF)",
              "lang": "en"
            },
            {
              "value": "Bruk av fornybart sekund\u00e6re brensel (RSF)",
              "lang": "no"
            }
          ],
          "type": "flow data set",
          "refObjectId": "64333088-a55f-4aa2-9a31-c10b07816787",
          "version": "30.00.000"
        },
        "exchange direction": "INPUT",
        "meanAmount": 0.0,
        "resultingAmount": 0.0,
        "minimumAmount": 0.0,
        "maximumAmount": 0.0,
        "uncertaintyDistributionType": "UNDEFINED",
        "relativeStandardDeviation95In": "0",
        "dataSourceType": "Primary",
        "dataDerivationTypeStatus": "MEASURED",
        "other": {
          "anies": [
            {
              "value": "0.000000000000",
              "module": "A1"
            },
            {
              "value": "0.000000000000",
              "module": "A2"
            },
            {
              "value": "0.000000000000",
              "module": "A3"
            },
            {
              "value": "0.000000000000",
              "module": "A4"
            },
            {
              "value": "0.000000000000",
              "module": "A5"
            },
            {
              "value": "0.000000000000",
              "module": "B1"
            },
            {
              "value": "0.000000000000",
              "module": "B2"
            },
            {
              "value": "0.000000000000",
              "module": "B3"
            },
            {
              "value": "0.000000000000",
              "module": "B4"
            },
            {
              "value": "0.000000000000",
              "module": "B5"
            },
            {
              "value": "0.000000000000",
              "module": "B6"
            },
            {
              "value": "0.000000000000",
              "module": "B7"
            },
            {
              "value": "0.000000000000",
              "module": "C1"
            },
            {
              "value": "0.000000000000",
              "module": "C2"
            },
            {
              "value": "0.000000000000",
              "module": "C3"
            },
            {
              "value": "0.000000000000",
              "module": "C4"
            },
            {
              "value": "0.000000000000",
              "module": "D"
            },
            {
              "name": "referenceToUnitGroupDataSet",
              "value": {
                "shortDescription": [
                  {
                    "value": "MJ"
                  }
                ],
                "type": "unit group data set",
                "refObjectId": "93a60a57-a3c8-11da-a746-0800200c9a66",
                "uri": "../unitgroups/93a60a57-a3c8-11da-a746-0800200c9a66"
              }
            }
          ]
        },
        "flowProperties": [],
        "typeOfFlow": "Other flow",
        "classification": {
          "classHierarchy": "Gr\u00f6\u00dfen / Umweltliche Gr\u00f6\u00dfen / EPD EN 15804 / LCI Indikatoren",
          "name": "GaBiCategories"
        }
      },
      {
        "dataSetInternalID": 10,
        "referenceToFlowDataSet": {
          "shortDescription": [
            {
              "value": "Use of non renewable secondary fuels (NRSF)",
              "lang": "en"
            },
            {
              "value": "Bruk av ikke fornybart sekund\u00e6re brensel (NRSF)",
              "lang": "no"
            }
          ],
          "type": "flow data set",
          "refObjectId": "89def144-d39a-4287-b86f-efde453ddcb2",
          "version": "30.00.000"
        },
        "exchange direction": "INPUT",
        "meanAmount": 0.0,
        "resultingAmount": 0.0,
        "minimumAmount": 0.0,
        "maximumAmount": 0.0,
        "uncertaintyDistributionType": "UNDEFINED",
        "relativeStandardDeviation95In": "0",
        "dataSourceType": "Primary",
        "dataDerivationTypeStatus": "MEASURED",
        "other": {
          "anies": [
            {
              "value": "0.000000000000",
              "module": "A1"
            },
            {
              "value": "0.000000000000",
              "module": "A2"
            },
            {
              "value": "0.000000000000",
              "module": "A3"
            },
            {
              "value": "0.000000000000",
              "module": "A4"
            },
            {
              "value": "0.000000000000",
              "module": "A5"
            },
            {
              "value": "0.000000000000",
              "module": "B1"
            },
            {
              "value": "0.000000000000",
              "module": "B2"
            },
            {
              "value": "0.000000000000",
              "module": "B3"
            },
            {
              "value": "0.000000000000",
              "module": "B4"
            },
            {
              "value": "0.000000000000",
              "module": "B5"
            },
            {
              "value": "0.000000000000",
              "module": "B6"
            },
            {
              "value": "0.000000000000",
              "module": "B7"
            },
            {
              "value": "0.000000000000",
              "module": "C1"
            },
            {
              "value": "0.000000000000",
              "module": "C2"
            },
            {
              "value": "0.000000000000",
              "module": "C3"
            },
            {
              "value": "0.000000000000",
              "module": "C4"
            },
            {
              "value": "0.000000000000",
              "module": "D"
            },
            {
              "name": "referenceToUnitGroupDataSet",
              "value": {
                "shortDescription": [
                  {
                    "value": "MJ"
                  }
                ],
                "type": "unit group data set",
                "refObjectId": "93a60a57-a3c8-11da-a746-0800200c9a66",
                "uri": "../unitgroups/93a60a57-a3c8-11da-a746-0800200c9a66"
              }
            }
          ]
        },
        "flowProperties": [],
        "typeOfFlow": "Other flow",
        "classification": {
          "classHierarchy": "Gr\u00f6\u00dfen / Umweltliche Gr\u00f6\u00dfen / EPD EN 15804 / LCI Indikatoren",
          "name": "GaBiCategories"
        }
      },
      {
        "dataSetInternalID": 11,
        "referenceToFlowDataSet": {
          "shortDescription": [
            {
              "value": "Use of net fresh water (FW)",
              "lang": "en"
            },
            {
              "value": "Netto bruk av ferskvann (W)",
              "lang": "no"
            }
          ],
          "type": "flow data set",
          "refObjectId": "3cf952c8-f3a4-461d-8c96-96456ca62246",
          "version": "30.00.000"
        },
        "exchange direction": "INPUT",
        "meanAmount": 0.0,
        "resultingAmount": 0.0,
        "minimumAmount": 0.0,
        "maximumAmount": 0.0,
        "uncertaintyDistributionType": "UNDEFINED",
        "relativeStandardDeviation95In": "0",
        "dataSourceType": "Primary",
        "dataDerivationTypeStatus": "MEASURED",
        "other": {
          "anies": [
            {
              "value": "0.003370000000",
              "module": "A1"
            },
            {
              "value": "0.000009080000",
              "module": "A2"
            },
            {
              "value": "0.000004140000",
              "module": "A3"
            },
            {
              "value": "0.000017200000",
              "module": "A4"
            },
            {
              "value": "0.000355000000",
              "module": "A5"
            },
            {
              "value": "0.000000000000",
              "module": "B1"
            },
            {
              "value": "0.000000000000",
              "module": "B2"
            },
            {
              "value": "0.000000000000",
              "module": "B3"
            },
            {
              "value": "0.000000000000",
              "module": "B4"
            },
            {
              "value": "0.000000000000",
              "module": "B5"
            },
            {
              "value": "0.000000000000",
              "module": "B6"
            },
            {
              "value": "0.000000000000",
              "module": "B7"
            },
            {
              "value": "0.000016500000",
              "module": "C1"
            },
            {
              "value": "0.000004420000",
              "module": "C2"
            },
            {
              "value": "0.000244000000",
              "module": "C3"
            },
            {
              "value": "0.000003240000",
              "module": "C4"
            },
            {
              "value": "-0.000533000000",
              "module": "D"
            },
            {
              "name": "referenceToUnitGroupDataSet",
              "value": {
                "shortDescription": [
                  {
                    "value": "m3"
                  }
                ],
                "type": "unit group data set",
                "refObjectId": "cd950537-0a98-4044-9ba7-9f9a68d0a504",
                "uri": "../unitgroups/cd950537-0a98-4044-9ba7-9f9a68d0a504"
              }
            }
          ]
        },
        "flowProperties": [],
        "typeOfFlow": "Other flow",
        "classification": {
          "classHierarchy": "Gr\u00f6\u00dfen / Umweltliche Gr\u00f6\u00dfen / EPD EN 15804 / LCI Indikatoren",
          "name": "GaBiCategories"
        }
      },
      {
        "dataSetInternalID": 12,
        "referenceToFlowDataSet": {
          "shortDescription": [
            {
              "value": "Hazardous waste disposed (HWD)",
              "lang": "en"
            },
            {
              "value": "Avhendet farlig avfall (HW)",
              "lang": "no"
            }
          ],
          "type": "flow data set",
          "refObjectId": "430f9e0f-59b2-46a0-8e0d-55e0e84948fc",
          "version": "30.00.000"
        },
        "exchange direction": "OUTPUT",
        "meanAmount": 0.0,
        "resultingAmount": 0.0,
        "minimumAmount": 0.0,
        "maximumAmount": 0.0,
        "uncertaintyDistributionType": "UNDEFINED",
        "relativeStandardDeviation95In": "0",
        "dataSourceType": "Primary",
        "dataDerivationTypeStatus": "MEASURED",
        "other": {
          "anies": [
            {
              "value": "0.000000006990",
              "module": "A1"
            },
            {
              "value": "0.000000000007",
              "module": "A2"
            },
            {
              "value": "0.000000000055",
              "module": "A3"
            },
            {
              "value": "0.000000000014",
              "module": "A4"
            },
            {
              "value": "0.000000000707",
              "module": "A5"
            },
            {
              "value": "0.000000000000",
              "module": "B1"
            },
            {
              "value": "0.000000000000",
              "module": "B2"
            },
            {
              "value": "0.000000000000",
              "module": "B3"
            },
            {
              "value": "0.000000000000",
              "module": "B4"
            },
            {
              "value": "0.000000000000",
              "module": "B5"
            },
            {
              "value": "0.000000000000",
              "module": "B6"
            },
            {
              "value": "0.000000000000",
              "module": "B7"
            },
            {
              "value": "0.000000000010",
              "module": "C1"
            },
            {
              "value": "0.000000000003",
              "module": "C2"
            },
            {
              "value": "0.000000000039",
              "module": "C3"
            },
            {
              "value": "0.000000000022",
              "module": "C4"
            },
            {
              "value": "-0.000000000632",
              "module": "D"
            },
            {
              "name": "referenceToUnitGroupDataSet",
              "value": {
                "shortDescription": [
                  {
                    "value": "kg"
                  }
                ],
                "type": "unit group data set",
                "refObjectId": "ad38d542-3fe9-439d-9b95-2f5f7752acaf",
                "uri": "../unitgroups/ad38d542-3fe9-439d-9b95-2f5f7752acaf"
              }
            }
          ]
        },
        "flowProperties": [],
        "typeOfFlow": "Other flow",
        "classification": {
          "classHierarchy": "Gr\u00f6\u00dfen / Umweltliche Gr\u00f6\u00dfen / EPD EN 15804 / LCI Indikatoren",
          "name": "GaBiCategories"
        }
      },
      {
        "dataSetInternalID": 13,
        "referenceToFlowDataSet": {
          "shortDescription": [
            {
              "value": "Non hazardous waste dispose (NHWD)",
              "lang": "en"
            },
            {
              "value": "Avhendet ikke-farlig avfall (NHW)",
              "lang": "no"
            }
          ],
          "type": "flow data set",
          "refObjectId": "b29ef66b-e286-4afa-949f-62f1a7b4d7fa",
          "version": "30.00.000"
        },
        "exchange direction": "OUTPUT",
        "meanAmount": 0.0,
        "resultingAmount": 0.0,
        "minimumAmount": 0.0,
        "maximumAmount": 0.0,
        "uncertaintyDistributionType": "UNDEFINED",
        "relativeStandardDeviation95In": "0",
        "dataSourceType": "Primary",
        "dataDerivationTypeStatus": "MEASURED",
        "other": {
          "anies": [
            {
              "value": "0.009560000000",
              "module": "A1"
            },
            {
              "value": "0.000021700000",
              "module": "A2"
            },
            {
              "value": "0.000452000000",
              "module": "A3"
            },
            {
              "value": "0.000046400000",
              "module": "A4"
            },
            {
              "value": "0.019200000000",
              "module": "A5"
            },
            {
              "value": "0.000000000000",
              "module": "B1"
            },
            {
              "value": "0.000000000000",
              "module": "B2"
            },
            {
              "value": "0.000000000000",
              "module": "B3"
            },
            {
              "value": "0.000000000000",
              "module": "B4"
            },
            {
              "value": "0.000000000000",
              "module": "B5"
            },
            {
              "value": "0.000000000000",
              "module": "B6"
            },
            {
              "value": "0.000000000000",
              "module": "B7"
            },
            {
              "value": "0.000026100000",
              "module": "C1"
            },
            {
              "value": "0.000010300000",
              "module": "C2"
            },
            {
              "value": "0.002460000000",
              "module": "C3"
            },
            {
              "value": "0.116000000000",
              "module": "C4"
            },
            {
              "value": "-0.000849000000",
              "module": "D"
            },
            {
              "name": "referenceToUnitGroupDataSet",
              "value": {
                "shortDescription": [
                  {
                    "value": "kg"
                  }
                ],
                "type": "unit group data set",
                "refObjectId": "ad38d542-3fe9-439d-9b95-2f5f7752acaf",
                "uri": "../unitgroups/ad38d542-3fe9-439d-9b95-2f5f7752acaf"
              }
            }
          ]
        },
        "flowProperties": [],
        "typeOfFlow": "Other flow",
        "classification": {
          "classHierarchy": "Gr\u00f6\u00dfen / Umweltliche Gr\u00f6\u00dfen / EPD EN 15804 / LCI Indikatoren",
          "name": "GaBiCategories"
        }
      },
      {
        "dataSetInternalID": 14,
        "referenceToFlowDataSet": {
          "shortDescription": [
            {
              "value": "Radioactive waste disposed (RWD)",
              "lang": "en"
            },
            {
              "value": "Avhendet radioaktivt avfall (RW)",
              "lang": "no"
            }
          ],
          "type": "flow data set",
          "refObjectId": "3449546e-52ad-4b39-b809-9fb77cea8ff6",
          "version": "30.00.000"
        },
        "exchange direction": "OUTPUT",
        "meanAmount": 0.0,
        "resultingAmount": 0.0,
        "minimumAmount": 0.0,
        "maximumAmount": 0.0,
        "uncertaintyDistributionType": "UNDEFINED",
        "relativeStandardDeviation95In": "0",
        "dataSourceType": "Primary",
        "dataDerivationTypeStatus": "MEASURED",
        "other": {
          "anies": [
            {
              "value": "0.000305000000",
              "module": "A1"
            },
            {
              "value": "0.000000251000",
              "module": "A2"
            },
            {
              "value": "0.000000304000",
              "module": "A3"
            },
            {
              "value": "0.000000534000",
              "module": "A4"
            },
            {
              "value": "0.000025700000",
              "module": "A5"
            },
            {
              "value": "0.000000000000",
              "module": "B1"
            },
            {
              "value": "0.000000000000",
              "module": "B2"
            },
            {
              "value": "0.000000000000",
              "module": "B3"
            },
            {
              "value": "0.000000000000",
              "module": "B4"
            },
            {
              "value": "0.000000000000",
              "module": "B5"
            },
            {
              "value": "0.000000000000",
              "module": "B6"
            },
            {
              "value": "0.000000000000",
              "module": "B7"
            },
            {
              "value": "0.000005480000",
              "module": "C1"
            },
            {
              "value": "0.000000083700",
              "module": "C2"
            },
            {
              "value": "0.000014600000",
              "module": "C3"
            },
            {
              "value": "0.000001410000",
              "module": "C4"
            },
            {
              "value": "-0.000069000000",
              "module": "D"
            },
            {
              "name": "referenceToUnitGroupDataSet",
              "value": {
                "shortDescription": [
                  {
                    "value": "kg"
                  }
                ],
                "type": "unit group data set",
                "refObjectId": "ad38d542-3fe9-439d-9b95-2f5f7752acaf",
                "uri": "../unitgroups/ad38d542-3fe9-439d-9b95-2f5f7752acaf"
              }
            }
          ]
        },
        "flowProperties": [],
        "typeOfFlow": "Other flow",
        "classification": {
          "classHierarchy": "Gr\u00f6\u00dfen / Umweltliche Gr\u00f6\u00dfen / EPD EN 15804 / LCI Indikatoren",
          "name": "GaBiCategories"
        }
      },
      {
        "dataSetInternalID": 15,
        "referenceToFlowDataSet": {
          "shortDescription": [
            {
              "value": "Components for re-use (CRU)",
              "lang": "en"
            },
            {
              "value": "Komponenter for gjenbruk (CR)",
              "lang": "no"
            }
          ],
          "type": "flow data set",
          "refObjectId": "a2b32f97-3fc7-4af2-b209-525bc6426f33",
          "version": "30.00.000"
        },
        "exchange direction": "OUTPUT",
        "meanAmount": 0.0,
        "resultingAmount": 0.0,
        "minimumAmount": 0.0,
        "maximumAmount": 0.0,
        "uncertaintyDistributionType": "UNDEFINED",
        "relativeStandardDeviation95In": "0",
        "dataSourceType": "Primary",
        "dataDerivationTypeStatus": "MEASURED",
        "other": {
          "anies": [
            {
              "value": "0.000000000000",
              "module": "A1"
            },
            {
              "value": "0.000000000000",
              "module": "A2"
            },
            {
              "value": "0.000000000000",
              "module": "A3"
            },
            {
              "value": "0.000000000000",
              "module": "A4"
            },
            {
              "value": "0.000000000000",
              "module": "A5"
            },
            {
              "value": "0.000000000000",
              "module": "B1"
            },
            {
              "value": "0.000000000000",
              "module": "B2"
            },
            {
              "value": "0.000000000000",
              "module": "B3"
            },
            {
              "value": "0.000000000000",
              "module": "B4"
            },
            {
              "value": "0.000000000000",
              "module": "B5"
            },
            {
              "value": "0.000000000000",
              "module": "B6"
            },
            {
              "value": "0.000000000000",
              "module": "B7"
            },
            {
              "value": "0.000000000000",
              "module": "C1"
            },
            {
              "value": "0.000000000000",
              "module": "C2"
            },
            {
              "value": "0.000000000000",
              "module": "C3"
            },
            {
              "value": "0.000000000000",
              "module": "C4"
            },
            {
              "value": "0.000000000000",
              "module": "D"
            },
            {
              "name": "referenceToUnitGroupDataSet",
              "value": {
                "shortDescription": [
                  {
                    "value": "kg"
                  }
                ],
                "type": "unit group data set",
                "refObjectId": "ad38d542-3fe9-439d-9b95-2f5f7752acaf",
                "uri": "../unitgroups/ad38d542-3fe9-439d-9b95-2f5f7752acaf"
              }
            }
          ]
        },
        "flowProperties": [],
        "typeOfFlow": "Other flow",
        "classification": {
          "classHierarchy": "Gr\u00f6\u00dfen / Umweltliche Gr\u00f6\u00dfen / EPD EN 15804 / LCI Indikatoren",
          "name": "GaBiCategories"
        }
      },
      {
        "dataSetInternalID": 16,
        "referenceToFlowDataSet": {
          "shortDescription": [
            {
              "value": "Materials for recycling (MFR)",
              "lang": "en"
            },
            {
              "value": "Materialer for resirkulering (MR)",
              "lang": "no"
            }
          ],
          "type": "flow data set",
          "refObjectId": "d7fe48a5-4103-49c8-9aae-b0b5dfdbd6ae",
          "version": "30.00.000"
        },
        "exchange direction": "OUTPUT",
        "meanAmount": 0.0,
        "resultingAmount": 0.0,
        "minimumAmount": 0.0,
        "maximumAmount": 0.0,
        "uncertaintyDistributionType": "UNDEFINED",
        "relativeStandardDeviation95In": "0",
        "dataSourceType": "Primary",
        "dataDerivationTypeStatus": "MEASURED",
        "other": {
          "anies": [
            {
              "value": "0.000000000000",
              "module": "A1"
            },
            {
              "value": "0.000000000000",
              "module": "A2"
            },
            {
              "value": "0.000000000000",
              "module": "A3"
            },
            {
              "value": "0.000000000000",
              "module": "A4"
            },
            {
              "value": "0.001450000000",
              "module": "A5"
            },
            {
              "value": "0.000000000000",
              "module": "B1"
            },
            {
              "value": "0.000000000000",
              "module": "B2"
            },
            {
              "value": "0.000000000000",
              "module": "B3"
            },
            {
              "value": "0.000000000000",
              "module": "B4"
            },
            {
              "value": "0.000000000000",
              "module": "B5"
            },
            {
              "value": "0.000000000000",
              "module": "B6"
            },
            {
              "value": "0.000000000000",
              "module": "B7"
            },
            {
              "value": "0.000000000000",
              "module": "C1"
            },
            {
              "value": "0.000000000000",
              "module": "C2"
            },
            {
              "value": "0.031600000000",
              "module": "C3"
            },
            {
              "value": "0.000000000000",
              "module": "C4"
            },
            {
              "value": "0.000000000000",
              "module": "D"
            },
            {
              "name": "referenceToUnitGroupDataSet",
              "value": {
                "shortDescription": [
                  {
                    "value": "kg"
                  }
                ],
                "type": "unit group data set",
                "refObjectId": "ad38d542-3fe9-439d-9b95-2f5f7752acaf",
                "uri": "../unitgroups/ad38d542-3fe9-439d-9b95-2f5f7752acaf"
              }
            }
          ]
        },
        "flowProperties": [],
        "typeOfFlow": "Other flow",
        "classification": {
          "classHierarchy": "Gr\u00f6\u00dfen / Umweltliche Gr\u00f6\u00dfen / EPD EN 15804 / LCI Indikatoren",
          "name": "GaBiCategories"
        }
      },
      {
        "dataSetInternalID": 17,
        "referenceToFlowDataSet": {
          "shortDescription": [
            {
              "value": "Materials for energy recovery (MER)",
              "lang": "en"
            },
            {
              "value": "Materialer for energigjenvinning (MER)",
              "lang": "no"
            }
          ],
          "type": "flow data set",
          "refObjectId": "59a9181c-3aaf-46ee-8b13-2b3723b6e447",
          "version": "30.00.000"
        },
        "exchange direction": "OUTPUT",
        "meanAmount": 0.0,
        "resultingAmount": 0.0,
        "minimumAmount": 0.0,
        "maximumAmount": 0.0,
        "uncertaintyDistributionType": "UNDEFINED",
        "relativeStandardDeviation95In": "0",
        "dataSourceType": "Primary",
        "dataDerivationTypeStatus": "MEASURED",
        "other": {
          "anies": [
            {
              "value": "0.000000000000",
              "module": "A1"
            },
            {
              "value": "0.000000000000",
              "module": "A2"
            },
            {
              "value": "0.000000000000",
              "module": "A3"
            },
            {
              "value": "0.000000000000",
              "module": "A4"
            },
            {
              "value": "0.000000000000",
              "module": "A5"
            },
            {
              "value": "0.000000000000",
              "module": "B1"
            },
            {
              "value": "0.000000000000",
              "module": "B2"
            },
            {
              "value": "0.000000000000",
              "module": "B3"
            },
            {
              "value": "0.000000000000",
              "module": "B4"
            },
            {
              "value": "0.000000000000",
              "module": "B5"
            },
            {
              "value": "0.000000000000",
              "module": "B6"
            },
            {
              "value": "0.000000000000",
              "module": "B7"
            },
            {
              "value": "0.000000000000",
              "module": "C1"
            },
            {
              "value": "0.000000000000",
              "module": "C2"
            },
            {
              "value": "0.000000000000",
              "module": "C3"
            },
            {
              "value": "0.000000000000",
              "module": "C4"
            },
            {
              "value": "0.000000000000",
              "module": "D"
            },
            {
              "name": "referenceToUnitGroupDataSet",
              "value": {
                "shortDescription": [
                  {
                    "value": "kg"
                  }
                ],
                "type": "unit group data set",
                "refObjectId": "ad38d542-3fe9-439d-9b95-2f5f7752acaf",
                "uri": "../unitgroups/ad38d542-3fe9-439d-9b95-2f5f7752acaf"
              }
            }
          ]
        },
        "flowProperties": [],
        "typeOfFlow": "Other flow",
        "classification": {
          "classHierarchy": "Gr\u00f6\u00dfen / Umweltliche Gr\u00f6\u00dfen / EPD EN 15804 / LCI Indikatoren",
          "name": "GaBiCategories"
        }
      },
      {
        "dataSetInternalID": 18,
        "referenceToFlowDataSet": {
          "shortDescription": [
            {
              "value": "Exported electrical energy (EEE)",
              "lang": "en"
            },
            {
              "value": "Eksportert elektrisk energi(EEE)",
              "lang": "no"
            }
          ],
          "type": "flow data set",
          "refObjectId": "4da0c987-2b76-40d6-9e9e-82a017aaaf29",
          "version": "30.00.000"
        },
        "exchange direction": "OUTPUT",
        "meanAmount": 0.0,
        "resultingAmount": 0.0,
        "minimumAmount": 0.0,
        "maximumAmount": 0.0,
        "uncertaintyDistributionType": "UNDEFINED",
        "relativeStandardDeviation95In": "0",
        "dataSourceType": "Primary",
        "dataDerivationTypeStatus": "MEASURED",
        "other": {
          "anies": [
            {
              "value": "0.000000000000",
              "module": "A1"
            },
            {
              "value": "0.000000000000",
              "module": "A2"
            },
            {
              "value": "0.000000000000",
              "module": "A3"
            },
            {
              "value": "0.000000000000",
              "module": "A4"
            },
            {
              "value": "0.021200000000",
              "module": "A5"
            },
            {
              "value": "0.000000000000",
              "module": "B1"
            },
            {
              "value": "0.000000000000",
              "module": "B2"
            },
            {
              "value": "0.000000000000",
              "module": "B3"
            },
            {
              "value": "0.000000000000",
              "module": "B4"
            },
            {
              "value": "0.000000000000",
              "module": "B5"
            },
            {
              "value": "0.000000000000",
              "module": "B6"
            },
            {
              "value": "0.000000000000",
              "module": "B7"
            },
            {
              "value": "0.000000000000",
              "module": "C1"
            },
            {
              "value": "0.000000000000",
              "module": "C2"
            },
            {
              "value": "0.154000000000",
              "module": "C3"
            },
            {
              "value": "0.000000000000",
              "module": "C4"
            },
            {
              "value": "0.000000000000",
              "module": "D"
            },
            {
              "name": "referenceToUnitGroupDataSet",
              "value": {
                "shortDescription": [
                  {
                    "value": "MJ"
                  }
                ],
                "type": "unit group data set",
                "refObjectId": "93a60a57-a3c8-11da-a746-0800200c9a66",
                "uri": "../unitgroups/93a60a57-a3c8-11da-a746-0800200c9a66"
              }
            }
          ]
        },
        "flowProperties": [],
        "typeOfFlow": "Other flow",
        "classification": {
          "classHierarchy": "Gr\u00f6\u00dfen / Umweltliche Gr\u00f6\u00dfen / EPD EN 15804 / LCI Indikatoren",
          "name": "GaBiCategories"
        }
      },
      {
        "dataSetInternalID": 19,
        "referenceToFlowDataSet": {
          "shortDescription": [
            {
              "value": "Exported thermal energy (EET)",
              "lang": "en"
            },
            {
              "value": "Eksportert termisk energi (ETE)",
              "lang": "no"
            }
          ],
          "type": "flow data set",
          "refObjectId": "98daf38a-7a79-46d3-9a37-2b7bd0955810",
          "version": "30.00.000"
        },
        "exchange direction": "OUTPUT",
        "meanAmount": 0.0,
        "resultingAmount": 0.0,
        "minimumAmount": 0.0,
        "maximumAmount": 0.0,
        "uncertaintyDistributionType": "UNDEFINED",
        "relativeStandardDeviation95In": "0",
        "dataSourceType": "Primary",
        "dataDerivationTypeStatus": "MEASURED",
        "other": {
          "anies": [
            {
              "value": "0.000000000000",
              "module": "A1"
            },
            {
              "value": "0.000000000000",
              "module": "A2"
            },
            {
              "value": "0.000000000000",
              "module": "A3"
            },
            {
              "value": "0.000000000000",
              "module": "A4"
            },
            {
              "value": "0.032300000000",
              "module": "A5"
            },
            {
              "value": "0.000000000000",
              "module": "B1"
            },
            {
              "value": "0.000000000000",
              "module": "B2"
            },
            {
              "value": "0.000000000000",
              "module": "B3"
            },
            {
              "value": "0.000000000000",
              "module": "B4"
            },
            {
              "value": "0.000000000000",
              "module": "B5"
            },
            {
              "value": "0.000000000000",
              "module": "B6"
            },
            {
              "value": "0.000000000000",
              "module": "B7"
            },
            {
              "value": "0.000000000000",
              "module": "C1"
            },
            {
              "value": "0.000000000000",
              "module": "C2"
            },
            {
              "value": "0.263000000000",
              "module": "C3"
            },
            {
              "value": "0.000000000000",
              "module": "C4"
            },
            {
              "value": "0.000000000000",
              "module": "D"
            },
            {
              "name": "referenceToUnitGroupDataSet",
              "value": {
                "shortDescription": [
                  {
                    "value": "MJ"
                  }
                ],
                "type": "unit group data set",
                "refObjectId": "93a60a57-a3c8-11da-a746-0800200c9a66",
                "uri": "../unitgroups/93a60a57-a3c8-11da-a746-0800200c9a66"
              }
            }
          ]
        },
        "flowProperties": [],
        "typeOfFlow": "Other flow",
        "classification": {
          "classHierarchy": "Gr\u00f6\u00dfen / Umweltliche Gr\u00f6\u00dfen / EPD EN 15804 / LCI Indikatoren",
          "name": "GaBiCategories"
        }
      }
    ]
  },
  "LCIAResults": {
    "LCIAResult": [
      {
        "referenceToLCIAMethodDataSet": {
          "shortDescription": [
            {
              "value": "Acidification potential, Accumulated Exceedance (AP)",
              "lang": "en"
            },
            {
              "value": "Forsurningspotensial for kilder p\u00e5 land og vann (AP)",
              "lang": "no"
            }
          ],
          "type": "LCIA method data set",
          "refObjectId": "b5c611c6-def3-11e6-bf01-fe55135034f3",
          "version": "00.01.000"
        },
        "meanAmount": 0.0,
        "uncertaintyDistributionType": "undefined",
        "relativeStandardDeviation95In": 0,
        "other": {
          "anies": [
            {
              "value": "0.001210000000",
              "module": "A1"
            },
            {
              "value": "0.000033400000",
              "module": "A2"
            },
            {
              "value": "0.000003190000",
              "module": "A3"
            },
            {
              "value": "0.000259000000",
              "module": "A4"
            },
            {
              "value": "0.000129000000",
              "module": "A5"
            },
            {
              "value": "0.000000000000",
              "module": "B1"
            },
            {
              "value": "0.000000000000",
              "module": "B2"
            },
            {
              "value": "0.000000000000",
              "module": "B3"
            },
            {
              "value": "0.000000000000",
              "module": "B4"
            },
            {
              "value": "0.000000000000",
              "module": "B5"
            },
            {
              "value": "0.000000000000",
              "module": "B6"
            },
            {
              "value": "0.000000000000",
              "module": "B7"
            },
            {
              "value": "0.000004300000",
              "module": "C1"
            },
            {
              "value": "0.000014700000",
              "module": "C2"
            },
            {
              "value": "0.000025300000",
              "module": "C3"
            },
            {
              "value": "0.000027400000",
              "module": "C4"
            },
            {
              "value": "-0.000162000000",
              "module": "D"
            },
            {
              "name": "referenceToUnitGroupDataSet",
              "value": {
                "shortDescription": [
                  {
                    "value": "mol H+ eqv."
                  }
                ],
                "type": "unit group data set",
                "refObjectId": "42e089ac-92bf-4bf2-8ca1-5fc40d18f2ed",
                "uri": "../unitgroups/42e089ac-92bf-4bf2-8ca1-5fc40d18f2ed"
              }
            }
          ]
        }
      },
      {
        "referenceToLCIAMethodDataSet": {
          "shortDescription": [
            {
              "value": "Global Warming Potential - total (GWP-total)",
              "lang": "en"
            },
            {
              "value": "Globalt oppvarmingspotensial -totalt (GWPtotal)",
              "lang": "no"
            }
          ],
          "type": "LCIA method data set",
          "refObjectId": "6a37f984-a4b3-458a-a20a-64418c145fa2",
          "version": "00.02.000"
        },
        "meanAmount": 0.0,
        "uncertaintyDistributionType": "undefined",
        "relativeStandardDeviation95In": 0,
        "other": {
          "anies": [
            {
              "value": "0.612000000000",
              "module": "A1"
            },
            {
              "value": "0.010400000000",
              "module": "A2"
            },
            {
              "value": "0.001640000000",
              "module": "A3"
            },
            {
              "value": "0.024400000000",
              "module": "A4"
            },
            {
              "value": "0.084100000000",
              "module": "A5"
            },
            {
              "value": "0.000000000000",
              "module": "B1"
            },
            {
              "value": "0.000000000000",
              "module": "B2"
            },
            {
              "value": "0.000000000000",
              "module": "B3"
            },
            {
              "value": "0.000000000000",
              "module": "B4"
            },
            {
              "value": "0.000000000000",
              "module": "B5"
            },
            {
              "value": "0.000000000000",
              "module": "B6"
            },
            {
              "value": "0.000000000000",
              "module": "B7"
            },
            {
              "value": "0.002090000000",
              "module": "C1"
            },
            {
              "value": "0.005220000000",
              "module": "C2"
            },
            {
              "value": "0.098900000000",
              "module": "C3"
            },
            {
              "value": "0.009530000000",
              "module": "C4"
            },
            {
              "value": "-0.108000000000",
              "module": "D"
            },
            {
              "name": "referenceToUnitGroupDataSet",
              "value": {
                "shortDescription": [
                  {
                    "value": "kg CO2 eqv."
                  }
                ],
                "type": "unit group data set",
                "refObjectId": "1ebf3012-d0db-4de2-aefd-ef30cedb0be1",
                "uri": "../unitgroups/1ebf3012-d0db-4de2-aefd-ef30cedb0be1"
              }
            }
          ]
        }
      },
      {
        "referenceToLCIAMethodDataSet": {
          "shortDescription": [
            {
              "value": "Global Warming Potential - biogenic (GWP-biogenic)",
              "lang": "en"
            },
            {
              "value": "Globalt oppvarmingspotensial - biogene kilder( GWP-biogenic)",
              "lang": "no"
            }
          ],
          "type": "LCIA method data set",
          "refObjectId": "2356e1ab-0185-4db5-86e5-16de51c7485c",
          "version": "00.02.000"
        },
        "meanAmount": 0.0,
        "uncertaintyDistributionType": "undefined",
        "relativeStandardDeviation95In": 0,
        "other": {
          "anies": [
            {
              "value": "-0.009140000000",
              "module": "A1"
            },
            {
              "value": "0.000000000000",
              "module": "A2"
            },
            {
              "value": "0.000024800000",
              "module": "A3"
            },
            {
              "value": "0.000000000000",
              "module": "A4"
            },
            {
              "value": "0.011900000000",
              "module": "A5"
            },
            {
              "value": "0.000000000000",
              "module": "B1"
            },
            {
              "value": "0.000000000000",
              "module": "B2"
            },
            {
              "value": "0.000000000000",
              "module": "B3"
            },
            {
              "value": "0.000000000000",
              "module": "B4"
            },
            {
              "value": "0.000000000000",
              "module": "B5"
            },
            {
              "value": "0.000000000000",
              "module": "B6"
            },
            {
              "value": "0.000000000000",
              "module": "B7"
            },
            {
              "value": "0.000017600000",
              "module": "C1"
            },
            {
              "value": "0.000000000000",
              "module": "C2"
            },
            {
              "value": "0.000115000000",
              "module": "C3"
            },
            {
              "value": "-0.000076500000",
              "module": "C4"
            },
            {
              "value": "-0.000530000000",
              "module": "D"
            },
            {
              "name": "referenceToUnitGroupDataSet",
              "value": {
                "shortDescription": [
                  {
                    "value": "kg CO2 eqv."
                  }
                ],
                "type": "unit group data set",
                "refObjectId": "1ebf3012-d0db-4de2-aefd-ef30cedb0be1",
                "uri": "../unitgroups/1ebf3012-d0db-4de2-aefd-ef30cedb0be1"
              }
            }
          ]
        }
      },
      {
        "referenceToLCIAMethodDataSet": {
          "shortDescription": [
            {
              "value": "Global Warming Potential - fossil fuels (GWP-fossil)",
              "lang": "en"
            },
            {
              "value": "Globalt oppvarmingspotensial - fossile brensler (GWP-fossil)",
              "lang": "no"
            }
          ],
          "type": "LCIA method data set",
          "refObjectId": "5f635281-343e-44fb-83df-1971b155e6b6",
          "version": "00.01.000"
        },
        "meanAmount": 0.0,
        "uncertaintyDistributionType": "undefined",
        "relativeStandardDeviation95In": 0,
        "other": {
          "anies": [
            {
              "value": "0.621000000000",
              "module": "A1"
            },
            {
              "value": "0.010400000000",
              "module": "A2"
            },
            {
              "value": "0.001610000000",
              "module": "A3"
            },
            {
              "value": "0.024300000000",
              "module": "A4"
            },
            {
              "value": "0.072200000000",
              "module": "A5"
            },
            {
              "value": "0.000000000000",
              "module": "B1"
            },
            {
              "value": "0.000000000000",
              "module": "B2"
            },
            {
              "value": "0.000000000000",
              "module": "B3"
            },
            {
              "value": "0.000000000000",
              "module": "B4"
            },
            {
              "value": "0.000000000000",
              "module": "B5"
            },
            {
              "value": "0.000000000000",
              "module": "B6"
            },
            {
              "value": "0.000000000000",
              "module": "B7"
            },
            {
              "value": "0.002070000000",
              "module": "C1"
            },
            {
              "value": "0.005180000000",
              "module": "C2"
            },
            {
              "value": "0.098800000000",
              "module": "C3"
            },
            {
              "value": "0.009600000000",
              "module": "C4"
            },
            {
              "value": "-0.108000000000",
              "module": "D"
            },
            {
              "name": "referenceToUnitGroupDataSet",
              "value": {
                "shortDescription": [
                  {
                    "value": "kg CO2 eqv."
                  }
                ],
                "type": "unit group data set",
                "refObjectId": "1ebf3012-d0db-4de2-aefd-ef30cedb0be1",
                "uri": "../unitgroups/1ebf3012-d0db-4de2-aefd-ef30cedb0be1"
              }
            }
          ]
        }
      },
      {
        "referenceToLCIAMethodDataSet": {
          "shortDescription": [
            {
              "value": "Global Warming Potential - land use and land use change (GWP-luluc)",
              "lang": "en"
            },
            {
              "value": "Globalt oppvarmingspotensial arealbruk endringer i bruk av arealer (GWP-luluc)",
              "lang": "no"
            }
          ],
          "type": "LCIA method data set",
          "refObjectId": "4331bbdb-978a-490d-8707-eeb047f01a55",
          "version": "00.02.000"
        },
        "meanAmount": 0.0,
        "uncertaintyDistributionType": "undefined",
        "relativeStandardDeviation95In": 0,
        "other": {
          "anies": [
            {
              "value": "0.000352000000",
              "module": "A1"
            },
            {
              "value": "0.000084500000",
              "module": "A2"
            },
            {
              "value": "0.000000861000",
              "module": "A3"
            },
            {
              "value": "0.000157000000",
              "module": "A4"
            },
            {
              "value": "0.000047000000",
              "module": "A5"
            },
            {
              "value": "0.000000000000",
              "module": "B1"
            },
            {
              "value": "0.000000000000",
              "module": "B2"
            },
            {
              "value": "0.000000000000",
              "module": "B3"
            },
            {
              "value": "0.000000000000",
              "module": "B4"
            },
            {
              "value": "0.000000000000",
              "module": "B5"
            },
            {
              "value": "0.000000000000",
              "module": "B6"
            },
            {
              "value": "0.000000000000",
              "module": "B7"
            },
            {
              "value": "0.000002930000",
              "module": "C1"
            },
            {
              "value": "0.000042500000",
              "module": "C2"
            },
            {
              "value": "0.000008670000",
              "module": "C3"
            },
            {
              "value": "0.000007080000",
              "module": "C4"
            },
            {
              "value": "-0.000052400000",
              "module": "D"
            },
            {
              "name": "referenceToUnitGroupDataSet",
              "value": {
                "shortDescription": [
                  {
                    "value": "kg CO2 eqv."
                  }
                ],
                "type": "unit group data set",
                "refObjectId": "1ebf3012-d0db-4de2-aefd-ef30cedb0be1",
                "uri": "../unitgroups/1ebf3012-d0db-4de2-aefd-ef30cedb0be1"
              }
            }
          ]
        }
      },
      {
        "referenceToLCIAMethodDataSet": {
          "shortDescription": [
            {
              "value": "Potential Comparative Toxic Unit for ecosystems (ETP-fw)",
              "lang": "en"
            },
            {
              "value": "\u00d8kotoksisitet, ferskvann (ETP-fw)",
              "lang": "no"
            }
          ],
          "type": "LCIA method data set",
          "refObjectId": "ee1082d1-b0f7-43ca-a1f0-21e2a4a74511",
          "version": "00.01.000"
        },
        "meanAmount": 0.0,
        "uncertaintyDistributionType": "undefined",
        "relativeStandardDeviation95In": 0,
        "other": {
          "anies": [
            {
              "value": "0.000000000000",
              "module": "A1"
            },
            {
              "value": "0.000000000000",
              "module": "A2"
            },
            {
              "value": "0.000000000000",
              "module": "A3"
            },
            {
              "value": "0.000000000000",
              "module": "A4"
            },
            {
              "value": "0.000000000000",
              "module": "A5"
            },
            {
              "value": "0.000000000000",
              "module": "B1"
            },
            {
              "value": "0.000000000000",
              "module": "B2"
            },
            {
              "value": "0.000000000000",
              "module": "B3"
            },
            {
              "value": "0.000000000000",
              "module": "B4"
            },
            {
              "value": "0.000000000000",
              "module": "B5"
            },
            {
              "value": "0.000000000000",
              "module": "B6"
            },
            {
              "value": "0.000000000000",
              "module": "B7"
            },
            {
              "value": "0.000000000000",
              "module": "C1"
            },
            {
              "value": "0.000000000000",
              "module": "C2"
            },
            {
              "value": "0.000000000000",
              "module": "C3"
            },
            {
              "value": "0.000000000000",
              "module": "C4"
            },
            {
              "value": "0.000000000000",
              "module": "D"
            },
            {
              "name": "referenceToUnitGroupDataSet",
              "value": {
                "shortDescription": [
                  {
                    "value": "CTUe"
                  }
                ],
                "type": "unit group data set",
                "refObjectId": "aa959ded-f1eb-4efb-9c5c-2d60be36b3e6",
                "uri": "../unitgroups/aa959ded-f1eb-4efb-9c5c-2d60be36b3e6"
              }
            }
          ]
        }
      },
      {
        "referenceToLCIAMethodDataSet": {
          "shortDescription": [
            {
              "value": "Potential incidence of disease due to PM emissions (PM)",
              "lang": "en"
            },
            {
              "value": "Partikkelutslipp (PM)",
              "lang": "no"
            }
          ],
          "type": "LCIA method data set",
          "refObjectId": "b5c602c6-def3-11e6-bf01-fe55135034f3",
          "version": "00.01.000"
        },
        "meanAmount": 0.0,
        "uncertaintyDistributionType": "undefined",
        "relativeStandardDeviation95In": 0,
        "other": {
          "anies": [
            {
              "value": "0.000000000000",
              "module": "A1"
            },
            {
              "value": "0.000000000000",
              "module": "A2"
            },
            {
              "value": "0.000000000000",
              "module": "A3"
            },
            {
              "value": "0.000000000000",
              "module": "A4"
            },
            {
              "value": "0.000000000000",
              "module": "A5"
            },
            {
              "value": "0.000000000000",
              "module": "B1"
            },
            {
              "value": "0.000000000000",
              "module": "B2"
            },
            {
              "value": "0.000000000000",
              "module": "B3"
            },
            {
              "value": "0.000000000000",
              "module": "B4"
            },
            {
              "value": "0.000000000000",
              "module": "B5"
            },
            {
              "value": "0.000000000000",
              "module": "B6"
            },
            {
              "value": "0.000000000000",
              "module": "B7"
            },
            {
              "value": "0.000000000000",
              "module": "C1"
            },
            {
              "value": "0.000000000000",
              "module": "C2"
            },
            {
              "value": "0.000000000000",
              "module": "C3"
            },
            {
              "value": "0.000000000000",
              "module": "C4"
            },
            {
              "value": "0.000000000000",
              "module": "D"
            },
            {
              "name": "referenceToUnitGroupDataSet",
              "value": {
                "shortDescription": [
                  {
                    "value": "disease incidence"
                  }
                ],
                "type": "unit group data set",
                "refObjectId": "3883559b-648f-4afc-8ba2-0bd24f3affa3",
                "uri": "../unitgroups/3883559b-648f-4afc-8ba2-0bd24f3affa3"
              }
            }
          ]
        }
      },
      {
        "referenceToLCIAMethodDataSet": {
          "shortDescription": [
            {
              "value": "Eutrophication potential - marine (EP-marine)",
              "lang": "en"
            },
            {
              "value": "Overgj\u00f8dslingspotensial til hav (EP-marine), hav og jord",
              "lang": "no"
            }
          ],
          "type": "LCIA method data set",
          "refObjectId": "b5c619fa-def3-11e6-bf01-fe55135034f3",
          "version": "00.01.000"
        },
        "meanAmount": 0.0,
        "uncertaintyDistributionType": "undefined",
        "relativeStandardDeviation95In": 0,
        "other": {
          "anies": [
            {
              "value": "0.000283000000",
              "module": "A1"
            },
            {
              "value": "0.000015300000",
              "module": "A2"
            },
            {
              "value": "0.000000916000",
              "module": "A3"
            },
            {
              "value": "0.000079500000",
              "module": "A4"
            },
            {
              "value": "0.000031800000",
              "module": "A5"
            },
            {
              "value": "0.000000000000",
              "module": "B1"
            },
            {
              "value": "0.000000000000",
              "module": "B2"
            },
            {
              "value": "0.000000000000",
              "module": "B3"
            },
            {
              "value": "0.000000000000",
              "module": "B4"
            },
            {
              "value": "0.000000000000",
              "module": "B5"
            },
            {
              "value": "0.000000000000",
              "module": "B6"
            },
            {
              "value": "0.000000000000",
              "module": "B7"
            },
            {
              "value": "0.000001020000",
              "module": "C1"
            },
            {
              "value": "0.000006620000",
              "module": "C2"
            },
            {
              "value": "0.000007250000",
              "module": "C3"
            },
            {
              "value": "0.000009890000",
              "module": "C4"
            },
            {
              "value": "-0.000043300000",
              "module": "D"
            },
            {
              "name": "referenceToUnitGroupDataSet",
              "value": {
                "shortDescription": [
                  {
                    "value": "kg N eqv."
                  }
                ],
                "type": "unit group data set",
                "refObjectId": "d05bb823-ecdf-4686-8c40-bf1d9257859f",
                "uri": "../unitgroups/d05bb823-ecdf-4686-8c40-bf1d9257859f"
              }
            }
          ]
        }
      },
      {
        "referenceToLCIAMethodDataSet": {
          "shortDescription": [
            {
              "value": "Eutrophication potential - freshwater (EP-freshwater)",
              "lang": "en"
            },
            {
              "value": "Overgj\u00f8dslingspotensial til ferskvann (EP-freshwater)",
              "lang": "no"
            }
          ],
          "type": "LCIA method data set",
          "refObjectId": "b53ec18f-7377-4ad3-86eb-cc3f4f276b2b",
          "version": "00.01.000"
        },
        "meanAmount": 0.0,
        "uncertaintyDistributionType": "undefined",
        "relativeStandardDeviation95In": 0,
        "other": {
          "anies": [
            {
              "value": "0.000001050000",
              "module": "A1"
            },
            {
              "value": "0.000000030700",
              "module": "A2"
            },
            {
              "value": "0.000000004870",
              "module": "A3"
            },
            {
              "value": "0.000000058200",
              "module": "A4"
            },
            {
              "value": "0.000000363000",
              "module": "A5"
            },
            {
              "value": "0.000000000000",
              "module": "B1"
            },
            {
              "value": "0.000000000000",
              "module": "B2"
            },
            {
              "value": "0.000000000000",
              "module": "B3"
            },
            {
              "value": "0.000000000000",
              "module": "B4"
            },
            {
              "value": "0.000000000000",
              "module": "B5"
            },
            {
              "value": "0.000000000000",
              "module": "B6"
            },
            {
              "value": "0.000000000000",
              "module": "B7"
            },
            {
              "value": "0.000000005550",
              "module": "C1"
            },
            {
              "value": "0.000000015400",
              "module": "C2"
            },
            {
              "value": "0.000000087100",
              "module": "C3"
            },
            {
              "value": "0.000001760000",
              "module": "C4"
            },
            {
              "value": "-0.000000135000",
              "module": "D"
            },
            {
              "name": "referenceToUnitGroupDataSet",
              "value": {
                "shortDescription": [
                  {
                    "value": "kg P eqv."
                  }
                ],
                "type": "unit group data set",
                "refObjectId": "0429039d-a61d-4590-ba67-aa4a20a810a1",
                "uri": "../unitgroups/0429039d-a61d-4590-ba67-aa4a20a810a1"
              }
            }
          ]
        }
      },
      {
        "referenceToLCIAMethodDataSet": {
          "shortDescription": [
            {
              "value": "Eutrophication potential - terrestrial (EP-terrestrial)",
              "lang": "en"
            },
            {
              "value": "Overgj\u00f8dslingspotensial til jord (EP-terrestrial)",
              "lang": "no"
            }
          ],
          "type": "LCIA method data set",
          "refObjectId": "b5c614d2-def3-11e6-bf01-fe55135034f3",
          "version": "00.01.000"
        },
        "meanAmount": 0.0,
        "uncertaintyDistributionType": "undefined",
        "relativeStandardDeviation95In": 0,
        "other": {
          "anies": [
            {
              "value": "0.003090000000",
              "module": "A1"
            },
            {
              "value": "0.000170000000",
              "module": "A2"
            },
            {
              "value": "0.000009870000",
              "module": "A3"
            },
            {
              "value": "0.000878000000",
              "module": "A4"
            },
            {
              "value": "0.000344000000",
              "module": "A5"
            },
            {
              "value": "0.000000000000",
              "module": "B1"
            },
            {
              "value": "0.000000000000",
              "module": "B2"
            },
            {
              "value": "0.000000000000",
              "module": "B3"
            },
            {
              "value": "0.000000000000",
              "module": "B4"
            },
            {
              "value": "0.000000000000",
              "module": "B5"
            },
            {
              "value": "0.000000000000",
              "module": "B6"
            },
            {
              "value": "0.000000000000",
              "module": "B7"
            },
            {
              "value": "0.000010700000",
              "module": "C1"
            },
            {
              "value": "0.000074500000",
              "module": "C2"
            },
            {
              "value": "0.000094000000",
              "module": "C3"
            },
            {
              "value": "0.000074700000",
              "module": "C4"
            },
            {
              "value": "-0.000465000000",
              "module": "D"
            },
            {
              "name": "referenceToUnitGroupDataSet",
              "value": {
                "shortDescription": [
                  {
                    "value": "mol N eqv."
                  }
                ],
                "type": "unit group data set",
                "refObjectId": "71b4d617-0ec9-4d3f-b65e-e438940c2401",
                "uri": "../unitgroups/71b4d617-0ec9-4d3f-b65e-e438940c2401"
              }
            }
          ]
        }
      },
      {
        "referenceToLCIAMethodDataSet": {
          "shortDescription": [
            {
              "value": "Potential Comparative Toxic Unit for humans - cancer effects (HTP-c)",
              "lang": "en"
            },
            {
              "value": "Toksisitet p\u00e5virkning p\u00e5 mennesker, kreft (HTP-c)",
              "lang": "no"
            }
          ],
          "type": "LCIA method data set",
          "refObjectId": "2299222a-bbd8-474f-9d4f-4dd1f18aea7c",
          "version": "00.01.000"
        },
        "meanAmount": 0.0,
        "uncertaintyDistributionType": "undefined",
        "relativeStandardDeviation95In": 0,
        "other": {
          "anies": [
            {
              "value": "0.000000000000",
              "module": "A1"
            },
            {
              "value": "0.000000000000",
              "module": "A2"
            },
            {
              "value": "0.000000000000",
              "module": "A3"
            },
            {
              "value": "0.000000000000",
              "module": "A4"
            },
            {
              "value": "0.000000000000",
              "module": "A5"
            },
            {
              "value": "0.000000000000",
              "module": "B1"
            },
            {
              "value": "0.000000000000",
              "module": "B2"
            },
            {
              "value": "0.000000000000",
              "module": "B3"
            },
            {
              "value": "0.000000000000",
              "module": "B4"
            },
            {
              "value": "0.000000000000",
              "module": "B5"
            },
            {
              "value": "0.000000000000",
              "module": "B6"
            },
            {
              "value": "0.000000000000",
              "module": "B7"
            },
            {
              "value": "0.000000000000",
              "module": "C1"
            },
            {
              "value": "0.000000000000",
              "module": "C2"
            },
            {
              "value": "0.000000000000",
              "module": "C3"
            },
            {
              "value": "0.000000000000",
              "module": "C4"
            },
            {
              "value": "0.000000000000",
              "module": "D"
            },
            {
              "name": "referenceToUnitGroupDataSet",
              "value": {
                "shortDescription": [
                  {
                    "value": "CTUh"
                  }
                ],
                "type": "unit group data set",
                "refObjectId": "d4c9523e-2d7e-49fd-8469-998f547d3a70",
                "uri": "../unitgroups/d4c9523e-2d7e-49fd-8469-998f547d3a70"
              }
            }
          ]
        }
      },
      {
        "referenceToLCIAMethodDataSet": {
          "shortDescription": [
            {
              "value": "Potential Comparative Toxic Unit for humans - non-cancer effects (HTP-nc)",
              "lang": "en"
            },
            {
              "value": "Toksisitet p\u00e5virkning p\u00e5 mennesker, andre effekter enn kreft (HTP-nc) ",
              "lang": "no"
            }
          ],
          "type": "LCIA method data set",
          "refObjectId": "3af763a5-b7a1-48c9-9cee-1f223481fcef",
          "version": "00.01.000"
        },
        "meanAmount": 0.0,
        "uncertaintyDistributionType": "undefined",
        "relativeStandardDeviation95In": 0,
        "other": {
          "anies": [
            {
              "value": "0.000000000000",
              "module": "A1"
            },
            {
              "value": "0.000000000000",
              "module": "A2"
            },
            {
              "value": "0.000000000000",
              "module": "A3"
            },
            {
              "value": "0.000000000000",
              "module": "A4"
            },
            {
              "value": "0.000000000000",
              "module": "A5"
            },
            {
              "value": "0.000000000000",
              "module": "B1"
            },
            {
              "value": "0.000000000000",
              "module": "B2"
            },
            {
              "value": "0.000000000000",
              "module": "B3"
            },
            {
              "value": "0.000000000000",
              "module": "B4"
            },
            {
              "value": "0.000000000000",
              "module": "B5"
            },
            {
              "value": "0.000000000000",
              "module": "B6"
            },
            {
              "value": "0.000000000000",
              "module": "B7"
            },
            {
              "value": "0.000000000000",
              "module": "C1"
            },
            {
              "value": "0.000000000000",
              "module": "C2"
            },
            {
              "value": "0.000000000000",
              "module": "C3"
            },
            {
              "value": "0.000000000000",
              "module": "C4"
            },
            {
              "value": "0.000000000000",
              "module": "D"
            },
            {
              "name": "referenceToUnitGroupDataSet",
              "value": {
                "shortDescription": [
                  {
                    "value": "CTUh"
                  }
                ],
                "type": "unit group data set",
                "refObjectId": "d4c9523e-2d7e-49fd-8469-998f547d3a70",
                "uri": "../unitgroups/d4c9523e-2d7e-49fd-8469-998f547d3a70"
              }
            }
          ]
        }
      },
      {
        "referenceToLCIAMethodDataSet": {
          "shortDescription": [
            {
              "value": "Potential Human exposure efficiency relative to U235 (IRP)",
              "lang": "en"
            },
            {
              "value": "Ioniserende str\u00e5ling, helseeffekt (IRP)",
              "lang": "no"
            }
          ],
          "type": "LCIA method data set",
          "refObjectId": "b5c632be-def3-11e6-bf01-fe55135034f3",
          "version": "00.01.000"
        },
        "meanAmount": 0.0,
        "uncertaintyDistributionType": "undefined",
        "relativeStandardDeviation95In": 0,
        "other": {
          "anies": [
            {
              "value": "0.000000000000",
              "module": "A1"
            },
            {
              "value": "0.000000000000",
              "module": "A2"
            },
            {
              "value": "0.000000000000",
              "module": "A3"
            },
            {
              "value": "0.000000000000",
              "module": "A4"
            },
            {
              "value": "0.000000000000",
              "module": "A5"
            },
            {
              "value": "0.000000000000",
              "module": "B1"
            },
            {
              "value": "0.000000000000",
              "module": "B2"
            },
            {
              "value": "0.000000000000",
              "module": "B3"
            },
            {
              "value": "0.000000000000",
              "module": "B4"
            },
            {
              "value": "0.000000000000",
              "module": "B5"
            },
            {
              "value": "0.000000000000",
              "module": "B6"
            },
            {
              "value": "0.000000000000",
              "module": "B7"
            },
            {
              "value": "0.000000000000",
              "module": "C1"
            },
            {
              "value": "0.000000000000",
              "module": "C2"
            },
            {
              "value": "0.000000000000",
              "module": "C3"
            },
            {
              "value": "0.000000000000",
              "module": "C4"
            },
            {
              "value": "0.000000000000",
              "module": "D"
            },
            {
              "name": "referenceToUnitGroupDataSet",
              "value": {
                "shortDescription": [
                  {
                    "value": "kBq U235 eqv."
                  }
                ],
                "type": "unit group data set",
                "refObjectId": "456b05bf-1415-44a9-9993-02452f554c09",
                "uri": "../unitgroups/456b05bf-1415-44a9-9993-02452f554c09"
              }
            }
          ]
        }
      },
      {
        "referenceToLCIAMethodDataSet": {
          "shortDescription": [
            {
              "value": "Potential Soil quality index (SQP)",
              "lang": "en"
            },
            {
              "value": "P\u00e5virkninger knyttet til arealbruksendringer / jordkvalitet (SQP)",
              "lang": "no"
            }
          ],
          "type": "LCIA method data set",
          "refObjectId": "b2ad6890-c78d-11e6-9d9d-cec0c932ce01",
          "version": "00.01.000"
        },
        "meanAmount": 0.0,
        "uncertaintyDistributionType": "undefined",
        "relativeStandardDeviation95In": 0,
        "other": {
          "anies": [
            {
              "value": "0.000000000000",
              "module": "A1"
            },
            {
              "value": "0.000000000000",
              "module": "A2"
            },
            {
              "value": "0.000000000000",
              "module": "A3"
            },
            {
              "value": "0.000000000000",
              "module": "A4"
            },
            {
              "value": "0.000000000000",
              "module": "A5"
            },
            {
              "value": "0.000000000000",
              "module": "B1"
            },
            {
              "value": "0.000000000000",
              "module": "B2"
            },
            {
              "value": "0.000000000000",
              "module": "B3"
            },
            {
              "value": "0.000000000000",
              "module": "B4"
            },
            {
              "value": "0.000000000000",
              "module": "B5"
            },
            {
              "value": "0.000000000000",
              "module": "B6"
            },
            {
              "value": "0.000000000000",
              "module": "B7"
            },
            {
              "value": "0.000000000000",
              "module": "C1"
            },
            {
              "value": "0.000000000000",
              "module": "C2"
            },
            {
              "value": "0.000000000000",
              "module": "C3"
            },
            {
              "value": "0.000000000000",
              "module": "C4"
            },
            {
              "value": "0.000000000000",
              "module": "D"
            },
            {
              "name": "referenceToUnitGroupDataSet",
              "value": {
                "shortDescription": [
                  {
                    "value": "unitless"
                  }
                ],
                "type": "unit group data set",
                "refObjectId": "f130951c-e67f-4f7f-8dd4-665de3974e18",
                "uri": "../unitgroups/f130951c-e67f-4f7f-8dd4-665de3974e18"
              }
            }
          ]
        }
      },
      {
        "referenceToLCIAMethodDataSet": {
          "shortDescription": [
            {
              "value": "Depletion potential of the stratospheric ozone layer (ODP)",
              "lang": "en"
            },
            {
              "value": "Potensial for nedbryting av stratosf\u00e6risk ozon (ODP)",
              "lang": "no"
            }
          ],
          "type": "LCIA method data set",
          "refObjectId": "b5c629d6-def3-11e6-bf01-fe55135034f3",
          "version": "00.01.000"
        },
        "meanAmount": 0.0,
        "uncertaintyDistributionType": "undefined",
        "relativeStandardDeviation95In": 0,
        "other": {
          "anies": [
            {
              "value": "0.000000000000",
              "module": "A1"
            },
            {
              "value": "0.000000000000",
              "module": "A2"
            },
            {
              "value": "0.000000000000",
              "module": "A3"
            },
            {
              "value": "0.000000000000",
              "module": "A4"
            },
            {
              "value": "0.000000000000",
              "module": "A5"
            },
            {
              "value": "0.000000000000",
              "module": "B1"
            },
            {
              "value": "0.000000000000",
              "module": "B2"
            },
            {
              "value": "0.000000000000",
              "module": "B3"
            },
            {
              "value": "0.000000000000",
              "module": "B4"
            },
            {
              "value": "0.000000000000",
              "module": "B5"
            },
            {
              "value": "0.000000000000",
              "module": "B6"
            },
            {
              "value": "0.000000000000",
              "module": "B7"
            },
            {
              "value": "0.000000000000",
              "module": "C1"
            },
            {
              "value": "0.000000000000",
              "module": "C2"
            },
            {
              "value": "0.000000000000",
              "module": "C3"
            },
            {
              "value": "0.000000000000",
              "module": "C4"
            },
            {
              "value": "0.000000000000",
              "module": "D"
            },
            {
              "name": "referenceToUnitGroupDataSet",
              "value": {
                "shortDescription": [
                  {
                    "value": "kg CFC 11 eqv."
                  }
                ],
                "type": "unit group data set",
                "refObjectId": "d9e957c9-7309-4474-bf3a-7777df6c4e5b",
                "uri": "../unitgroups/d9e957c9-7309-4474-bf3a-7777df6c4e5b"
              }
            }
          ]
        }
      },
      {
        "referenceToLCIAMethodDataSet": {
          "shortDescription": [
            {
              "value": "Photochemical Ozone Creation Potential (POCP)",
              "lang": "en"
            },
            {
              "value": "Potensial for fotokjemisk oksidantdanning (POCP)",
              "lang": "no"
            }
          ],
          "type": "LCIA method data set",
          "refObjectId": "b5c610fe-def3-11e6-bf01-fe55135034f3",
          "version": "00.01.000"
        },
        "meanAmount": 0.0,
        "uncertaintyDistributionType": "undefined",
        "relativeStandardDeviation95In": 0,
        "other": {
          "anies": [
            {
              "value": "0.001080000000",
              "module": "A1"
            },
            {
              "value": "0.000030100000",
              "module": "A2"
            },
            {
              "value": "0.000003140000",
              "module": "A3"
            },
            {
              "value": "0.000197000000",
              "module": "A4"
            },
            {
              "value": "0.000117000000",
              "module": "A5"
            },
            {
              "value": "0.000000000000",
              "module": "B1"
            },
            {
              "value": "0.000000000000",
              "module": "B2"
            },
            {
              "value": "0.000000000000",
              "module": "B3"
            },
            {
              "value": "0.000000000000",
              "module": "B4"
            },
            {
              "value": "0.000000000000",
              "module": "B5"
            },
            {
              "value": "0.000000000000",
              "module": "B6"
            },
            {
              "value": "0.000000000000",
              "module": "B7"
            },
            {
              "value": "0.000002770000",
              "module": "C1"
            },
            {
              "value": "0.000013100000",
              "module": "C2"
            },
            {
              "value": "0.000019400000",
              "module": "C3"
            },
            {
              "value": "0.000022600000",
              "module": "C4"
            },
            {
              "value": "-0.000156000000",
              "module": "D"
            },
            {
              "name": "referenceToUnitGroupDataSet",
              "value": {
                "shortDescription": [
                  {
                    "value": "kg NMVOC eqv."
                  }
                ],
                "type": "unit group data set",
                "refObjectId": "d27c25f8-fbc1-44c6-b47b-4adbae4199c6",
                "uri": "../unitgroups/d27c25f8-fbc1-44c6-b47b-4adbae4199c6"
              }
            }
          ]
        }
      },
      {
        "referenceToLCIAMethodDataSet": {
          "shortDescription": [
            {
              "value": "Abiotic depletion potential - fossil resources (ADPF)",
              "lang": "en"
            },
            {
              "value": "Abiotisk utarmingspotensial for fossile ressurser, fosile brensler (ADP-fossil)",
              "lang": "no"
            }
          ],
          "type": "LCIA method data set",
          "refObjectId": "b2ad6110-c78d-11e6-9d9d-cec0c932ce01",
          "version": "00.01.000"
        },
        "meanAmount": 0.0,
        "uncertaintyDistributionType": "undefined",
        "relativeStandardDeviation95In": 0,
        "other": {
          "anies": [
            {
              "value": "17.200000000000",
              "module": "A1"
            },
            {
              "value": "0.138000000000",
              "module": "A2"
            },
            {
              "value": "0.012700000000",
              "module": "A3"
            },
            {
              "value": "0.317000000000",
              "module": "A4"
            },
            {
              "value": "1.730000000000",
              "module": "A5"
            },
            {
              "value": "0.000000000000",
              "module": "B1"
            },
            {
              "value": "0.000000000000",
              "module": "B2"
            },
            {
              "value": "0.000000000000",
              "module": "B3"
            },
            {
              "value": "0.000000000000",
              "module": "B4"
            },
            {
              "value": "0.000000000000",
              "module": "B5"
            },
            {
              "value": "0.000000000000",
              "module": "B6"
            },
            {
              "value": "0.000000000000",
              "module": "B7"
            },
            {
              "value": "0.036800000000",
              "module": "C1"
            },
            {
              "value": "0.069100000000",
              "module": "C2"
            },
            {
              "value": "0.168000000000",
              "module": "C3"
            },
            {
              "value": "0.121000000000",
              "module": "C4"
            },
            {
              "value": "-2.760000000000",
              "module": "D"
            },
            {
              "name": "referenceToUnitGroupDataSet",
              "value": {
                "shortDescription": [
                  {
                    "value": "MJ"
                  }
                ],
                "type": "unit group data set",
                "refObjectId": "93a60a57-a3c8-11da-a746-0800200c9a66",
                "uri": "../unitgroups/93a60a57-a3c8-11da-a746-0800200c9a66"
              }
            }
          ]
        }
      },
      {
        "referenceToLCIAMethodDataSet": {
          "shortDescription": [
            {
              "value": "Abiotic depletion potential - non-fossil resources (ADPE)",
              "lang": "en"
            },
            {
              "value": "Abiotisk utarmingspotensial for ikke-fossile ressurser, mineraler (ADP-elements)",
              "lang": "no"
            }
          ],
          "type": "LCIA method data set",
          "refObjectId": "b2ad6494-c78d-11e6-9d9d-cec0c932ce01",
          "version": "00.01.000"
        },
        "meanAmount": 0.0,
        "uncertaintyDistributionType": "undefined",
        "relativeStandardDeviation95In": 0,
        "other": {
          "anies": [
            {
              "value": "0.000015300000",
              "module": "A1"
            },
            {
              "value": "0.000000000916",
              "module": "A2"
            },
            {
              "value": "0.000000047600",
              "module": "A3"
            },
            {
              "value": "0.000000001850",
              "module": "A4"
            },
            {
              "value": "0.000001550000",
              "module": "A5"
            },
            {
              "value": "0.000000000000",
              "module": "B1"
            },
            {
              "value": "0.000000000000",
              "module": "B2"
            },
            {
              "value": "0.000000000000",
              "module": "B3"
            },
            {
              "value": "0.000000000000",
              "module": "B4"
            },
            {
              "value": "0.000000000000",
              "module": "B5"
            },
            {
              "value": "0.000000000000",
              "module": "B6"
            },
            {
              "value": "0.000000000000",
              "module": "B7"
            },
            {
              "value": "0.000000000609",
              "module": "C1"
            },
            {
              "value": "0.000000000395",
              "module": "C2"
            },
            {
              "value": "0.000000001870",
              "module": "C3"
            },
            {
              "value": "0.000000000572",
              "module": "C4"
            },
            {
              "value": "-0.000000015100",
              "module": "D"
            },
            {
              "name": "referenceToUnitGroupDataSet",
              "value": {
                "shortDescription": [
                  {
                    "value": "kg Sb-eqv."
                  }
                ],
                "type": "unit group data set",
                "refObjectId": "54ccd2d9-a32a-4fc2-923d-f2c8c93e89d4",
                "uri": "../unitgroups/54ccd2d9-a32a-4fc2-923d-f2c8c93e89d4"
              }
            }
          ]
        }
      },
      {
        "referenceToLCIAMethodDataSet": {
          "shortDescription": [
            {
              "value": "Water (user) deprivation potential (WDP)",
              "lang": "en"
            },
            {
              "value": "Utarmingspotensial for vannressurser (WDP)",
              "lang": "no"
            }
          ],
          "type": "LCIA method data set",
          "refObjectId": "b2ad66ce-c78d-11e6-9d9d-cec0c932ce01",
          "version": "00.01.000"
        },
        "meanAmount": 0.0,
        "uncertaintyDistributionType": "undefined",
        "relativeStandardDeviation95In": 0,
        "other": {
          "anies": [
            {
              "value": "0.058500000000",
              "module": "A1"
            },
            {
              "value": "0.000095900000",
              "module": "A2"
            },
            {
              "value": "0.000138000000",
              "module": "A3"
            },
            {
              "value": "0.000186000000",
              "module": "A4"
            },
            {
              "value": "0.006940000000",
              "module": "A5"
            },
            {
              "value": "0.000000000000",
              "module": "B1"
            },
            {
              "value": "0.000000000000",
              "module": "B2"
            },
            {
              "value": "0.000000000000",
              "module": "B3"
            },
            {
              "value": "0.000000000000",
              "module": "B4"
            },
            {
              "value": "0.000000000000",
              "module": "B5"
            },
            {
              "value": "0.000000000000",
              "module": "B6"
            },
            {
              "value": "0.000000000000",
              "module": "B7"
            },
            {
              "value": "0.000332000000",
              "module": "C1"
            },
            {
              "value": "0.000045100000",
              "module": "C2"
            },
            {
              "value": "0.009430000000",
              "module": "C3"
            },
            {
              "value": "-0.000011600000",
              "module": "C4"
            },
            {
              "value": "-0.010300000000",
              "module": "D"
            },
            {
              "name": "referenceToUnitGroupDataSet",
              "value": {
                "shortDescription": [
                  {
                    "value": "m3 world eqv."
                  }
                ],
                "type": "unit group data set",
                "refObjectId": "6ae2df01-888e-46c8-b17d-49fa3869b476",
                "uri": "../unitgroups/6ae2df01-888e-46c8-b17d-49fa3869b476"
              }
            }
          ]
        }
      },
      {
        "referenceToLCIAMethodDataSet": {
          "shortDescription": [
            {
              "value": "Global warming potential except emissions and uptake of biogenic carbon (GWP-IOBC/GHG)",
              "lang": "en"
            },
            {
              "value": "Globalt oppvarmingspotensial beregnet etter prinsippet om umiddelbar oksidasjon (GWP-IOBC)",
              "lang": "no"
            }
          ],
          "type": "LCIA method data set",
          "refObjectId": "fb774615-0575-45de-9a89-1ded92f19770",
          "version": "00.01.000"
        },
        "meanAmount": 0.0,
        "uncertaintyDistributionType": "undefined",
        "relativeStandardDeviation95In": 0,
        "other": {
          "anies": [
            {
              "name": "referenceToUnitGroupDataSet",
              "value": {
                "shortDescription": [
                  {
                    "value": "kg CO2 eqv."
                  }
                ],
                "type": "unit group data set",
                "refObjectId": "1ebf3012-d0db-4de2-aefd-ef30cedb0be1",
                "uri": "../unitgroups/1ebf3012-d0db-4de2-aefd-ef30cedb0be1"
              }
            }
          ]
        }
      }
    ]
  },
  "otherAttributes": {
    "{http://www.indata.network/EPD/2019}epd-version": "1.2"
  },
  "version": "1.1",
  "source": "https://node.epditaly.it/resource/datastocks/24493f94-1ca8-4cc7-a056-67cbe25aef5a/processes/0b18264c-993d-4a53-8e09-2eb44d178231"
}