{
  "processInformation": {
    "dataSetInformation": {
      "UUID": "0f3ae6eb-563f-471b-810a-a018cec5bc34",
      "name": {
        "baseName": [
          {
            "value": "POLYETHYLENE PIPING SYSTEM FOR WATER, GAS AND INDUSTRIAL APPLICATIONS TYPE \u201cPOLIETILENETUBI\u201d AND ELOFIT",
            "lang": "en"
          }
        ]
      },
      "classificationInformation": {
        "classification": [
          {
            "class": [
              {
                "value": "Other transportable goods, except metal products, machinery and equipment",
                "level": 0,
                "classId": "3"
              },
              {
                "value": "Rubber and plastics products",
                "level": 1,
                "classId": "36"
              }
            ],
            "name": "CPC 2.1"
          }
        ]
      },
      "generalComment": [
        {
          "value": "EPDITALY0089\r\nViene considerato l'intero ciclo di vita del prodotto dalla culla alla tomba \u201cfrom cradle to grave\" e i moduli di seguito descritti: A1, A2, A3, A4, A5, B1, B2, B3, B4, B5, B6, B7, C1, C2, C3, C4, D",
          "lang": "en"
        }
      ]
    },
    "quantitativeReference": {
      "referenceToReferenceFlow": [
        1
      ],
      "type": "Reference flow(s)"
    },
    "time": {
      "referenceYear": 2018,
      "dataSetValidUntil": 2024,
      "timeRepresentativenessDescription": [
        {
          "value": "dal 08/12/2019 al 08/12/2024 (Reference year: anno di raccolta dati 2018)",
          "lang": "en"
        }
      ],
      "other": {
        "anies": [
          {
            "name": "publicationDateOfEPD",
            "value": 1579132800000
          }
        ]
      }
    },
    "geography": {
      "locationOfOperationSupplyOrProduction": {
        "descriptionOfRestrictions": [
          {
            "value": "I sistemi di tubazioni in polietilene per acqua, gas e applicazioni industriali, vengono prodotti negli stabilimenti di Via dell'Artigianato n. 13 - 40023 Castel Guelfo di Bologna (BO) e Via Stefano Ferrario n. 8, Z.I. Sud-Ovest - 21052 Busto Arsizio (VA) Italy",
            "lang": "en"
          }
        ],
        "location": "GLO"
      }
    },
    "technology": {
      "technologyDescriptionAndIncludedProcesses": [
        {
          "value": "Qui di seguito viene descritto il processo di produzione dei sistemi di tubazioni in polietilene per acqua, gas e applicazioni industriali oggetto della presente EPD: La linea di estrusione dei tubi \u00e8 composta da estrusore, matrice, sistemi di raffreddamento, estrattore, stampante, sega e attrezzature di stacco. La funzione dell'estrusore \u00e8 quella di riscaldare, fondere, mescolare e trasportare il materiale alla filiera, dove viene modellato in un tubo. La linea del processo di stampaggio a iniezione dei raccordi, \u00e8 costituita da due presse, una per aprire e chiudere il blocco dello stampo e da un estrusore a iniezione per iniettare il materiale nella cavit\u00e0 del blocco stampo. ",
          "lang": "en"
        }
      ],
      "technologicalApplicability": [
        {
          "value": "Nupi Industrie Italiane S.p.A. produces Polyethylene (High density HDPE and Low density LDPE) pipes and fittings systems for the distribution of water, gas and industrial fluids under pressure.",
          "lang": "en"
        }
      ],
      "referenceToTechnologyFlowDiagrammOrPicture": [
        {
          "shortDescription": [
            {
              "value": "EPDITALY0089 flowchart",
              "lang": "en"
            }
          ],
          "type": "source data set",
          "refObjectId": "9184de88-b6e3-43fd-b838-be50eee626c7",
          "version": "00.00.002"
        }
      ]
    }
  },
  "modellingAndValidation": {
    "LCIMethodAndAllocation": {
      "typeOfDataSet": "EPD",
      "referenceToLCAMethodDetails": [
        {
          "shortDescription": [
            {
              "value": "PCR ICMQ-001/15 rev2.1",
              "lang": "en"
            }
          ],
          "type": "source data set",
          "refObjectId": "bc34cb82-81d9-4dde-9791-c1f91218a52f",
          "version": "00.00.002"
        }
      ],
      "other": {
        "anies": [
          {
            "name": "subType",
            "value": "average dataset"
          }
        ]
      }
    },
    "dataSourcesTreatmentAndRepresentativeness": {
      "referenceToDataSource": [
        {
          "shortDescription": [
            {
              "value": "GaBi database (general)",
              "lang": "en"
            }
          ],
          "type": "source data set",
          "refObjectId": "28d74cc0-db8b-4d7e-bc44-5f6d56ce0c4a",
          "version": "00.03.002"
        }
      ],
      "other": {
        "anies": [
          {
            "name": "referenceToOriginalEPD",
            "value": {
              "shortDescription": {
                "value": "EPDITALY0089 PDF",
                "defaultValue": "EPDITALY0089 PDF",
                "lstrings": [
                  {
                    "lang": "en",
                    "value": "EPDITALY0089 PDF"
                  }
                ]
              },
              "version": {
                "version": 2,
                "majorVersion": 0,
                "minorVersion": 0,
                "subMinorVersion": 2,
                "zero": false,
                "versionString": "00.00.002"
              },
              "type": "source data set",
              "uuid": {
                "uuid": "90861af6-6720-4198-9a42-9ab21b7f2a41"
              },
              "refObjectId": "90861af6-6720-4198-9a42-9ab21b7f2a41",
              "versionAsString": "00.00.002",
              "resourceURLs": [
                "https://node.epditaly.it/resource/sources/90861af6-6720-4198-9a42-9ab21b7f2a41/EPDITALY0089.pdf?version=00.00.002"
              ]
            }
          }
        ]
      }
    },
    "validation": {
      "review": [
        {
          "referenceToNameOfReviewerAndInstitution": [
            {
              "shortDescription": [
                {
                  "value": "ICMQ S.p.A.",
                  "lang": "en"
                }
              ],
              "type": "contact data set",
              "refObjectId": "6a2483f7-d823-4b36-ab56-f3b5bbaa976a",
              "version": "00.00.001"
            }
          ],
          "type": "Accredited third party review"
        }
      ]
    },
    "complianceDeclarations": {
      "compliance": [
        {
          "referenceToComplianceSystem": {
            "shortDescription": [
              {
                "value": "ISO 14025",
                "lang": "en"
              }
            ],
            "type": "source data set",
            "refObjectId": "4f2eb655-6e44-4874-a95a-e28f5442cd4d",
            "version": "00.00.001"
          }
        },
        {
          "referenceToComplianceSystem": {
            "shortDescription": [
              {
                "value": "EN 15804",
                "lang": "de"
              }
            ],
            "type": "source data set",
            "refObjectId": "b00f9ec0-7874-11e3-981f-0800200c9a66",
            "version": "00.02.000"
          }
        }
      ]
    }
  },
  "administrativeInformation": {
    "dataEntryBy": {
      "timeStamp": 1639411123682,
      "referenceToDataSetFormat": [
        {
          "shortDescription": [
            {
              "value": "EPD Data Format Extension",
              "lang": "de"
            }
          ],
          "type": "source data set",
          "refObjectId": "cba73800-7874-11e3-981f-0800200c9a66",
          "version": "00.01.000"
        },
        {
          "shortDescription": [
            {
              "value": "ILCD format",
              "lang": "en"
            }
          ],
          "type": "source data set",
          "refObjectId": "a97a0155-0234-4b87-b4ce-a45da52f2a40",
          "version": "01.00.000",
          "uri": "http://lca.jrc.ec.europa.eu/lcainfohub/sample_data/ilcd/sources/ILCD_Format_a97a0155-0234-4b87-b4ce-a45da52f2a40_01.00.000.xml"
        },
        {
          "shortDescription": [
            {
              "value": "EPD Data Format Extensions v1.2",
              "lang": "en"
            },
            {
              "value": "EPD-Datenformaterweiterungen v1.2",
              "lang": "de"
            }
          ],
          "type": "source data set",
          "refObjectId": "a29449fd-aa2f-4de8-b5d7-4b06b43c6fde",
          "version": "00.01.000"
        }
      ]
    },
    "publicationAndOwnership": {
      "dataSetVersion": "00.00.028",
      "referenceToRegistrationAuthority": {
        "shortDescription": [
          {
            "value": "ICMQ S.p.A.",
            "lang": "en"
          }
        ],
        "type": "contact data set",
        "refObjectId": "6a2483f7-d823-4b36-ab56-f3b5bbaa976a",
        "version": "00.00.001"
      },
      "registrationNumber": "EPDITALY0089",
      "referenceToOwnershipOfDataSet": {
        "shortDescription": [
          {
            "value": "Nupi Industrie Italiane S.p.A.",
            "lang": "en"
          }
        ],
        "type": "contact data set",
        "refObjectId": "85555831-9600-4de6-864c-03e9d611ab75",
        "version": "00.00.001"
      },
      "other": {
        "anies": [
          {
            "name": "referenceToPublisher",
            "value": {
              "shortDescription": [
                {
                  "value": "EPDItaly",
                  "lang": "en"
                }
              ],
              "type": "contact data set",
              "refObjectId": "9433b9cf-1d4a-420f-8c09-88d2472225b9",
              "version": "00.00.001"
            }
          }
        ]
      }
    }
  },
  "exchanges": {
    "exchange": [
      {
        "dataSetInternalID": 1,
        "referenceToFlowDataSet": {
          "shortDescription": [
            {
              "value": "POLYETHYLENE PIPING SYSTEM FOR WATER, GAS AND INDUSTRIAL APPLICATIONS TYPE \u201cPOLIETILENETUBI\u201d AND ELOFIT",
              "lang": "en"
            }
          ],
          "type": "flow data set",
          "refObjectId": "ebd8c4a1-e403-4992-abcf-8639a8f482f2",
          "version": "00.00.001"
        },
        "meanAmount": 1.0,
        "resultingAmount": 1.0,
        "referenceFlow": true,
        "resultingflowAmount": 100.0,
        "flowProperties": [
          {
            "name": [
              {
                "lang": "en",
                "value": "Length"
              }
            ],
            "uuid": "838aaa23-0117-11db-92e3-0800200c9a66",
            "referenceFlowProperty": true,
            "meanValue": 100.0,
            "referenceUnit": "m",
            "unitGroupUUID": "838aaa22-0117-11db-92e3-0800200c9a66"
          }
        ],
        "materialProperties": [
          {
            "name": "bulk density",
            "value": "951.0",
            "unit": "kg/m^3",
            "unitDescription": "kilograms per cubic metre"
          }
        ],
        "typeOfFlow": "Product flow"
      },
      {
        "dataSetInternalID": 2,
        "referenceToFlowDataSet": {
          "shortDescription": [
            {
              "value": "Components for re-use (CRU)",
              "lang": "en"
            },
            {
              "value": "Komponenten f\u00fcr die Wiederverwendung (CRU)",
              "lang": "de"
            },
            {
              "value": "Componentes para su reutilizaci\u00f3n (CRU)",
              "lang": "es"
            }
          ],
          "type": "flow data set",
          "refObjectId": "a2b32f97-3fc7-4af2-b209-525bc6426f33",
          "version": "30.00.000"
        },
        "exchange direction": "OUTPUT",
        "meanAmount": 0.0,
        "other": {
          "anies": [
            {
              "value": "0.0",
              "module": "A1-A3"
            },
            {
              "value": "0.0",
              "module": "A4"
            },
            {
              "value": "0.0",
              "module": "A5"
            },
            {
              "value": "0.0",
              "module": "B1"
            },
            {
              "value": "0.0",
              "module": "B2"
            },
            {
              "value": "0.0",
              "module": "B3"
            },
            {
              "value": "0.0",
              "module": "B4"
            },
            {
              "value": "0.0",
              "module": "B5"
            },
            {
              "value": "0.0",
              "module": "B6"
            },
            {
              "value": "0.0",
              "module": "B7"
            },
            {
              "value": "0.0",
              "module": "C1"
            },
            {
              "value": "0.0",
              "module": "C2"
            },
            {
              "value": "0.0",
              "module": "C3"
            },
            {
              "value": "0.0",
              "module": "C4"
            },
            {
              "value": "0.0",
              "module": "D"
            },
            {
              "name": "referenceToUnitGroupDataSet",
              "value": {
                "shortDescription": [
                  {
                    "value": "kg"
                  }
                ],
                "type": "unit group data set",
                "refObjectId": "ad38d542-3fe9-439d-9b95-2f5f7752acaf",
                "uri": "../unitgroups/ad38d542-3fe9-439d-9b95-2f5f7752acaf"
              }
            }
          ]
        },
        "flowProperties": [],
        "typeOfFlow": "Other flow",
        "classification": {
          "classHierarchy": "Gr\u00f6\u00dfen / Umweltliche Gr\u00f6\u00dfen / EPD EN 15804 / LCI Indikatoren",
          "name": "GaBiCategories"
        }
      },
      {
        "dataSetInternalID": 3,
        "referenceToFlowDataSet": {
          "shortDescription": [
            {
              "value": "Exported electrical energy (EEE)",
              "lang": "en"
            },
            {
              "value": "Exportierte elektrische Energie (EEE)",
              "lang": "de"
            },
            {
              "value": "Energ\u00eda exportada electrica (EEE)",
              "lang": "es"
            }
          ],
          "type": "flow data set",
          "refObjectId": "4da0c987-2b76-40d6-9e9e-82a017aaaf29",
          "version": "30.00.000"
        },
        "exchange direction": "OUTPUT",
        "meanAmount": 0.0,
        "other": {
          "anies": [
            {
              "value": "0.0",
              "module": "A1-A3"
            },
            {
              "value": "0.0",
              "module": "A4"
            },
            {
              "value": "18.9",
              "module": "A5"
            },
            {
              "value": "0.0",
              "module": "B1"
            },
            {
              "value": "0.0",
              "module": "B2"
            },
            {
              "value": "0.0",
              "module": "B3"
            },
            {
              "value": "0.0",
              "module": "B4"
            },
            {
              "value": "0.0",
              "module": "B5"
            },
            {
              "value": "0.0",
              "module": "B6"
            },
            {
              "value": "0.0",
              "module": "B7"
            },
            {
              "value": "0.0",
              "module": "C1"
            },
            {
              "value": "0.0",
              "module": "C2"
            },
            {
              "value": "32.7",
              "module": "C3"
            },
            {
              "value": "0.0",
              "module": "C4"
            },
            {
              "value": "0.0",
              "module": "D"
            },
            {
              "name": "referenceToUnitGroupDataSet",
              "value": {
                "shortDescription": [
                  {
                    "value": "MJ"
                  }
                ],
                "type": "unit group data set",
                "refObjectId": "93a60a57-a3c8-11da-a746-0800200c9a66",
                "uri": "../unitgroups/93a60a57-a3c8-11da-a746-0800200c9a66"
              }
            }
          ]
        },
        "flowProperties": [],
        "typeOfFlow": "Other flow",
        "classification": {
          "classHierarchy": "Gr\u00f6\u00dfen / Umweltliche Gr\u00f6\u00dfen / EPD EN 15804 / LCI Indikatoren",
          "name": "GaBiCategories"
        }
      },
      {
        "dataSetInternalID": 4,
        "referenceToFlowDataSet": {
          "shortDescription": [
            {
              "value": "Exported thermal energy (EET)",
              "lang": "en"
            },
            {
              "value": "Exportierte thermische Energie (EET)",
              "lang": "de"
            },
            {
              "value": "Energ\u00eda exportada termal (EET)",
              "lang": "es"
            }
          ],
          "type": "flow data set",
          "refObjectId": "98daf38a-7a79-46d3-9a37-2b7bd0955810",
          "version": "30.00.000"
        },
        "exchange direction": "OUTPUT",
        "meanAmount": 0.0,
        "other": {
          "anies": [
            {
              "value": "0.0",
              "module": "A1-A3"
            },
            {
              "value": "0.0",
              "module": "A4"
            },
            {
              "value": "34.8",
              "module": "A5"
            },
            {
              "value": "0.0",
              "module": "B1"
            },
            {
              "value": "0.0",
              "module": "B2"
            },
            {
              "value": "0.0",
              "module": "B3"
            },
            {
              "value": "0.0",
              "module": "B4"
            },
            {
              "value": "0.0",
              "module": "B5"
            },
            {
              "value": "0.0",
              "module": "B6"
            },
            {
              "value": "0.0",
              "module": "B7"
            },
            {
              "value": "0.0",
              "module": "C1"
            },
            {
              "value": "0.0",
              "module": "C2"
            },
            {
              "value": "58.2",
              "module": "C3"
            },
            {
              "value": "0.0",
              "module": "C4"
            },
            {
              "value": "0.0",
              "module": "D"
            },
            {
              "name": "referenceToUnitGroupDataSet",
              "value": {
                "shortDescription": [
                  {
                    "value": "MJ"
                  }
                ],
                "type": "unit group data set",
                "refObjectId": "93a60a57-a3c8-11da-a746-0800200c9a66",
                "uri": "../unitgroups/93a60a57-a3c8-11da-a746-0800200c9a66"
              }
            }
          ]
        },
        "flowProperties": [],
        "typeOfFlow": "Other flow",
        "classification": {
          "classHierarchy": "Gr\u00f6\u00dfen / Umweltliche Gr\u00f6\u00dfen / EPD EN 15804 / LCI Indikatoren",
          "name": "GaBiCategories"
        }
      },
      {
        "dataSetInternalID": 5,
        "referenceToFlowDataSet": {
          "shortDescription": [
            {
              "value": "Hazardous waste disposed (HWD)",
              "lang": "en"
            },
            {
              "value": "Gef\u00e4hrlicher Abfall zur Deponie (HWD)",
              "lang": "de"
            },
            {
              "value": "Residuos peligrosos eliminados (HWD)",
              "lang": "es"
            }
          ],
          "type": "flow data set",
          "refObjectId": "430f9e0f-59b2-46a0-8e0d-55e0e84948fc",
          "version": "30.00.000"
        },
        "exchange direction": "OUTPUT",
        "meanAmount": 0.0,
        "other": {
          "anies": [
            {
              "value": "2.46E-5",
              "module": "A1-A3"
            },
            {
              "value": "1.17E-5",
              "module": "A4"
            },
            {
              "value": "1.43E-4",
              "module": "A5"
            },
            {
              "value": "0.0",
              "module": "B1"
            },
            {
              "value": "0.0",
              "module": "B2"
            },
            {
              "value": "0.0",
              "module": "B3"
            },
            {
              "value": "0.0",
              "module": "B4"
            },
            {
              "value": "0.0",
              "module": "B5"
            },
            {
              "value": "0.0",
              "module": "B6"
            },
            {
              "value": "0.0",
              "module": "B7"
            },
            {
              "value": "9.88E-10",
              "module": "C1"
            },
            {
              "value": "7.69E-7",
              "module": "C2"
            },
            {
              "value": "1.72E-8",
              "module": "C3"
            },
            {
              "value": "0.0",
              "module": "C4"
            },
            {
              "value": "-2.31E-7",
              "module": "D"
            },
            {
              "name": "referenceToUnitGroupDataSet",
              "value": {
                "shortDescription": [
                  {
                    "value": "kg"
                  }
                ],
                "type": "unit group data set",
                "refObjectId": "ad38d542-3fe9-439d-9b95-2f5f7752acaf",
                "uri": "../unitgroups/ad38d542-3fe9-439d-9b95-2f5f7752acaf"
              }
            }
          ]
        },
        "flowProperties": [],
        "typeOfFlow": "Other flow",
        "classification": {
          "classHierarchy": "Gr\u00f6\u00dfen / Umweltliche Gr\u00f6\u00dfen / EPD EN 15804 / LCI Indikatoren",
          "name": "GaBiCategories"
        }
      },
      {
        "dataSetInternalID": 6,
        "referenceToFlowDataSet": {
          "shortDescription": [
            {
              "value": "Materials for energy recovery (MER)",
              "lang": "en"
            },
            {
              "value": "Stoffe f\u00fcr die Energier\u00fcckgewinnung (MER)",
              "lang": "de"
            },
            {
              "value": "Materiales para valorizaci\u00f3n energ\u00e9tica (recuperaci\u00f3n de energ\u00eda) (MER)",
              "lang": "es"
            }
          ],
          "type": "flow data set",
          "refObjectId": "59a9181c-3aaf-46ee-8b13-2b3723b6e447",
          "version": "30.00.000"
        },
        "exchange direction": "OUTPUT",
        "meanAmount": 0.0,
        "other": {
          "anies": [
            {
              "value": "0.0",
              "module": "A1-A3"
            },
            {
              "value": "0.0",
              "module": "A4"
            },
            {
              "value": "0.0",
              "module": "A5"
            },
            {
              "value": "0.0",
              "module": "B1"
            },
            {
              "value": "0.0",
              "module": "B2"
            },
            {
              "value": "0.0",
              "module": "B3"
            },
            {
              "value": "0.0",
              "module": "B4"
            },
            {
              "value": "0.0",
              "module": "B5"
            },
            {
              "value": "0.0",
              "module": "B6"
            },
            {
              "value": "0.0",
              "module": "B7"
            },
            {
              "value": "0.0",
              "module": "C1"
            },
            {
              "value": "0.0",
              "module": "C2"
            },
            {
              "value": "0.0",
              "module": "C3"
            },
            {
              "value": "0.0",
              "module": "C4"
            },
            {
              "value": "0.0",
              "module": "D"
            },
            {
              "name": "referenceToUnitGroupDataSet",
              "value": {
                "shortDescription": [
                  {
                    "value": "kg"
                  }
                ],
                "type": "unit group data set",
                "refObjectId": "ad38d542-3fe9-439d-9b95-2f5f7752acaf",
                "uri": "../unitgroups/ad38d542-3fe9-439d-9b95-2f5f7752acaf"
              }
            }
          ]
        },
        "flowProperties": [],
        "typeOfFlow": "Other flow",
        "classification": {
          "classHierarchy": "Gr\u00f6\u00dfen / Umweltliche Gr\u00f6\u00dfen / EPD EN 15804 / LCI Indikatoren",
          "name": "GaBiCategories"
        }
      },
      {
        "dataSetInternalID": 7,
        "referenceToFlowDataSet": {
          "shortDescription": [
            {
              "value": "Materials for recycling (MFR)",
              "lang": "en"
            },
            {
              "value": "Stoffe zum Recycling (MFR)",
              "lang": "de"
            },
            {
              "value": "Materiales para el reciclaje (MFR)",
              "lang": "es"
            }
          ],
          "type": "flow data set",
          "refObjectId": "d7fe48a5-4103-49c8-9aae-b0b5dfdbd6ae",
          "version": "30.00.000"
        },
        "exchange direction": "OUTPUT",
        "meanAmount": 0.0,
        "other": {
          "anies": [
            {
              "value": "0.0",
              "module": "A1-A3"
            },
            {
              "value": "0.0",
              "module": "A4"
            },
            {
              "value": "2.78",
              "module": "A5"
            },
            {
              "value": "0.0",
              "module": "B1"
            },
            {
              "value": "0.0",
              "module": "B2"
            },
            {
              "value": "0.0",
              "module": "B3"
            },
            {
              "value": "0.0",
              "module": "B4"
            },
            {
              "value": "0.0",
              "module": "B5"
            },
            {
              "value": "0.0",
              "module": "B6"
            },
            {
              "value": "0.0",
              "module": "B7"
            },
            {
              "value": "0.0",
              "module": "C1"
            },
            {
              "value": "0.0",
              "module": "C2"
            },
            {
              "value": "4.24",
              "module": "C3"
            },
            {
              "value": "0.0",
              "module": "C4"
            },
            {
              "value": "0.0",
              "module": "D"
            },
            {
              "name": "referenceToUnitGroupDataSet",
              "value": {
                "shortDescription": [
                  {
                    "value": "kg"
                  }
                ],
                "type": "unit group data set",
                "refObjectId": "ad38d542-3fe9-439d-9b95-2f5f7752acaf",
                "uri": "../unitgroups/ad38d542-3fe9-439d-9b95-2f5f7752acaf"
              }
            }
          ]
        },
        "flowProperties": [],
        "typeOfFlow": "Other flow",
        "classification": {
          "classHierarchy": "Gr\u00f6\u00dfen / Umweltliche Gr\u00f6\u00dfen / EPD EN 15804 / LCI Indikatoren",
          "name": "GaBiCategories"
        }
      },
      {
        "dataSetInternalID": 8,
        "referenceToFlowDataSet": {
          "shortDescription": [
            {
              "value": "Non hazardous waste dispose (NHWD)",
              "lang": "en"
            },
            {
              "value": "Entsorgter nicht gef\u00e4hrlicher Abfall (NHWD)",
              "lang": "de"
            },
            {
              "value": "Residuos no peligrosos eliminados (NHWD)",
              "lang": "es"
            }
          ],
          "type": "flow data set",
          "refObjectId": "b29ef66b-e286-4afa-949f-62f1a7b4d7fa",
          "version": "30.00.000"
        },
        "exchange direction": "OUTPUT",
        "meanAmount": 0.0,
        "other": {
          "anies": [
            {
              "value": "12.1",
              "module": "A1-A3"
            },
            {
              "value": "0.0181",
              "module": "A4"
            },
            {
              "value": "9.67",
              "module": "A5"
            },
            {
              "value": "0.0",
              "module": "B1"
            },
            {
              "value": "0.0",
              "module": "B2"
            },
            {
              "value": "0.0",
              "module": "B3"
            },
            {
              "value": "0.0",
              "module": "B4"
            },
            {
              "value": "0.0",
              "module": "B5"
            },
            {
              "value": "0.0",
              "module": "B6"
            },
            {
              "value": "0.0",
              "module": "B7"
            },
            {
              "value": "0.0015",
              "module": "C1"
            },
            {
              "value": "0.00112",
              "module": "C2"
            },
            {
              "value": "0.731",
              "module": "C3"
            },
            {
              "value": "0.0",
              "module": "C4"
            },
            {
              "value": "-0.267",
              "module": "D"
            },
            {
              "name": "referenceToUnitGroupDataSet",
              "value": {
                "shortDescription": [
                  {
                    "value": "kg"
                  }
                ],
                "type": "unit group data set",
                "refObjectId": "ad38d542-3fe9-439d-9b95-2f5f7752acaf",
                "uri": "../unitgroups/ad38d542-3fe9-439d-9b95-2f5f7752acaf"
              }
            }
          ]
        },
        "flowProperties": [],
        "typeOfFlow": "Other flow",
        "classification": {
          "classHierarchy": "Gr\u00f6\u00dfen / Umweltliche Gr\u00f6\u00dfen / EPD EN 15804 / LCI Indikatoren",
          "name": "GaBiCategories"
        }
      },
      {
        "dataSetInternalID": 9,
        "referenceToFlowDataSet": {
          "shortDescription": [
            {
              "value": "Radioactive waste disposed (RWD)",
              "lang": "en"
            },
            {
              "value": "Entsorgter radioaktiver Abfall (RWD)",
              "lang": "de"
            },
            {
              "value": "Residuos radiactivos eliminados (RWD)",
              "lang": "es"
            }
          ],
          "type": "flow data set",
          "refObjectId": "3449546e-52ad-4b39-b809-9fb77cea8ff6",
          "version": "30.00.000"
        },
        "exchange direction": "OUTPUT",
        "meanAmount": 0.0,
        "other": {
          "anies": [
            {
              "value": "0.194",
              "module": "A1-A3"
            },
            {
              "value": "5.1E-4",
              "module": "A4"
            },
            {
              "value": "0.00723",
              "module": "A5"
            },
            {
              "value": "0.0",
              "module": "B1"
            },
            {
              "value": "0.0",
              "module": "B2"
            },
            {
              "value": "0.0",
              "module": "B3"
            },
            {
              "value": "0.0",
              "module": "B4"
            },
            {
              "value": "0.0",
              "module": "B5"
            },
            {
              "value": "0.0",
              "module": "B6"
            },
            {
              "value": "0.0",
              "module": "B7"
            },
            {
              "value": "3.33E-4",
              "module": "C1"
            },
            {
              "value": "1.87E-5",
              "module": "C2"
            },
            {
              "value": "0.00211",
              "module": "C3"
            },
            {
              "value": "0.0",
              "module": "C4"
            },
            {
              "value": "-0.0247",
              "module": "D"
            },
            {
              "name": "referenceToUnitGroupDataSet",
              "value": {
                "shortDescription": [
                  {
                    "value": "kg"
                  }
                ],
                "type": "unit group data set",
                "refObjectId": "ad38d542-3fe9-439d-9b95-2f5f7752acaf",
                "uri": "../unitgroups/ad38d542-3fe9-439d-9b95-2f5f7752acaf"
              }
            }
          ]
        },
        "flowProperties": [],
        "typeOfFlow": "Other flow",
        "classification": {
          "classHierarchy": "Gr\u00f6\u00dfen / Umweltliche Gr\u00f6\u00dfen / EPD EN 15804 / LCI Indikatoren",
          "name": "GaBiCategories"
        }
      },
      {
        "dataSetInternalID": 10,
        "referenceToFlowDataSet": {
          "shortDescription": [
            {
              "value": "Total use of non renewable primary energy resource (PENRT)",
              "lang": "en"
            },
            {
              "value": "Total nicht erneuerbare Prim\u00e4renergie (PENRT)",
              "lang": "de"
            },
            {
              "value": "Uso total de la energ\u00eda primaria no renovable (energ\u00eda primaria y recursos de energ\u00eda primaria renovable utilizada como materia prima) (PENRT)",
              "lang": "es"
            }
          ],
          "type": "flow data set",
          "refObjectId": "06159210-646b-4c8d-8583-da9b3b95a6c1",
          "version": "30.00.000"
        },
        "exchange direction": "INPUT",
        "meanAmount": 0.0,
        "other": {
          "anies": [
            {
              "value": "16600.0",
              "module": "A1-A3"
            },
            {
              "value": "277.0",
              "module": "A4"
            },
            {
              "value": "2860.0",
              "module": "A5"
            },
            {
              "value": "0.0",
              "module": "B1"
            },
            {
              "value": "0.0",
              "module": "B2"
            },
            {
              "value": "0.0",
              "module": "B3"
            },
            {
              "value": "0.0",
              "module": "B4"
            },
            {
              "value": "0.0",
              "module": "B5"
            },
            {
              "value": "0.0",
              "module": "B6"
            },
            {
              "value": "0.0",
              "module": "B7"
            },
            {
              "value": "2.07",
              "module": "C1"
            },
            {
              "value": "13.8",
              "module": "C2"
            },
            {
              "value": "34.4",
              "module": "C3"
            },
            {
              "value": "0.0",
              "module": "C4"
            },
            {
              "value": "-733.0",
              "module": "D"
            },
            {
              "name": "referenceToUnitGroupDataSet",
              "value": {
                "shortDescription": [
                  {
                    "value": "MJ"
                  }
                ],
                "type": "unit group data set",
                "refObjectId": "93a60a57-a3c8-11da-a746-0800200c9a66",
                "uri": "../unitgroups/93a60a57-a3c8-11da-a746-0800200c9a66"
              }
            }
          ]
        },
        "flowProperties": [],
        "typeOfFlow": "Other flow",
        "classification": {
          "classHierarchy": "Gr\u00f6\u00dfen / Umweltliche Gr\u00f6\u00dfen / EPD EN 15804 / LCI Indikatoren",
          "name": "GaBiCategories"
        }
      },
      {
        "dataSetInternalID": 11,
        "referenceToFlowDataSet": {
          "shortDescription": [
            {
              "value": "Total use of renewable primary energy resources (PERT)",
              "lang": "en"
            },
            {
              "value": "Total erneuerbare Prim\u00e4renergie (PERT)",
              "lang": "de"
            },
            {
              "value": "Uso total de la energ\u00eda primaria renovable (energ\u00eda primaria y recursos de energ\u00eda primaria renovable utilizada como materia prima) (PERT)",
              "lang": "es"
            }
          ],
          "type": "flow data set",
          "refObjectId": "53f97275-fa8a-4cdd-9024-65936002acd0",
          "version": "30.00.000"
        },
        "exchange direction": "INPUT",
        "meanAmount": 0.0,
        "other": {
          "anies": [
            {
              "value": "1420.0",
              "module": "A1-A3"
            },
            {
              "value": "12.7",
              "module": "A4"
            },
            {
              "value": "157.0",
              "module": "A5"
            },
            {
              "value": "0.0",
              "module": "B1"
            },
            {
              "value": "0.0",
              "module": "B2"
            },
            {
              "value": "0.0",
              "module": "B3"
            },
            {
              "value": "0.0",
              "module": "B4"
            },
            {
              "value": "0.0",
              "module": "B5"
            },
            {
              "value": "0.0",
              "module": "B6"
            },
            {
              "value": "0.0",
              "module": "B7"
            },
            {
              "value": "0.832",
              "module": "C1"
            },
            {
              "value": "0.799",
              "module": "C2"
            },
            {
              "value": "3.54",
              "module": "C3"
            },
            {
              "value": "0.0",
              "module": "C4"
            },
            {
              "value": "-75.5",
              "module": "D"
            },
            {
              "name": "referenceToUnitGroupDataSet",
              "value": {
                "shortDescription": [
                  {
                    "value": "MJ"
                  }
                ],
                "type": "unit group data set",
                "refObjectId": "93a60a57-a3c8-11da-a746-0800200c9a66",
                "uri": "../unitgroups/93a60a57-a3c8-11da-a746-0800200c9a66"
              }
            }
          ]
        },
        "flowProperties": [],
        "typeOfFlow": "Other flow",
        "classification": {
          "classHierarchy": "Gr\u00f6\u00dfen / Umweltliche Gr\u00f6\u00dfen / EPD EN 15804 / LCI Indikatoren",
          "name": "GaBiCategories"
        }
      },
      {
        "dataSetInternalID": 12,
        "referenceToFlowDataSet": {
          "shortDescription": [
            {
              "value": "Use of net fresh water (FW)",
              "lang": "en"
            },
            {
              "value": "Einsatz von S\u00fc\u00dfwasserressourcen (FW)",
              "lang": "de"
            },
            {
              "value": "Uso neto de recursos de agua dulce (FW)",
              "lang": "es"
            }
          ],
          "type": "flow data set",
          "refObjectId": "3cf952c8-f3a4-461d-8c96-96456ca62246",
          "version": "30.00.000"
        },
        "exchange direction": "INPUT",
        "meanAmount": 0.0,
        "other": {
          "anies": [
            {
              "value": "3.0",
              "module": "A1-A3"
            },
            {
              "value": "0.0214",
              "module": "A4"
            },
            {
              "value": "0.315",
              "module": "A5"
            },
            {
              "value": "0.0",
              "module": "B1"
            },
            {
              "value": "0.0",
              "module": "B2"
            },
            {
              "value": "0.0",
              "module": "B3"
            },
            {
              "value": "0.0",
              "module": "B4"
            },
            {
              "value": "0.0",
              "module": "B5"
            },
            {
              "value": "0.0",
              "module": "B6"
            },
            {
              "value": "0.0",
              "module": "B7"
            },
            {
              "value": "9.8E-4",
              "module": "C1"
            },
            {
              "value": "0.00135",
              "module": "C2"
            },
            {
              "value": "0.0425",
              "module": "C3"
            },
            {
              "value": "0.0",
              "module": "C4"
            },
            {
              "value": "-0.125",
              "module": "D"
            },
            {
              "name": "referenceToUnitGroupDataSet",
              "value": {
                "shortDescription": [
                  {
                    "value": "m3"
                  }
                ],
                "type": "unit group data set",
                "refObjectId": "cd950537-0a98-4044-9ba7-9f9a68d0a504",
                "uri": "../unitgroups/cd950537-0a98-4044-9ba7-9f9a68d0a504"
              }
            }
          ]
        },
        "flowProperties": [],
        "typeOfFlow": "Other flow",
        "classification": {
          "classHierarchy": "Gr\u00f6\u00dfen / Umweltliche Gr\u00f6\u00dfen / EPD EN 15804 / LCI Indikatoren",
          "name": "GaBiCategories"
        }
      },
      {
        "dataSetInternalID": 13,
        "referenceToFlowDataSet": {
          "shortDescription": [
            {
              "value": "Use of non renewable primary energy (PENRE)",
              "lang": "en"
            },
            {
              "value": "Nicht-erneuerbare Prim\u00e4renergie als Energietr\u00e4ger (PENRE)",
              "lang": "de"
            },
            {
              "value": "Uso de energ\u00eda primaria no renovable, excluyendo los recursos de energ\u00eda primaria no renovable utilizada como materia prima (PENRE)",
              "lang": "es"
            }
          ],
          "type": "flow data set",
          "refObjectId": "ac857178-2b45-46ec-892a-a9a4332f0372",
          "version": "30.00.000"
        },
        "exchange direction": "INPUT",
        "meanAmount": 0.0,
        "other": {
          "anies": [
            {
              "value": "7590.0",
              "module": "A1-A3"
            },
            {
              "value": "277.0",
              "module": "A4"
            },
            {
              "value": "2960.0",
              "module": "A5"
            },
            {
              "value": "0.0",
              "module": "B1"
            },
            {
              "value": "0.0",
              "module": "B2"
            },
            {
              "value": "0.0",
              "module": "B3"
            },
            {
              "value": "0.0",
              "module": "B4"
            },
            {
              "value": "0.0",
              "module": "B5"
            },
            {
              "value": "0.0",
              "module": "B6"
            },
            {
              "value": "0.0",
              "module": "B7"
            },
            {
              "value": "2.07",
              "module": "C1"
            },
            {
              "value": "13.8",
              "module": "C2"
            },
            {
              "value": "259.0",
              "module": "C3"
            },
            {
              "value": "0.0",
              "module": "C4"
            },
            {
              "value": "-733.0",
              "module": "D"
            },
            {
              "name": "referenceToUnitGroupDataSet",
              "value": {
                "shortDescription": [
                  {
                    "value": "MJ"
                  }
                ],
                "type": "unit group data set",
                "refObjectId": "93a60a57-a3c8-11da-a746-0800200c9a66",
                "uri": "../unitgroups/93a60a57-a3c8-11da-a746-0800200c9a66"
              }
            }
          ]
        },
        "flowProperties": [],
        "typeOfFlow": "Other flow",
        "classification": {
          "classHierarchy": "Gr\u00f6\u00dfen / Umweltliche Gr\u00f6\u00dfen / EPD EN 15804 / LCI Indikatoren",
          "name": "GaBiCategories"
        }
      },
      {
        "dataSetInternalID": 14,
        "referenceToFlowDataSet": {
          "shortDescription": [
            {
              "value": "Use of non renewable primary energy resources used as raw materials (PENRM)",
              "lang": "en"
            },
            {
              "value": "Nicht-erneuerbare Prim\u00e4renergie zur stofflichen Nutzung (PENRM)",
              "lang": "de"
            },
            {
              "value": "Uso de la energ\u00eda primaria no renovable utilizada como materia prima (PENRM)",
              "lang": "es"
            }
          ],
          "type": "flow data set",
          "refObjectId": "1421caa0-679d-4bf4-b282-0eb850ccae27",
          "version": "30.00.000"
        },
        "exchange direction": "INPUT",
        "meanAmount": 0.0,
        "other": {
          "anies": [
            {
              "value": "8990.0",
              "module": "A1-A3"
            },
            {
              "value": "0.0",
              "module": "A4"
            },
            {
              "value": "-101.0",
              "module": "A5"
            },
            {
              "value": "0.0",
              "module": "B1"
            },
            {
              "value": "0.0",
              "module": "B2"
            },
            {
              "value": "0.0",
              "module": "B3"
            },
            {
              "value": "0.0",
              "module": "B4"
            },
            {
              "value": "0.0",
              "module": "B5"
            },
            {
              "value": "0.0",
              "module": "B6"
            },
            {
              "value": "0.0",
              "module": "B7"
            },
            {
              "value": "0.0",
              "module": "C1"
            },
            {
              "value": "0.0",
              "module": "C2"
            },
            {
              "value": "-224.0",
              "module": "C3"
            },
            {
              "value": "0.0",
              "module": "C4"
            },
            {
              "value": "0.0",
              "module": "D"
            },
            {
              "name": "referenceToUnitGroupDataSet",
              "value": {
                "shortDescription": [
                  {
                    "value": "MJ"
                  }
                ],
                "type": "unit group data set",
                "refObjectId": "93a60a57-a3c8-11da-a746-0800200c9a66",
                "uri": "../unitgroups/93a60a57-a3c8-11da-a746-0800200c9a66"
              }
            }
          ]
        },
        "flowProperties": [],
        "typeOfFlow": "Other flow",
        "classification": {
          "classHierarchy": "Gr\u00f6\u00dfen / Umweltliche Gr\u00f6\u00dfen / EPD EN 15804 / LCI Indikatoren",
          "name": "GaBiCategories"
        }
      },
      {
        "dataSetInternalID": 15,
        "referenceToFlowDataSet": {
          "shortDescription": [
            {
              "value": "Use of non renewable secondary fuels (NRSF)",
              "lang": "en"
            },
            {
              "value": "Nicht erneuerbare Sekund\u00e4rbrennstoffe (NRSF)",
              "lang": "de"
            },
            {
              "value": "Uso de combustibles secundarios no renovables (NRSF)",
              "lang": "es"
            }
          ],
          "type": "flow data set",
          "refObjectId": "89def144-d39a-4287-b86f-efde453ddcb2",
          "version": "30.00.000"
        },
        "exchange direction": "INPUT",
        "meanAmount": 0.0,
        "other": {
          "anies": [
            {
              "value": "1.09E-9",
              "module": "A1-A3"
            },
            {
              "value": "0.0",
              "module": "A4"
            },
            {
              "value": "1.08E-21",
              "module": "A5"
            },
            {
              "value": "0.0",
              "module": "B1"
            },
            {
              "value": "0.0",
              "module": "B2"
            },
            {
              "value": "0.0",
              "module": "B3"
            },
            {
              "value": "0.0",
              "module": "B4"
            },
            {
              "value": "0.0",
              "module": "B5"
            },
            {
              "value": "0.0",
              "module": "B6"
            },
            {
              "value": "0.0",
              "module": "B7"
            },
            {
              "value": "0.0",
              "module": "C1"
            },
            {
              "value": "0.0",
              "module": "C2"
            },
            {
              "value": "0.0",
              "module": "C3"
            },
            {
              "value": "0.0",
              "module": "C4"
            },
            {
              "value": "-1.38E-21",
              "module": "D"
            },
            {
              "name": "referenceToUnitGroupDataSet",
              "value": {
                "shortDescription": [
                  {
                    "value": "MJ"
                  }
                ],
                "type": "unit group data set",
                "refObjectId": "93a60a57-a3c8-11da-a746-0800200c9a66",
                "uri": "../unitgroups/93a60a57-a3c8-11da-a746-0800200c9a66"
              }
            }
          ]
        },
        "flowProperties": [],
        "typeOfFlow": "Other flow",
        "classification": {
          "classHierarchy": "Gr\u00f6\u00dfen / Umweltliche Gr\u00f6\u00dfen / EPD EN 15804 / LCI Indikatoren",
          "name": "GaBiCategories"
        }
      },
      {
        "dataSetInternalID": 16,
        "referenceToFlowDataSet": {
          "shortDescription": [
            {
              "value": "Use of renewable primary energy (PERE)",
              "lang": "en"
            },
            {
              "value": "Erneuerbare Prim\u00e4renergie als Energietr\u00e4ger (PERE)",
              "lang": "de"
            },
            {
              "value": "Uso de energ\u00eda primaria renovable excluyendo los recursos de energ\u00eda primaria renovable utilizada como materia prima (PERE)",
              "lang": "es"
            }
          ],
          "type": "flow data set",
          "refObjectId": "20f32be5-0398-4288-9b6d-accddd195317",
          "version": "30.00.000"
        },
        "exchange direction": "INPUT",
        "meanAmount": 0.0,
        "other": {
          "anies": [
            {
              "value": "1340.0",
              "module": "A1-A3"
            },
            {
              "value": "12.7",
              "module": "A4"
            },
            {
              "value": "177.0",
              "module": "A5"
            },
            {
              "value": "0.0",
              "module": "B1"
            },
            {
              "value": "0.0",
              "module": "B2"
            },
            {
              "value": "0.0",
              "module": "B3"
            },
            {
              "value": "0.0",
              "module": "B4"
            },
            {
              "value": "0.0",
              "module": "B5"
            },
            {
              "value": "0.0",
              "module": "B6"
            },
            {
              "value": "0.0",
              "module": "B7"
            },
            {
              "value": "0.832",
              "module": "C1"
            },
            {
              "value": "0.799",
              "module": "C2"
            },
            {
              "value": "3.54",
              "module": "C3"
            },
            {
              "value": "0.0",
              "module": "C4"
            },
            {
              "value": "-75.5",
              "module": "D"
            },
            {
              "name": "referenceToUnitGroupDataSet",
              "value": {
                "shortDescription": [
                  {
                    "value": "MJ"
                  }
                ],
                "type": "unit group data set",
                "refObjectId": "93a60a57-a3c8-11da-a746-0800200c9a66",
                "uri": "../unitgroups/93a60a57-a3c8-11da-a746-0800200c9a66"
              }
            }
          ]
        },
        "flowProperties": [],
        "typeOfFlow": "Other flow",
        "classification": {
          "classHierarchy": "Gr\u00f6\u00dfen / Umweltliche Gr\u00f6\u00dfen / EPD EN 15804 / LCI Indikatoren",
          "name": "GaBiCategories"
        }
      },
      {
        "dataSetInternalID": 17,
        "referenceToFlowDataSet": {
          "shortDescription": [
            {
              "value": "Use of renewable primary energy resources used as raw materials (PERM)",
              "lang": "en"
            },
            {
              "value": "Erneuerbare Prim\u00e4renergie zur stofflichen Nutzung (PERM)",
              "lang": "de"
            },
            {
              "value": "Uso de energ\u00eda primaria renovable utilizada como materia prima (PERM)",
              "lang": "es"
            }
          ],
          "type": "flow data set",
          "refObjectId": "fb3ec0de-548d-4508-aea5-00b73bf6f702",
          "version": "30.00.000"
        },
        "exchange direction": "INPUT",
        "meanAmount": 0.0,
        "other": {
          "anies": [
            {
              "value": "81.7",
              "module": "A1-A3"
            },
            {
              "value": "0.0",
              "module": "A4"
            },
            {
              "value": "-20.6",
              "module": "A5"
            },
            {
              "value": "0.0",
              "module": "B1"
            },
            {
              "value": "0.0",
              "module": "B2"
            },
            {
              "value": "0.0",
              "module": "B3"
            },
            {
              "value": "0.0",
              "module": "B4"
            },
            {
              "value": "0.0",
              "module": "B5"
            },
            {
              "value": "0.0",
              "module": "B6"
            },
            {
              "value": "0.0",
              "module": "B7"
            },
            {
              "value": "0.0",
              "module": "C1"
            },
            {
              "value": "0.0",
              "module": "C2"
            },
            {
              "value": "0.0",
              "module": "C3"
            },
            {
              "value": "0.0",
              "module": "C4"
            },
            {
              "value": "0.0",
              "module": "D"
            },
            {
              "name": "referenceToUnitGroupDataSet",
              "value": {
                "shortDescription": [
                  {
                    "value": "MJ"
                  }
                ],
                "type": "unit group data set",
                "refObjectId": "93a60a57-a3c8-11da-a746-0800200c9a66",
                "uri": "../unitgroups/93a60a57-a3c8-11da-a746-0800200c9a66"
              }
            }
          ]
        },
        "flowProperties": [],
        "typeOfFlow": "Other flow",
        "classification": {
          "classHierarchy": "Gr\u00f6\u00dfen / Umweltliche Gr\u00f6\u00dfen / EPD EN 15804 / LCI Indikatoren",
          "name": "GaBiCategories"
        }
      },
      {
        "dataSetInternalID": 18,
        "referenceToFlowDataSet": {
          "shortDescription": [
            {
              "value": "Use of renewable secondary fuels (RSF)",
              "lang": "en"
            },
            {
              "value": "Erneuerbare Sekund\u00e4rbrennstoffe (RSF)",
              "lang": "de"
            },
            {
              "value": "Uso de combustibles secundarios renovables (RSF)",
              "lang": "es"
            }
          ],
          "type": "flow data set",
          "refObjectId": "64333088-a55f-4aa2-9a31-c10b07816787",
          "version": "30.00.000"
        },
        "exchange direction": "INPUT",
        "meanAmount": 0.0,
        "other": {
          "anies": [
            {
              "value": "9.3E-11",
              "module": "A1-A3"
            },
            {
              "value": "0.0",
              "module": "A4"
            },
            {
              "value": "9.23E-23",
              "module": "A5"
            },
            {
              "value": "0.0",
              "module": "B1"
            },
            {
              "value": "0.0",
              "module": "B2"
            },
            {
              "value": "0.0",
              "module": "B3"
            },
            {
              "value": "0.0",
              "module": "B4"
            },
            {
              "value": "0.0",
              "module": "B5"
            },
            {
              "value": "0.0",
              "module": "B6"
            },
            {
              "value": "0.0",
              "module": "B7"
            },
            {
              "value": "0.0",
              "module": "C1"
            },
            {
              "value": "0.0",
              "module": "C2"
            },
            {
              "value": "0.0",
              "module": "C3"
            },
            {
              "value": "0.0",
              "module": "C4"
            },
            {
              "value": "-1.17E-22",
              "module": "D"
            },
            {
              "name": "referenceToUnitGroupDataSet",
              "value": {
                "shortDescription": [
                  {
                    "value": "MJ"
                  }
                ],
                "type": "unit group data set",
                "refObjectId": "93a60a57-a3c8-11da-a746-0800200c9a66",
                "uri": "../unitgroups/93a60a57-a3c8-11da-a746-0800200c9a66"
              }
            }
          ]
        },
        "flowProperties": [],
        "typeOfFlow": "Other flow",
        "classification": {
          "classHierarchy": "Gr\u00f6\u00dfen / Umweltliche Gr\u00f6\u00dfen / EPD EN 15804 / LCI Indikatoren",
          "name": "GaBiCategories"
        }
      },
      {
        "dataSetInternalID": 19,
        "referenceToFlowDataSet": {
          "shortDescription": [
            {
              "value": "Use of secondary material (SM)",
              "lang": "en"
            },
            {
              "value": "Einsatz von Sekund\u00e4rstoffen (SM)",
              "lang": "de"
            },
            {
              "value": "Uso de materiales secundarios (SM)",
              "lang": "es"
            }
          ],
          "type": "flow data set",
          "refObjectId": "c6a1f35f-2d09-4f54-8dfb-97e502e1ce92",
          "version": "30.00.000"
        },
        "exchange direction": "INPUT",
        "meanAmount": 0.0,
        "other": {
          "anies": [
            {
              "value": "0.0",
              "module": "A1-A3"
            },
            {
              "value": "0.0",
              "module": "A4"
            },
            {
              "value": "0.0",
              "module": "A5"
            },
            {
              "value": "0.0",
              "module": "B1"
            },
            {
              "value": "0.0",
              "module": "B2"
            },
            {
              "value": "0.0",
              "module": "B3"
            },
            {
              "value": "0.0",
              "module": "B4"
            },
            {
              "value": "0.0",
              "module": "B5"
            },
            {
              "value": "0.0",
              "module": "B6"
            },
            {
              "value": "0.0",
              "module": "B7"
            },
            {
              "value": "0.0",
              "module": "C1"
            },
            {
              "value": "0.0",
              "module": "C2"
            },
            {
              "value": "0.0",
              "module": "C3"
            },
            {
              "value": "0.0",
              "module": "C4"
            },
            {
              "value": "4.41",
              "module": "D"
            },
            {
              "name": "referenceToUnitGroupDataSet",
              "value": {
                "shortDescription": [
                  {
                    "value": "kg"
                  }
                ],
                "type": "unit group data set",
                "refObjectId": "ad38d542-3fe9-439d-9b95-2f5f7752acaf",
                "uri": "../unitgroups/ad38d542-3fe9-439d-9b95-2f5f7752acaf"
              }
            }
          ]
        },
        "flowProperties": [],
        "typeOfFlow": "Other flow",
        "classification": {
          "classHierarchy": "Gr\u00f6\u00dfen / Umweltliche Gr\u00f6\u00dfen / EPD EN 15804 / LCI Indikatoren",
          "name": "GaBiCategories"
        }
      }
    ]
  },
  "LCIAResults": {
    "LCIAResult": [
      {
        "referenceToLCIAMethodDataSet": {
          "shortDescription": [
            {
              "value": "Abiotic depletion potential for fossil resources (ADPF)",
              "lang": "en"
            },
            {
              "value": "Potenzial f\u00fcr den abiotischen Abbau fossiler Brennstoffe (ADPF)",
              "lang": "de"
            },
            {
              "value": "Potencial de agotamiento de recursos abi\u00f3ticos para recursos f\u00f3siles (ADPF)",
              "lang": "es"
            }
          ],
          "type": "LCIA method data set",
          "refObjectId": "804ebcdf-309d-4098-8ed8-fdaf2f389981",
          "version": "00.01.000"
        },
        "meanAmount": 0.0,
        "other": {
          "anies": [
            {
              "value": "16100.0",
              "module": "A1-A3"
            },
            {
              "value": "275.0",
              "module": "A4"
            },
            {
              "value": "2840.0",
              "module": "A5"
            },
            {
              "value": "0.0",
              "module": "B1"
            },
            {
              "value": "0.0",
              "module": "B2"
            },
            {
              "value": "0.0",
              "module": "B3"
            },
            {
              "value": "0.0",
              "module": "B4"
            },
            {
              "value": "0.0",
              "module": "B5"
            },
            {
              "value": "0.0",
              "module": "B6"
            },
            {
              "value": "0.0",
              "module": "B7"
            },
            {
              "value": "1.23",
              "module": "C1"
            },
            {
              "value": "13.7",
              "module": "C2"
            },
            {
              "value": "29.0",
              "module": "C3"
            },
            {
              "value": "0.0",
              "module": "C4"
            },
            {
              "value": "-671.0",
              "module": "D"
            },
            {
              "name": "referenceToUnitGroupDataSet",
              "value": {
                "shortDescription": [
                  {
                    "value": "MJ"
                  }
                ],
                "type": "unit group data set",
                "refObjectId": "93a60a57-a3c8-11da-a746-0800200c9a66",
                "uri": "../unitgroups/93a60a57-a3c8-11da-a746-0800200c9a66"
              }
            }
          ]
        }
      },
      {
        "referenceToLCIAMethodDataSet": {
          "shortDescription": [
            {
              "value": "Abiotic depletion potential for non fossil resources (ADPE)",
              "lang": "en"
            },
            {
              "value": "Potenzial f\u00fcr den abiotischen Abbau nicht fossiler Ressourcen (ADPE)",
              "lang": "de"
            },
            {
              "value": "Potencial de agotamiento de recursos abi\u00f3ticos para recursos no f\u00f3siles (ADPE)",
              "lang": "es"
            }
          ],
          "type": "LCIA method data set",
          "refObjectId": "f7c73bb9-ab1a-4249-9c6d-379a0de6f67e",
          "version": "00.01.000"
        },
        "meanAmount": 0.0,
        "other": {
          "anies": [
            {
              "value": "0.00386",
              "module": "A1-A3"
            },
            {
              "value": "1.48E-6",
              "module": "A4"
            },
            {
              "value": "1.76E-5",
              "module": "A5"
            },
            {
              "value": "0.0",
              "module": "B1"
            },
            {
              "value": "0.0",
              "module": "B2"
            },
            {
              "value": "0.0",
              "module": "B3"
            },
            {
              "value": "0.0",
              "module": "B4"
            },
            {
              "value": "0.0",
              "module": "B5"
            },
            {
              "value": "0.0",
              "module": "B6"
            },
            {
              "value": "0.0",
              "module": "B7"
            },
            {
              "value": "3.64E-8",
              "module": "C1"
            },
            {
              "value": "7.8E-8",
              "module": "C2"
            },
            {
              "value": "8.99E-7",
              "module": "C3"
            },
            {
              "value": "0.0",
              "module": "C4"
            },
            {
              "value": "-1.69E-5",
              "module": "D"
            },
            {
              "name": "referenceToUnitGroupDataSet",
              "value": {
                "shortDescription": [
                  {
                    "value": "kg Sb-\u00c4qv."
                  }
                ],
                "type": "unit group data set",
                "refObjectId": "54ccd2d9-a32a-4fc2-923d-f2c8c93e89d4",
                "uri": "../unitgroups/54ccd2d9-a32a-4fc2-923d-f2c8c93e89d4"
              }
            }
          ]
        }
      },
      {
        "referenceToLCIAMethodDataSet": {
          "shortDescription": [
            {
              "value": "Acidification potential of soil and water (AP)",
              "lang": "en"
            },
            {
              "value": "Versauerungspotenzial von Boden und Wasser (AP)",
              "lang": "de"
            },
            {
              "value": "Potencial de acidificaci\u00f3n del suelo y de los recursos de agua (AP)",
              "lang": "es"
            }
          ],
          "type": "LCIA method data set",
          "refObjectId": "b4274add-93b7-4905-a5e4-2e878c4e4216",
          "version": "00.01.000"
        },
        "meanAmount": 0.0,
        "other": {
          "anies": [
            {
              "value": "1.05",
              "module": "A1-A3"
            },
            {
              "value": "0.182",
              "module": "A4"
            },
            {
              "value": "1.4",
              "module": "A5"
            },
            {
              "value": "0.0",
              "module": "B1"
            },
            {
              "value": "0.0",
              "module": "B2"
            },
            {
              "value": "0.0",
              "module": "B3"
            },
            {
              "value": "0.0",
              "module": "B4"
            },
            {
              "value": "0.0",
              "module": "B5"
            },
            {
              "value": "0.0",
              "module": "B6"
            },
            {
              "value": "0.0",
              "module": "B7"
            },
            {
              "value": "3.24E-4",
              "module": "C1"
            },
            {
              "value": "8.15E-4",
              "module": "C2"
            },
            {
              "value": "0.00621",
              "module": "C3"
            },
            {
              "value": "0.0",
              "module": "C4"
            },
            {
              "value": "-0.0495",
              "module": "D"
            },
            {
              "name": "referenceToUnitGroupDataSet",
              "value": {
                "shortDescription": [
                  {
                    "value": "kg SO2-\u00c4qv."
                  }
                ],
                "type": "unit group data set",
                "refObjectId": "bc50c624-a9bc-45b1-a9b0-e6b10d00476f",
                "uri": "../unitgroups/bc50c624-a9bc-45b1-a9b0-e6b10d00476f"
              }
            }
          ]
        }
      },
      {
        "referenceToLCIAMethodDataSet": {
          "shortDescription": [
            {
              "value": "Eutrophication potential (EP)",
              "lang": "en"
            },
            {
              "value": "Eutrophierungspotenzial (EP)",
              "lang": "de"
            },
            {
              "value": "Potencial de eutrofizaci\u00f3n (EP)",
              "lang": "es"
            }
          ],
          "type": "LCIA method data set",
          "refObjectId": "f58827d0-b407-4ec6-be75-8b69efb98a0f",
          "version": "00.01.000"
        },
        "meanAmount": 0.0,
        "other": {
          "anies": [
            {
              "value": "0.118",
              "module": "A1-A3"
            },
            {
              "value": "0.021",
              "module": "A4"
            },
            {
              "value": "0.281",
              "module": "A5"
            },
            {
              "value": "0.0",
              "module": "B1"
            },
            {
              "value": "0.0",
              "module": "B2"
            },
            {
              "value": "0.0",
              "module": "B3"
            },
            {
              "value": "0.0",
              "module": "B4"
            },
            {
              "value": "0.0",
              "module": "B5"
            },
            {
              "value": "0.0",
              "module": "B6"
            },
            {
              "value": "0.0",
              "module": "B7"
            },
            {
              "value": "3.04E-5",
              "module": "C1"
            },
            {
              "value": "1.8E-4",
              "module": "C2"
            },
            {
              "value": "0.00108",
              "module": "C3"
            },
            {
              "value": "0.0",
              "module": "C4"
            },
            {
              "value": "-0.00559",
              "module": "D"
            },
            {
              "name": "referenceToUnitGroupDataSet",
              "value": {
                "shortDescription": [
                  {
                    "value": "kg Phosphat-\u00c4qv."
                  }
                ],
                "type": "unit group data set",
                "refObjectId": "67b5401d-873c-485f-bcf3-6ae83b918822",
                "uri": "../unitgroups/67b5401d-873c-485f-bcf3-6ae83b918822"
              }
            }
          ]
        }
      },
      {
        "referenceToLCIAMethodDataSet": {
          "shortDescription": [
            {
              "value": "Global warming potential (GWP)",
              "lang": "en"
            },
            {
              "value": "Globales Erw\u00e4rmungspotenzial (GWP)",
              "lang": "de"
            },
            {
              "value": "Potencial de calentamiento global (GWP)",
              "lang": "es"
            }
          ],
          "type": "LCIA method data set",
          "refObjectId": "77e416eb-a363-4258-a04e-171d843a6460",
          "version": "00.01.000"
        },
        "meanAmount": 0.0,
        "other": {
          "anies": [
            {
              "value": "479.0",
              "module": "A1-A3"
            },
            {
              "value": "20.8",
              "module": "A4"
            },
            {
              "value": "207.0",
              "module": "A5"
            },
            {
              "value": "0.0",
              "module": "B1"
            },
            {
              "value": "0.0",
              "module": "B2"
            },
            {
              "value": "0.0",
              "module": "B3"
            },
            {
              "value": "0.0",
              "module": "B4"
            },
            {
              "value": "0.0",
              "module": "B5"
            },
            {
              "value": "0.0",
              "module": "B6"
            },
            {
              "value": "0.0",
              "module": "B7"
            },
            {
              "value": "0.114",
              "module": "C1"
            },
            {
              "value": "1.01",
              "module": "C2"
            },
            {
              "value": "17.7",
              "module": "C3"
            },
            {
              "value": "0.0",
              "module": "C4"
            },
            {
              "value": "-26.7",
              "module": "D"
            },
            {
              "name": "referenceToUnitGroupDataSet",
              "value": {
                "shortDescription": [
                  {
                    "value": "kg CO2-\u00c4qv."
                  }
                ],
                "type": "unit group data set",
                "refObjectId": "1ebf3012-d0db-4de2-aefd-ef30cedb0be1",
                "uri": "../unitgroups/1ebf3012-d0db-4de2-aefd-ef30cedb0be1"
              }
            }
          ]
        }
      },
      {
        "referenceToLCIAMethodDataSet": {
          "shortDescription": [
            {
              "value": "Depletion potential of the stratospheric ozone layer (ODP)",
              "lang": "en"
            },
            {
              "value": "Abbau Potential der stratosph\u00e4rischen Ozonschicht (ODP)",
              "lang": "de"
            },
            {
              "value": "Potencial de agotamiento de la capa de ozono estratosf\u00e9rico (ODP)",
              "lang": "es"
            }
          ],
          "type": "LCIA method data set",
          "refObjectId": "06dcd26f-025f-401a-a7c1-5e457eb54637",
          "version": "00.01.000"
        },
        "meanAmount": 0.0,
        "other": {
          "anies": [
            {
              "value": "2.03E-10",
              "module": "A1-A3"
            },
            {
              "value": "4.49E-15",
              "module": "A4"
            },
            {
              "value": "2.97E-12",
              "module": "A5"
            },
            {
              "value": "0.0",
              "module": "B1"
            },
            {
              "value": "0.0",
              "module": "B2"
            },
            {
              "value": "0.0",
              "module": "B3"
            },
            {
              "value": "0.0",
              "module": "B4"
            },
            {
              "value": "0.0",
              "module": "B5"
            },
            {
              "value": "0.0",
              "module": "B6"
            },
            {
              "value": "0.0",
              "module": "B7"
            },
            {
              "value": "3.2E-15",
              "module": "C1"
            },
            {
              "value": "1.67E-16",
              "module": "C2"
            },
            {
              "value": "6.33E-15",
              "module": "C3"
            },
            {
              "value": "0.0",
              "module": "C4"
            },
            {
              "value": "-2.62E-12",
              "module": "D"
            },
            {
              "name": "referenceToUnitGroupDataSet",
              "value": {
                "shortDescription": [
                  {
                    "value": "kg R11-\u00c4qv."
                  }
                ],
                "type": "unit group data set",
                "refObjectId": "88054749-b0a6-47ea-a82b-dc5b29326512",
                "uri": "../unitgroups/88054749-b0a6-47ea-a82b-dc5b29326512"
              }
            }
          ]
        }
      },
      {
        "referenceToLCIAMethodDataSet": {
          "shortDescription": [
            {
              "value": "Formation potential of tropospheric ozone (POCP)",
              "lang": "en"
            },
            {
              "value": "Bildungspotential f\u00fcr troposph\u00e4risches Ozon (POCP)",
              "lang": "de"
            },
            {
              "value": "Potencial de formaci\u00f3n de ozono troposf\u00e9rico (POCP)",
              "lang": "es"
            }
          ],
          "type": "LCIA method data set",
          "refObjectId": "1e84a202-dae6-42aa-9e9d-71ea48b8be00",
          "version": "00.01.000"
        },
        "meanAmount": 0.0,
        "other": {
          "anies": [
            {
              "value": "0.163",
              "module": "A1-A3"
            },
            {
              "value": "0.00917",
              "module": "A4"
            },
            {
              "value": "0.12",
              "module": "A5"
            },
            {
              "value": "0.0",
              "module": "B1"
            },
            {
              "value": "0.0",
              "module": "B2"
            },
            {
              "value": "0.0",
              "module": "B3"
            },
            {
              "value": "0.0",
              "module": "B4"
            },
            {
              "value": "0.0",
              "module": "B5"
            },
            {
              "value": "0.0",
              "module": "B6"
            },
            {
              "value": "0.0",
              "module": "B7"
            },
            {
              "value": "2.06E-5",
              "module": "C1"
            },
            {
              "value": "2.12E-5",
              "module": "C2"
            },
            {
              "value": "5.91E-4",
              "module": "C3"
            },
            {
              "value": "0.0",
              "module": "C4"
            },
            {
              "value": "-0.00696",
              "module": "D"
            },
            {
              "name": "referenceToUnitGroupDataSet",
              "value": {
                "shortDescription": [
                  {
                    "value": "kg Ethen-\u00c4qv."
                  }
                ],
                "type": "unit group data set",
                "refObjectId": "01c26c17-9a76-406e-8295-f17b55fd909e",
                "uri": "../unitgroups/01c26c17-9a76-406e-8295-f17b55fd909e"
              }
            }
          ]
        }
      }
    ]
  },
  "otherAttributes": {
    "{http://www.okworx.com/ILCD/Extensions/2018/Profile}profile": "EN_15804",
    "{http://www.indata.network/EPD/2019}epd-version": "1.2"
  },
  "version": "1.1",
  "source": "https://node.epditaly.it/resource/datastocks/24493f94-1ca8-4cc7-a056-67cbe25aef5a/processes/0f3ae6eb-563f-471b-810a-a018cec5bc34"
}