{
  "processInformation": {
    "dataSetInformation": {
      "UUID": "7b21d245-2b65-41d0-ba30-9b2585402b20",
      "name": {
        "baseName": [
          {
            "value": "COILS",
            "lang": "en"
          }
        ]
      },
      "generalComment": [
        {
          "value": "Data quality has been assessed and validated during data collection process.\n\nAccording to ISO 14040 and 14044, allocation is avoided whenever possible\nby dividing the system into sub-systems.\n\nAccording to EN:15804 the applied cut-off criterion for mass and energy\nflows is 1%.\n",
          "lang": "en"
        }
      ]
    },
    "quantitativeReference": {
      "referenceToReferenceFlow": [
        1
      ],
      "type": "Reference flow(s)"
    },
    "time": {
      "referenceYear": 2023,
      "dataSetValidUntil": 2028,
      "other": {
        "anies": [
          {
            "name": "publicationDateOfEPD",
            "value": 1690156800000
          }
        ]
      }
    },
    "geography": {
      "locationOfOperationSupplyOrProduction": {
        "descriptionOfRestrictions": [
          {
            "value": "global",
            "lang": "en"
          }
        ],
        "location": "IT"
      }
    },
    "technology": {
      "technologyDescriptionAndIncludedProcesses": [
        {
          "value": "\"Typical Tensile stress: Rm < 420 MPa\nStriction: Z > 70%\nSuccessful in tensile test\"\n",
          "lang": "en"
        }
      ],
      "technologicalApplicability": [
        {
          "value": "\"Dry cold or bath drawing makes it possible to obtain thin\nwires with diameters under a millimetre.\nAccording to the different grades, wire rod can be\nconverted into ribbed wires suitable for producing welded\nmesh for the construction industry, either in standard\nformat or to measure, or polished and zinc-plated wires\nused in agriculture and for special fencing.\"\n \"Coils: Diameters from 5,5 mm to 13,5 mm\nWeight from 1 800 to 2 100 kg\"",
          "lang": "en"
        }
      ]
    }
  },
  "modellingAndValidation": {
    "LCIMethodAndAllocation": {
      "typeOfDataSet": "EPD",
      "referenceToLCAMethodDetails": [
        {
          "shortDescription": [
            {
              "value": "PCR ICMQ 3.0 - rev. 3.0 - Products and services for construction",
              "lang": "en"
            }
          ],
          "type": "source data set",
          "refObjectId": "cf07c2df-2905-44f9-b3b7-6cedd92fbdeb",
          "version": "00.00.000"
        }
      ],
      "other": {
        "anies": [
          {
            "name": "subType",
            "value": "specific dataset"
          }
        ]
      }
    },
    "dataSourcesTreatmentAndRepresentativeness": {
      "referenceToDataSource": [
        {
          "shortDescription": [
            {
              "value": "ecoinvent database (all versions)",
              "lang": "en"
            }
          ],
          "type": "source data set",
          "refObjectId": "b497a91f-e14b-4b69-8f28-f50eb1576766",
          "version": "00.03.001",
          "uri": "http://openlca.org/ilcd/resource/sources/b497a91f-e14b-4b69-8f28-f50eb1576766"
        }
      ],
      "useAdviceForDataSet": [
        {
          "value": "cradle to gate with options: A1, A2, A3, A4, C1, C2, C3, C4, D\n",
          "lang": "en"
        }
      ],
      "other": {
        "anies": [
          {
            "name": "referenceToOriginalEPD",
            "value": {
              "shortDescription": {},
              "version": {
                "version": 0,
                "majorVersion": 0,
                "minorVersion": 0,
                "subMinorVersion": 0,
                "zero": true,
                "versionString": "00.00.000"
              },
              "type": "source data set",
              "uuid": {
                "uuid": "11f00bf1-5bcf-46e7-a1fb-188068bc0e87"
              },
              "refObjectId": "11f00bf1-5bcf-46e7-a1fb-188068bc0e87",
              "versionAsString": "00.00.000",
              "resourceURLs": [
                "https://node.epditaly.it/resource/sources/11f00bf1-5bcf-46e7-a1fb-188068bc0e87/https://www.epditaly.it/en/wp-content/uploads/2016/12/Feralpi_hot_2023_coils_EPDIT.pdf?version=00.00.000"
              ]
            }
          }
        ]
      }
    },
    "validation": {
      "review": [
        {
          "referenceToNameOfReviewerAndInstitution": [
            {
              "shortDescription": [
                {
                  "value": "ICMQ spa",
                  "lang": "en"
                }
              ],
              "type": "contact data set",
              "refObjectId": "cbb9d118-f872-4b99-920a-b1078fce25da",
              "version": "00.00.001"
            }
          ],
          "type": "Independent external review"
        }
      ]
    },
    "complianceDeclarations": {
      "compliance": [
        {
          "referenceToComplianceSystem": {
            "shortDescription": [
              {
                "value": "EN 15804+A2",
                "lang": "en"
              }
            ],
            "type": "source data set",
            "refObjectId": "c0016b33-8cf7-415c-ac6e-deba0d21440d",
            "version": "00.02.000"
          },
          "approvalOfOverallCompliance": "Fully compliant",
          "nomenclatureCompliance": "Fully compliant",
          "methodologicalCompliance": "Fully compliant",
          "reviewCompliance": "Fully compliant",
          "documentationCompliance": "Fully compliant",
          "qualityCompliance": "Fully compliant"
        },
        {
          "referenceToComplianceSystem": {
            "shortDescription": [
              {
                "value": "ISO 14025",
                "lang": "en"
              }
            ],
            "type": "source data set",
            "refObjectId": "4f2eb655-6e44-4874-a95a-e28f5442cd4d",
            "version": "00.00.001"
          },
          "approvalOfOverallCompliance": "Fully compliant",
          "nomenclatureCompliance": "Fully compliant",
          "methodologicalCompliance": "Fully compliant",
          "reviewCompliance": "Fully compliant",
          "documentationCompliance": "Fully compliant",
          "qualityCompliance": "Fully compliant"
        },
        {
          "referenceToComplianceSystem": {
            "shortDescription": [
              {
                "value": "ISO 21930",
                "lang": "en"
              }
            ],
            "type": "source data set",
            "refObjectId": "9c1e8451-2321-4498-b459-b6568b6b6547",
            "version": "00.00.001"
          },
          "approvalOfOverallCompliance": "Fully compliant",
          "nomenclatureCompliance": "Fully compliant",
          "methodologicalCompliance": "Fully compliant",
          "reviewCompliance": "Fully compliant",
          "documentationCompliance": "Fully compliant",
          "qualityCompliance": "Fully compliant"
        }
      ]
    }
  },
  "administrativeInformation": {
    "dataGenerator": {
      "referenceToPersonOrEntityGeneratingTheDataSet": [
        {
          "shortDescription": [
            {
              "value": "LCA.no AS",
              "lang": "en"
            }
          ],
          "type": "contact data set",
          "refObjectId": "77a6868e-b256-47c8-a410-32706b6e1814",
          "version": "00.00.001"
        }
      ]
    },
    "dataEntryBy": {
      "timeStamp": 1701253499000,
      "referenceToDataSetFormat": [
        {
          "shortDescription": [
            {
              "value": "ILCD format",
              "lang": "en"
            }
          ],
          "type": "source data set",
          "refObjectId": "a97a0155-0234-4b87-b4ce-a45da52f2a40",
          "version": "01.00.000",
          "uri": "http://lca.jrc.ec.europa.eu/lcainfohub/sample_data/ilcd/sources/ILCD_Format_a97a0155-0234-4b87-b4ce-a45da52f2a40_01.00.000.xml"
        },
        {
          "shortDescription": [
            {
              "value": "EPD Data Format Extensions v1.2",
              "lang": "no"
            },
            {
              "value": "EPD Data Format Extensions v1.2",
              "lang": "en"
            },
            {
              "value": "EPD-Datenformaterweiterungen v1.2",
              "lang": "de"
            }
          ],
          "type": "source data set",
          "refObjectId": "a29449fd-aa2f-4de8-b5d7-4b06b43c6fde",
          "version": "00.01.000"
        }
      ]
    },
    "publicationAndOwnership": {
      "dataSetVersion": "00.03.000",
      "dateOfLastRevision": 1701170727413,
      "referenceToRegistrationAuthority": {
        "shortDescription": [
          {
            "value": "EPDItaly",
            "lang": "en"
          }
        ],
        "type": "contact data set",
        "refObjectId": "9433b9cf-1d4a-420f-8c09-88d2472225b9",
        "version": "00.00.004"
      },
      "registrationNumber": "EPDITALY0497",
      "referenceToOwnershipOfDataSet": {
        "shortDescription": [
          {
            "value": "FERALPI SIDERURGICA SPA - FERALPI GROUP",
            "lang": "en"
          }
        ],
        "type": "contact data set",
        "refObjectId": "2773bb94-2048-4b67-a02c-a3c5b98124c5",
        "version": "00.00.000"
      },
      "copyright": true,
      "licenseType": "Free of charge for all users and uses",
      "accessRestrictions": [
        {
          "value": "None",
          "lang": "en"
        }
      ],
      "other": {
        "anies": [
          {
            "name": "referenceToPublisher",
            "value": {
              "shortDescription": [
                {
                  "value": "EPDItaly",
                  "lang": "en"
                }
              ],
              "type": "contact data set",
              "refObjectId": "9433b9cf-1d4a-420f-8c09-88d2472225b9",
              "version": "00.00.004"
            }
          }
        ]
      }
    }
  },
  "exchanges": {
    "exchange": [
      {
        "dataSetInternalID": 1,
        "referenceToFlowDataSet": {
          "shortDescription": [
            {
              "value": "COILS",
              "lang": "en"
            }
          ],
          "type": "flow data set",
          "refObjectId": "049dbbb8-a3a4-4798-bbcc-441f371d4e36",
          "version": "00.01.000"
        },
        "exchange direction": "OUTPUT",
        "meanAmount": 1.0,
        "resultingAmount": 1.0,
        "minimumAmount": 0.0,
        "maximumAmount": 0.0,
        "uncertaintyDistributionType": "UNDEFINED",
        "relativeStandardDeviation95In": "0",
        "dataSourceType": "Primary",
        "dataDerivationTypeStatus": "MEASURED",
        "referenceFlow": true,
        "resultingflowAmount": 1000.0,
        "flowProperties": [
          {
            "name": [
              {
                "lang": "no",
                "value": "Innhold av biogent karbon i emballasjen"
              },
              {
                "lang": "en",
                "value": "Carbon content (biogenic) - packaging"
              }
            ],
            "uuid": "262a541b-209e-44cc-a426-33bce30de7b1",
            "meanValue": 1.0
          },
          {
            "name": [
              {
                "lang": "no",
                "value": "Innhold av biogent karbon i produkt"
              },
              {
                "lang": "en",
                "value": "Carbon content (biogenic)"
              }
            ],
            "uuid": "62e503ce-544a-4599-b2ad-bcea15a7bf20",
            "meanValue": 1.0
          },
          {
            "name": [
              {
                "lang": "en",
                "value": "Mass"
              },
              {
                "lang": "de",
                "value": "Masse"
              }
            ],
            "uuid": "93a60a56-a3c8-11da-a746-0800200b9a66",
            "referenceFlowProperty": true,
            "meanValue": 1000.0,
            "referenceUnit": "kg",
            "unitGroupUUID": "ad38d542-3fe9-439d-9b95-2f5f7752acaf"
          }
        ],
        "typeOfFlow": "Product flow"
      },
      {
        "dataSetInternalID": 2,
        "referenceToFlowDataSet": {
          "shortDescription": [
            {
              "value": "Use of renewable primary energy (PERE)",
              "lang": "en"
            },
            {
              "value": "Fornybar prim\u00e6renergi brukt som energib\u00e6rer (RPEE)",
              "lang": "no"
            }
          ],
          "type": "flow data set",
          "refObjectId": "20f32be5-0398-4288-9b6d-accddd195317",
          "version": "30.00.000"
        },
        "exchange direction": "INPUT",
        "meanAmount": 0.0,
        "resultingAmount": 0.0,
        "minimumAmount": 0.0,
        "maximumAmount": 0.0,
        "uncertaintyDistributionType": "UNDEFINED",
        "relativeStandardDeviation95In": "0",
        "dataSourceType": "Primary",
        "dataDerivationTypeStatus": "MEASURED",
        "other": {
          "anies": [
            {
              "value": "0.000000000000",
              "module": "A1"
            },
            {
              "value": "0.000000000000",
              "module": "A2"
            },
            {
              "value": "0.000000000000",
              "module": "A3"
            },
            {
              "value": "0.000000000000",
              "module": "A4"
            },
            {
              "value": "0.000000000000",
              "module": "C1"
            },
            {
              "value": "0.000000000000",
              "module": "C2"
            },
            {
              "value": "0.000000000000",
              "module": "C3"
            },
            {
              "value": "0.000000000000",
              "module": "C4"
            },
            {
              "value": "0.000000000000",
              "module": "D"
            },
            {
              "name": "referenceToUnitGroupDataSet",
              "value": {
                "shortDescription": [
                  {
                    "value": "MJ"
                  }
                ],
                "type": "unit group data set",
                "refObjectId": "93a60a57-a3c8-11da-a746-0800200c9a66",
                "uri": "../unitgroups/93a60a57-a3c8-11da-a746-0800200c9a66"
              }
            }
          ]
        },
        "flowProperties": [],
        "typeOfFlow": "Other flow",
        "classification": {
          "classHierarchy": "Gr\u00f6\u00dfen / Umweltliche Gr\u00f6\u00dfen / EPD EN 15804 / LCI Indikatoren",
          "name": "GaBiCategories"
        }
      },
      {
        "dataSetInternalID": 3,
        "referenceToFlowDataSet": {
          "shortDescription": [
            {
              "value": "Use of renewable primary energy resources used as raw materials (PERM)",
              "lang": "en"
            },
            {
              "value": "Fornybar prim\u00e6renergi brukt som energib\u00e6rer (RPEE)",
              "lang": "no"
            }
          ],
          "type": "flow data set",
          "refObjectId": "fb3ec0de-548d-4508-aea5-00b73bf6f702",
          "version": "30.00.000"
        },
        "exchange direction": "INPUT",
        "meanAmount": 0.0,
        "resultingAmount": 0.0,
        "minimumAmount": 0.0,
        "maximumAmount": 0.0,
        "uncertaintyDistributionType": "UNDEFINED",
        "relativeStandardDeviation95In": "0",
        "dataSourceType": "Primary",
        "dataDerivationTypeStatus": "MEASURED",
        "other": {
          "anies": [
            {
              "value": "0.000000000000",
              "module": "A1"
            },
            {
              "value": "0.000000000000",
              "module": "A2"
            },
            {
              "value": "0.000000000000",
              "module": "A3"
            },
            {
              "value": "0.000000000000",
              "module": "A4"
            },
            {
              "value": "0.000000000000",
              "module": "C1"
            },
            {
              "value": "0.000000000000",
              "module": "C2"
            },
            {
              "value": "0.000000000000",
              "module": "C3"
            },
            {
              "value": "0.000000000000",
              "module": "C4"
            },
            {
              "value": "0.000000000000",
              "module": "D"
            },
            {
              "name": "referenceToUnitGroupDataSet",
              "value": {
                "shortDescription": [
                  {
                    "value": "MJ"
                  }
                ],
                "type": "unit group data set",
                "refObjectId": "93a60a57-a3c8-11da-a746-0800200c9a66",
                "uri": "../unitgroups/93a60a57-a3c8-11da-a746-0800200c9a66"
              }
            }
          ]
        },
        "flowProperties": [],
        "typeOfFlow": "Other flow",
        "classification": {
          "classHierarchy": "Gr\u00f6\u00dfen / Umweltliche Gr\u00f6\u00dfen / EPD EN 15804 / LCI Indikatoren",
          "name": "GaBiCategories"
        }
      },
      {
        "dataSetInternalID": 4,
        "referenceToFlowDataSet": {
          "shortDescription": [
            {
              "value": "Total use of renewable primary energy resource (PERT)",
              "lang": "en"
            },
            {
              "value": "Total bruk av fornybar prim\u00e6renergi (TPE)",
              "lang": "no"
            }
          ],
          "type": "flow data set",
          "refObjectId": "53f97275-fa8a-4cdd-9024-65936002acd0",
          "version": "30.00.000"
        },
        "exchange direction": "INPUT",
        "meanAmount": 0.0,
        "resultingAmount": 0.0,
        "minimumAmount": 0.0,
        "maximumAmount": 0.0,
        "uncertaintyDistributionType": "UNDEFINED",
        "relativeStandardDeviation95In": "0",
        "dataSourceType": "Primary",
        "dataDerivationTypeStatus": "MEASURED",
        "other": {
          "anies": [
            {
              "value": "0.000000000000",
              "module": "A1"
            },
            {
              "value": "0.000000000000",
              "module": "A2"
            },
            {
              "value": "0.000000000000",
              "module": "A3"
            },
            {
              "value": "0.000000000000",
              "module": "A4"
            },
            {
              "value": "0.000000000000",
              "module": "C1"
            },
            {
              "value": "0.000000000000",
              "module": "C2"
            },
            {
              "value": "0.000000000000",
              "module": "C3"
            },
            {
              "value": "0.000000000000",
              "module": "C4"
            },
            {
              "value": "0.000000000000",
              "module": "D"
            },
            {
              "name": "referenceToUnitGroupDataSet",
              "value": {
                "shortDescription": [
                  {
                    "value": "MJ"
                  }
                ],
                "type": "unit group data set",
                "refObjectId": "93a60a57-a3c8-11da-a746-0800200c9a66",
                "uri": "../unitgroups/93a60a57-a3c8-11da-a746-0800200c9a66"
              }
            }
          ]
        },
        "flowProperties": [],
        "typeOfFlow": "Other flow",
        "classification": {
          "classHierarchy": "Gr\u00f6\u00dfen / Umweltliche Gr\u00f6\u00dfen / EPD EN 15804 / LCI Indikatoren",
          "name": "GaBiCategories"
        }
      },
      {
        "dataSetInternalID": 5,
        "referenceToFlowDataSet": {
          "shortDescription": [
            {
              "value": "Use of non renewable primary energy (PENRE)",
              "lang": "en"
            },
            {
              "value": "Ikke fornybar prim\u00e6renergi brukt som energib\u00e6rer (NRPE)",
              "lang": "no"
            }
          ],
          "type": "flow data set",
          "refObjectId": "ac857178-2b45-46ec-892a-a9a4332f0372",
          "version": "30.00.000"
        },
        "exchange direction": "INPUT",
        "meanAmount": 0.0,
        "resultingAmount": 0.0,
        "minimumAmount": 0.0,
        "maximumAmount": 0.0,
        "uncertaintyDistributionType": "UNDEFINED",
        "relativeStandardDeviation95In": "0",
        "dataSourceType": "Primary",
        "dataDerivationTypeStatus": "MEASURED",
        "other": {
          "anies": [
            {
              "value": "0.000000000000",
              "module": "A1"
            },
            {
              "value": "0.000000000000",
              "module": "A2"
            },
            {
              "value": "0.000000000000",
              "module": "A3"
            },
            {
              "value": "0.000000000000",
              "module": "A4"
            },
            {
              "value": "0.000000000000",
              "module": "C1"
            },
            {
              "value": "0.000000000000",
              "module": "C2"
            },
            {
              "value": "0.000000000000",
              "module": "C3"
            },
            {
              "value": "0.000000000000",
              "module": "C4"
            },
            {
              "value": "0.000000000000",
              "module": "D"
            },
            {
              "name": "referenceToUnitGroupDataSet",
              "value": {
                "shortDescription": [
                  {
                    "value": "MJ"
                  }
                ],
                "type": "unit group data set",
                "refObjectId": "93a60a57-a3c8-11da-a746-0800200c9a66",
                "uri": "../unitgroups/93a60a57-a3c8-11da-a746-0800200c9a66"
              }
            }
          ]
        },
        "flowProperties": [],
        "typeOfFlow": "Other flow",
        "classification": {
          "classHierarchy": "Gr\u00f6\u00dfen / Umweltliche Gr\u00f6\u00dfen / EPD EN 15804 / LCI Indikatoren",
          "name": "GaBiCategories"
        }
      },
      {
        "dataSetInternalID": 6,
        "referenceToFlowDataSet": {
          "shortDescription": [
            {
              "value": "Use of non renewable primary energy resources used as raw materials (PENRM)",
              "lang": "en"
            },
            {
              "value": "Ikke fornybar prim\u00e6renergi brukt som r\u00e5materiale (NRPM)",
              "lang": "no"
            }
          ],
          "type": "flow data set",
          "refObjectId": "1421caa0-679d-4bf4-b282-0eb850ccae27",
          "version": "30.00.000"
        },
        "exchange direction": "INPUT",
        "meanAmount": 0.0,
        "resultingAmount": 0.0,
        "minimumAmount": 0.0,
        "maximumAmount": 0.0,
        "uncertaintyDistributionType": "UNDEFINED",
        "relativeStandardDeviation95In": "0",
        "dataSourceType": "Primary",
        "dataDerivationTypeStatus": "MEASURED",
        "other": {
          "anies": [
            {
              "value": "0.000000000000",
              "module": "A1"
            },
            {
              "value": "0.000000000000",
              "module": "A2"
            },
            {
              "value": "0.000000000000",
              "module": "A3"
            },
            {
              "value": "0.000000000000",
              "module": "A4"
            },
            {
              "value": "0.000000000000",
              "module": "C1"
            },
            {
              "value": "0.000000000000",
              "module": "C2"
            },
            {
              "value": "0.000000000000",
              "module": "C3"
            },
            {
              "value": "0.000000000000",
              "module": "C4"
            },
            {
              "value": "0.000000000000",
              "module": "D"
            },
            {
              "name": "referenceToUnitGroupDataSet",
              "value": {
                "shortDescription": [
                  {
                    "value": "MJ"
                  }
                ],
                "type": "unit group data set",
                "refObjectId": "93a60a57-a3c8-11da-a746-0800200c9a66",
                "uri": "../unitgroups/93a60a57-a3c8-11da-a746-0800200c9a66"
              }
            }
          ]
        },
        "flowProperties": [],
        "typeOfFlow": "Other flow",
        "classification": {
          "classHierarchy": "Gr\u00f6\u00dfen / Umweltliche Gr\u00f6\u00dfen / EPD EN 15804 / LCI Indikatoren",
          "name": "GaBiCategories"
        }
      },
      {
        "dataSetInternalID": 7,
        "referenceToFlowDataSet": {
          "shortDescription": [
            {
              "value": "Total use of non renewable primary energy resource (PENRT)",
              "lang": "en"
            },
            {
              "value": "Total nicht erneuerbare Prim\u00e4renergie (PENRT)",
              "lang": "no"
            }
          ],
          "type": "flow data set",
          "refObjectId": "06159210-646b-4c8d-8583-da9b3b95a6c1",
          "version": "30.00.000"
        },
        "exchange direction": "INPUT",
        "meanAmount": 0.0,
        "resultingAmount": 0.0,
        "minimumAmount": 0.0,
        "maximumAmount": 0.0,
        "uncertaintyDistributionType": "UNDEFINED",
        "relativeStandardDeviation95In": "0",
        "dataSourceType": "Primary",
        "dataDerivationTypeStatus": "MEASURED",
        "other": {
          "anies": [
            {
              "value": "0.000000000000",
              "module": "A1"
            },
            {
              "value": "0.000000000000",
              "module": "A2"
            },
            {
              "value": "0.000000000000",
              "module": "A3"
            },
            {
              "value": "0.000000000000",
              "module": "A4"
            },
            {
              "value": "0.000000000000",
              "module": "C1"
            },
            {
              "value": "0.000000000000",
              "module": "C2"
            },
            {
              "value": "0.000000000000",
              "module": "C3"
            },
            {
              "value": "0.000000000000",
              "module": "C4"
            },
            {
              "value": "0.000000000000",
              "module": "D"
            },
            {
              "name": "referenceToUnitGroupDataSet",
              "value": {
                "shortDescription": [
                  {
                    "value": "MJ"
                  }
                ],
                "type": "unit group data set",
                "refObjectId": "93a60a57-a3c8-11da-a746-0800200c9a66",
                "uri": "../unitgroups/93a60a57-a3c8-11da-a746-0800200c9a66"
              }
            }
          ]
        },
        "flowProperties": [],
        "typeOfFlow": "Other flow",
        "classification": {
          "classHierarchy": "Gr\u00f6\u00dfen / Umweltliche Gr\u00f6\u00dfen / EPD EN 15804 / LCI Indikatoren",
          "name": "GaBiCategories"
        }
      },
      {
        "dataSetInternalID": 8,
        "referenceToFlowDataSet": {
          "shortDescription": [
            {
              "value": "Use of secondary material (SM)",
              "lang": "en"
            },
            {
              "value": "Bruk av sekund\u00e6re materialer (SM)",
              "lang": "no"
            }
          ],
          "type": "flow data set",
          "refObjectId": "c6a1f35f-2d09-4f54-8dfb-97e502e1ce92",
          "version": "30.00.000"
        },
        "exchange direction": "INPUT",
        "meanAmount": 0.0,
        "resultingAmount": 0.0,
        "minimumAmount": 0.0,
        "maximumAmount": 0.0,
        "uncertaintyDistributionType": "UNDEFINED",
        "relativeStandardDeviation95In": "0",
        "dataSourceType": "Primary",
        "dataDerivationTypeStatus": "MEASURED",
        "other": {
          "anies": [
            {
              "value": "1187.351418949000",
              "module": "A1"
            },
            {
              "value": "0.000000000000",
              "module": "A2"
            },
            {
              "value": "0.000000000000",
              "module": "A3"
            },
            {
              "value": "0.000000000000",
              "module": "A4"
            },
            {
              "value": "0.000000000000",
              "module": "C1"
            },
            {
              "value": "0.000000000000",
              "module": "C2"
            },
            {
              "value": "0.000000000000",
              "module": "C3"
            },
            {
              "value": "0.000000000000",
              "module": "C4"
            },
            {
              "value": "0.000000000000",
              "module": "D"
            },
            {
              "name": "referenceToUnitGroupDataSet",
              "value": {
                "shortDescription": [
                  {
                    "value": "kg"
                  }
                ],
                "type": "unit group data set",
                "refObjectId": "ad38d542-3fe9-439d-9b95-2f5f7752acaf",
                "uri": "../unitgroups/ad38d542-3fe9-439d-9b95-2f5f7752acaf"
              }
            }
          ]
        },
        "flowProperties": [],
        "typeOfFlow": "Other flow",
        "classification": {
          "classHierarchy": "Gr\u00f6\u00dfen / Umweltliche Gr\u00f6\u00dfen / EPD EN 15804 / LCI Indikatoren",
          "name": "GaBiCategories"
        }
      },
      {
        "dataSetInternalID": 9,
        "referenceToFlowDataSet": {
          "shortDescription": [
            {
              "value": "Use of renewable secondary fuels (RSF)",
              "lang": "en"
            },
            {
              "value": "Bruk av fornybart sekund\u00e6re brensel (RSF)",
              "lang": "no"
            }
          ],
          "type": "flow data set",
          "refObjectId": "64333088-a55f-4aa2-9a31-c10b07816787",
          "version": "30.00.000"
        },
        "exchange direction": "INPUT",
        "meanAmount": 0.0,
        "resultingAmount": 0.0,
        "minimumAmount": 0.0,
        "maximumAmount": 0.0,
        "uncertaintyDistributionType": "UNDEFINED",
        "relativeStandardDeviation95In": "0",
        "dataSourceType": "Primary",
        "dataDerivationTypeStatus": "MEASURED",
        "other": {
          "anies": [
            {
              "value": "0.000000000000",
              "module": "A1"
            },
            {
              "value": "0.000000000000",
              "module": "A2"
            },
            {
              "value": "0.000000000000",
              "module": "A3"
            },
            {
              "value": "0.000000000000",
              "module": "A4"
            },
            {
              "value": "0.000000000000",
              "module": "C1"
            },
            {
              "value": "0.000000000000",
              "module": "C2"
            },
            {
              "value": "0.000000000000",
              "module": "C3"
            },
            {
              "value": "0.000000000000",
              "module": "C4"
            },
            {
              "value": "0.000000000000",
              "module": "D"
            },
            {
              "name": "referenceToUnitGroupDataSet",
              "value": {
                "shortDescription": [
                  {
                    "value": "MJ"
                  }
                ],
                "type": "unit group data set",
                "refObjectId": "93a60a57-a3c8-11da-a746-0800200c9a66",
                "uri": "../unitgroups/93a60a57-a3c8-11da-a746-0800200c9a66"
              }
            }
          ]
        },
        "flowProperties": [],
        "typeOfFlow": "Other flow",
        "classification": {
          "classHierarchy": "Gr\u00f6\u00dfen / Umweltliche Gr\u00f6\u00dfen / EPD EN 15804 / LCI Indikatoren",
          "name": "GaBiCategories"
        }
      },
      {
        "dataSetInternalID": 10,
        "referenceToFlowDataSet": {
          "shortDescription": [
            {
              "value": "Use of non renewable secondary fuels (NRSF)",
              "lang": "en"
            },
            {
              "value": "Bruk av ikke fornybart sekund\u00e6re brensel (NRSF)",
              "lang": "no"
            }
          ],
          "type": "flow data set",
          "refObjectId": "89def144-d39a-4287-b86f-efde453ddcb2",
          "version": "30.00.000"
        },
        "exchange direction": "INPUT",
        "meanAmount": 0.0,
        "resultingAmount": 0.0,
        "minimumAmount": 0.0,
        "maximumAmount": 0.0,
        "uncertaintyDistributionType": "UNDEFINED",
        "relativeStandardDeviation95In": "0",
        "dataSourceType": "Primary",
        "dataDerivationTypeStatus": "MEASURED",
        "other": {
          "anies": [
            {
              "value": "0.000000000000",
              "module": "A1"
            },
            {
              "value": "0.000000000000",
              "module": "A2"
            },
            {
              "value": "0.000000000000",
              "module": "A3"
            },
            {
              "value": "0.000000000000",
              "module": "A4"
            },
            {
              "value": "0.000000000000",
              "module": "C1"
            },
            {
              "value": "0.000000000000",
              "module": "C2"
            },
            {
              "value": "0.000000000000",
              "module": "C3"
            },
            {
              "value": "0.000000000000",
              "module": "C4"
            },
            {
              "value": "0.000000000000",
              "module": "D"
            },
            {
              "name": "referenceToUnitGroupDataSet",
              "value": {
                "shortDescription": [
                  {
                    "value": "MJ"
                  }
                ],
                "type": "unit group data set",
                "refObjectId": "93a60a57-a3c8-11da-a746-0800200c9a66",
                "uri": "../unitgroups/93a60a57-a3c8-11da-a746-0800200c9a66"
              }
            }
          ]
        },
        "flowProperties": [],
        "typeOfFlow": "Other flow",
        "classification": {
          "classHierarchy": "Gr\u00f6\u00dfen / Umweltliche Gr\u00f6\u00dfen / EPD EN 15804 / LCI Indikatoren",
          "name": "GaBiCategories"
        }
      },
      {
        "dataSetInternalID": 11,
        "referenceToFlowDataSet": {
          "shortDescription": [
            {
              "value": "Use of net fresh water (FW)",
              "lang": "en"
            },
            {
              "value": "Netto bruk av ferskvann (W)",
              "lang": "no"
            }
          ],
          "type": "flow data set",
          "refObjectId": "3cf952c8-f3a4-461d-8c96-96456ca62246",
          "version": "30.00.000"
        },
        "exchange direction": "INPUT",
        "meanAmount": 0.0,
        "resultingAmount": 0.0,
        "minimumAmount": 0.0,
        "maximumAmount": 0.0,
        "uncertaintyDistributionType": "UNDEFINED",
        "relativeStandardDeviation95In": "0",
        "dataSourceType": "Primary",
        "dataDerivationTypeStatus": "MEASURED",
        "other": {
          "anies": [
            {
              "value": "0.000000000000",
              "module": "A1"
            },
            {
              "value": "0.000000000000",
              "module": "A2"
            },
            {
              "value": "0.000000000000",
              "module": "A3"
            },
            {
              "value": "0.000000000000",
              "module": "A4"
            },
            {
              "value": "0.000000000000",
              "module": "C1"
            },
            {
              "value": "0.000000000000",
              "module": "C2"
            },
            {
              "value": "0.000000000000",
              "module": "C3"
            },
            {
              "value": "0.000000000000",
              "module": "C4"
            },
            {
              "value": "0.000000000000",
              "module": "D"
            },
            {
              "name": "referenceToUnitGroupDataSet",
              "value": {
                "shortDescription": [
                  {
                    "value": "m3"
                  }
                ],
                "type": "unit group data set",
                "refObjectId": "cd950537-0a98-4044-9ba7-9f9a68d0a504",
                "uri": "../unitgroups/cd950537-0a98-4044-9ba7-9f9a68d0a504"
              }
            }
          ]
        },
        "flowProperties": [],
        "typeOfFlow": "Other flow",
        "classification": {
          "classHierarchy": "Gr\u00f6\u00dfen / Umweltliche Gr\u00f6\u00dfen / EPD EN 15804 / LCI Indikatoren",
          "name": "GaBiCategories"
        }
      },
      {
        "dataSetInternalID": 12,
        "referenceToFlowDataSet": {
          "shortDescription": [
            {
              "value": "Hazardous waste disposed (HWD)",
              "lang": "en"
            },
            {
              "value": "Avhendet farlig avfall (HW)",
              "lang": "no"
            }
          ],
          "type": "flow data set",
          "refObjectId": "430f9e0f-59b2-46a0-8e0d-55e0e84948fc",
          "version": "30.00.000"
        },
        "exchange direction": "OUTPUT",
        "meanAmount": 0.0,
        "resultingAmount": 0.0,
        "minimumAmount": 0.0,
        "maximumAmount": 0.0,
        "uncertaintyDistributionType": "UNDEFINED",
        "relativeStandardDeviation95In": "0",
        "dataSourceType": "Primary",
        "dataDerivationTypeStatus": "MEASURED",
        "other": {
          "anies": [
            {
              "value": "0.000000000000",
              "module": "A1"
            },
            {
              "value": "0.000000000000",
              "module": "A2"
            },
            {
              "value": "0.000000000000",
              "module": "A3"
            },
            {
              "value": "0.000000000000",
              "module": "A4"
            },
            {
              "value": "0.000000000000",
              "module": "C1"
            },
            {
              "value": "0.000000000000",
              "module": "C2"
            },
            {
              "value": "0.000000000000",
              "module": "C3"
            },
            {
              "value": "0.000000000000",
              "module": "C4"
            },
            {
              "value": "0.000000000000",
              "module": "D"
            },
            {
              "name": "referenceToUnitGroupDataSet",
              "value": {
                "shortDescription": [
                  {
                    "value": "kg"
                  }
                ],
                "type": "unit group data set",
                "refObjectId": "ad38d542-3fe9-439d-9b95-2f5f7752acaf",
                "uri": "../unitgroups/ad38d542-3fe9-439d-9b95-2f5f7752acaf"
              }
            }
          ]
        },
        "flowProperties": [],
        "typeOfFlow": "Other flow",
        "classification": {
          "classHierarchy": "Gr\u00f6\u00dfen / Umweltliche Gr\u00f6\u00dfen / EPD EN 15804 / LCI Indikatoren",
          "name": "GaBiCategories"
        }
      },
      {
        "dataSetInternalID": 13,
        "referenceToFlowDataSet": {
          "shortDescription": [
            {
              "value": "Non hazardous waste dispose (NHWD)",
              "lang": "en"
            },
            {
              "value": "Avhendet ikke-farlig avfall (NHW)",
              "lang": "no"
            }
          ],
          "type": "flow data set",
          "refObjectId": "b29ef66b-e286-4afa-949f-62f1a7b4d7fa",
          "version": "30.00.000"
        },
        "exchange direction": "OUTPUT",
        "meanAmount": 0.0,
        "resultingAmount": 0.0,
        "minimumAmount": 0.0,
        "maximumAmount": 0.0,
        "uncertaintyDistributionType": "UNDEFINED",
        "relativeStandardDeviation95In": "0",
        "dataSourceType": "Primary",
        "dataDerivationTypeStatus": "MEASURED",
        "other": {
          "anies": [
            {
              "value": "0.000000000000",
              "module": "A1"
            },
            {
              "value": "0.000000000000",
              "module": "A2"
            },
            {
              "value": "0.000000000000",
              "module": "A3"
            },
            {
              "value": "0.000000000000",
              "module": "A4"
            },
            {
              "value": "0.000000000000",
              "module": "C1"
            },
            {
              "value": "0.000000000000",
              "module": "C2"
            },
            {
              "value": "0.000000000000",
              "module": "C3"
            },
            {
              "value": "0.000000000000",
              "module": "C4"
            },
            {
              "value": "0.000000000000",
              "module": "D"
            },
            {
              "name": "referenceToUnitGroupDataSet",
              "value": {
                "shortDescription": [
                  {
                    "value": "kg"
                  }
                ],
                "type": "unit group data set",
                "refObjectId": "ad38d542-3fe9-439d-9b95-2f5f7752acaf",
                "uri": "../unitgroups/ad38d542-3fe9-439d-9b95-2f5f7752acaf"
              }
            }
          ]
        },
        "flowProperties": [],
        "typeOfFlow": "Other flow",
        "classification": {
          "classHierarchy": "Gr\u00f6\u00dfen / Umweltliche Gr\u00f6\u00dfen / EPD EN 15804 / LCI Indikatoren",
          "name": "GaBiCategories"
        }
      },
      {
        "dataSetInternalID": 14,
        "referenceToFlowDataSet": {
          "shortDescription": [
            {
              "value": "Radioactive waste disposed (RWD)",
              "lang": "en"
            },
            {
              "value": "Avhendet radioaktivt avfall (RW)",
              "lang": "no"
            }
          ],
          "type": "flow data set",
          "refObjectId": "3449546e-52ad-4b39-b809-9fb77cea8ff6",
          "version": "30.00.000"
        },
        "exchange direction": "OUTPUT",
        "meanAmount": 0.0,
        "resultingAmount": 0.0,
        "minimumAmount": 0.0,
        "maximumAmount": 0.0,
        "uncertaintyDistributionType": "UNDEFINED",
        "relativeStandardDeviation95In": "0",
        "dataSourceType": "Primary",
        "dataDerivationTypeStatus": "MEASURED",
        "other": {
          "anies": [
            {
              "value": "0.000000000000",
              "module": "A1"
            },
            {
              "value": "0.000000000000",
              "module": "A2"
            },
            {
              "value": "0.000000000000",
              "module": "A3"
            },
            {
              "value": "0.000000000000",
              "module": "A4"
            },
            {
              "value": "0.000000000000",
              "module": "C1"
            },
            {
              "value": "0.000000000000",
              "module": "C2"
            },
            {
              "value": "0.000000000000",
              "module": "C3"
            },
            {
              "value": "0.000000000000",
              "module": "C4"
            },
            {
              "value": "0.000000000000",
              "module": "D"
            },
            {
              "name": "referenceToUnitGroupDataSet",
              "value": {
                "shortDescription": [
                  {
                    "value": "kg"
                  }
                ],
                "type": "unit group data set",
                "refObjectId": "ad38d542-3fe9-439d-9b95-2f5f7752acaf",
                "uri": "../unitgroups/ad38d542-3fe9-439d-9b95-2f5f7752acaf"
              }
            }
          ]
        },
        "flowProperties": [],
        "typeOfFlow": "Other flow",
        "classification": {
          "classHierarchy": "Gr\u00f6\u00dfen / Umweltliche Gr\u00f6\u00dfen / EPD EN 15804 / LCI Indikatoren",
          "name": "GaBiCategories"
        }
      },
      {
        "dataSetInternalID": 15,
        "referenceToFlowDataSet": {
          "shortDescription": [
            {
              "value": "Components for re-use (CRU)",
              "lang": "en"
            },
            {
              "value": "Komponenter for gjenbruk (CR)",
              "lang": "no"
            }
          ],
          "type": "flow data set",
          "refObjectId": "a2b32f97-3fc7-4af2-b209-525bc6426f33",
          "version": "30.00.000"
        },
        "exchange direction": "OUTPUT",
        "meanAmount": 0.0,
        "resultingAmount": 0.0,
        "minimumAmount": 0.0,
        "maximumAmount": 0.0,
        "uncertaintyDistributionType": "UNDEFINED",
        "relativeStandardDeviation95In": "0",
        "dataSourceType": "Primary",
        "dataDerivationTypeStatus": "MEASURED",
        "other": {
          "anies": [
            {
              "value": "0.000000000000",
              "module": "A1"
            },
            {
              "value": "0.000000000000",
              "module": "A2"
            },
            {
              "value": "0.000000000000",
              "module": "A3"
            },
            {
              "value": "0.000000000000",
              "module": "A4"
            },
            {
              "value": "0.000000000000",
              "module": "C1"
            },
            {
              "value": "0.000000000000",
              "module": "C2"
            },
            {
              "value": "0.000000000000",
              "module": "C3"
            },
            {
              "value": "0.000000000000",
              "module": "C4"
            },
            {
              "value": "0.000000000000",
              "module": "D"
            },
            {
              "name": "referenceToUnitGroupDataSet",
              "value": {
                "shortDescription": [
                  {
                    "value": "kg"
                  }
                ],
                "type": "unit group data set",
                "refObjectId": "ad38d542-3fe9-439d-9b95-2f5f7752acaf",
                "uri": "../unitgroups/ad38d542-3fe9-439d-9b95-2f5f7752acaf"
              }
            }
          ]
        },
        "flowProperties": [],
        "typeOfFlow": "Other flow",
        "classification": {
          "classHierarchy": "Gr\u00f6\u00dfen / Umweltliche Gr\u00f6\u00dfen / EPD EN 15804 / LCI Indikatoren",
          "name": "GaBiCategories"
        }
      },
      {
        "dataSetInternalID": 16,
        "referenceToFlowDataSet": {
          "shortDescription": [
            {
              "value": "Materials for recycling (MFR)",
              "lang": "en"
            },
            {
              "value": "Materialer for resirkulering (MR)",
              "lang": "no"
            }
          ],
          "type": "flow data set",
          "refObjectId": "d7fe48a5-4103-49c8-9aae-b0b5dfdbd6ae",
          "version": "30.00.000"
        },
        "exchange direction": "OUTPUT",
        "meanAmount": 0.0,
        "resultingAmount": 0.0,
        "minimumAmount": 0.0,
        "maximumAmount": 0.0,
        "uncertaintyDistributionType": "UNDEFINED",
        "relativeStandardDeviation95In": "0",
        "dataSourceType": "Primary",
        "dataDerivationTypeStatus": "MEASURED",
        "other": {
          "anies": [
            {
              "value": "0.000000000000",
              "module": "A1"
            },
            {
              "value": "0.000000000000",
              "module": "A2"
            },
            {
              "value": "0.000000000000",
              "module": "A3"
            },
            {
              "value": "0.000000000000",
              "module": "A4"
            },
            {
              "value": "0.000000000000",
              "module": "C1"
            },
            {
              "value": "0.000000000000",
              "module": "C2"
            },
            {
              "value": "0.000000000000",
              "module": "C3"
            },
            {
              "value": "0.000000000000",
              "module": "C4"
            },
            {
              "value": "0.000000000000",
              "module": "D"
            },
            {
              "name": "referenceToUnitGroupDataSet",
              "value": {
                "shortDescription": [
                  {
                    "value": "kg"
                  }
                ],
                "type": "unit group data set",
                "refObjectId": "ad38d542-3fe9-439d-9b95-2f5f7752acaf",
                "uri": "../unitgroups/ad38d542-3fe9-439d-9b95-2f5f7752acaf"
              }
            }
          ]
        },
        "flowProperties": [],
        "typeOfFlow": "Other flow",
        "classification": {
          "classHierarchy": "Gr\u00f6\u00dfen / Umweltliche Gr\u00f6\u00dfen / EPD EN 15804 / LCI Indikatoren",
          "name": "GaBiCategories"
        }
      },
      {
        "dataSetInternalID": 17,
        "referenceToFlowDataSet": {
          "shortDescription": [
            {
              "value": "Materials for energy recovery (MER)",
              "lang": "en"
            },
            {
              "value": "Materialer for energigjenvinning (MER)",
              "lang": "no"
            }
          ],
          "type": "flow data set",
          "refObjectId": "59a9181c-3aaf-46ee-8b13-2b3723b6e447",
          "version": "30.00.000"
        },
        "exchange direction": "OUTPUT",
        "meanAmount": 0.0,
        "resultingAmount": 0.0,
        "minimumAmount": 0.0,
        "maximumAmount": 0.0,
        "uncertaintyDistributionType": "UNDEFINED",
        "relativeStandardDeviation95In": "0",
        "dataSourceType": "Primary",
        "dataDerivationTypeStatus": "MEASURED",
        "other": {
          "anies": [
            {
              "value": "0.000000000000",
              "module": "A1"
            },
            {
              "value": "0.000000000000",
              "module": "A2"
            },
            {
              "value": "0.000000000000",
              "module": "A3"
            },
            {
              "value": "0.000000000000",
              "module": "A4"
            },
            {
              "value": "0.000000000000",
              "module": "C1"
            },
            {
              "value": "0.000000000000",
              "module": "C2"
            },
            {
              "value": "0.000000000000",
              "module": "C3"
            },
            {
              "value": "0.000000000000",
              "module": "C4"
            },
            {
              "value": "0.000000000000",
              "module": "D"
            },
            {
              "name": "referenceToUnitGroupDataSet",
              "value": {
                "shortDescription": [
                  {
                    "value": "kg"
                  }
                ],
                "type": "unit group data set",
                "refObjectId": "ad38d542-3fe9-439d-9b95-2f5f7752acaf",
                "uri": "../unitgroups/ad38d542-3fe9-439d-9b95-2f5f7752acaf"
              }
            }
          ]
        },
        "flowProperties": [],
        "typeOfFlow": "Other flow",
        "classification": {
          "classHierarchy": "Gr\u00f6\u00dfen / Umweltliche Gr\u00f6\u00dfen / EPD EN 15804 / LCI Indikatoren",
          "name": "GaBiCategories"
        }
      },
      {
        "dataSetInternalID": 18,
        "referenceToFlowDataSet": {
          "shortDescription": [
            {
              "value": "Exported electrical energy (EEE)",
              "lang": "en"
            },
            {
              "value": "Eksportert elektrisk energi(EEE)",
              "lang": "no"
            }
          ],
          "type": "flow data set",
          "refObjectId": "4da0c987-2b76-40d6-9e9e-82a017aaaf29",
          "version": "30.00.000"
        },
        "exchange direction": "OUTPUT",
        "meanAmount": 0.0,
        "resultingAmount": 0.0,
        "minimumAmount": 0.0,
        "maximumAmount": 0.0,
        "uncertaintyDistributionType": "UNDEFINED",
        "relativeStandardDeviation95In": "0",
        "dataSourceType": "Primary",
        "dataDerivationTypeStatus": "MEASURED",
        "other": {
          "anies": [
            {
              "value": "0.000000000000",
              "module": "A1"
            },
            {
              "value": "0.000000000000",
              "module": "A2"
            },
            {
              "value": "0.000000000000",
              "module": "A3"
            },
            {
              "value": "0.000000000000",
              "module": "A4"
            },
            {
              "value": "0.000000000000",
              "module": "C1"
            },
            {
              "value": "0.000000000000",
              "module": "C2"
            },
            {
              "value": "0.000000000000",
              "module": "C3"
            },
            {
              "value": "0.000000000000",
              "module": "C4"
            },
            {
              "value": "0.000000000000",
              "module": "D"
            },
            {
              "name": "referenceToUnitGroupDataSet",
              "value": {
                "shortDescription": [
                  {
                    "value": "MJ"
                  }
                ],
                "type": "unit group data set",
                "refObjectId": "93a60a57-a3c8-11da-a746-0800200c9a66",
                "uri": "../unitgroups/93a60a57-a3c8-11da-a746-0800200c9a66"
              }
            }
          ]
        },
        "flowProperties": [],
        "typeOfFlow": "Other flow",
        "classification": {
          "classHierarchy": "Gr\u00f6\u00dfen / Umweltliche Gr\u00f6\u00dfen / EPD EN 15804 / LCI Indikatoren",
          "name": "GaBiCategories"
        }
      },
      {
        "dataSetInternalID": 19,
        "referenceToFlowDataSet": {
          "shortDescription": [
            {
              "value": "Exported thermal energy (EET)",
              "lang": "en"
            },
            {
              "value": "Eksportert termisk energi (ETE)",
              "lang": "no"
            }
          ],
          "type": "flow data set",
          "refObjectId": "98daf38a-7a79-46d3-9a37-2b7bd0955810",
          "version": "30.00.000"
        },
        "exchange direction": "OUTPUT",
        "meanAmount": 0.0,
        "resultingAmount": 0.0,
        "minimumAmount": 0.0,
        "maximumAmount": 0.0,
        "uncertaintyDistributionType": "UNDEFINED",
        "relativeStandardDeviation95In": "0",
        "dataSourceType": "Primary",
        "dataDerivationTypeStatus": "MEASURED",
        "other": {
          "anies": [
            {
              "value": "0.000000000000",
              "module": "A1"
            },
            {
              "value": "0.000000000000",
              "module": "A2"
            },
            {
              "value": "0.000000000000",
              "module": "A3"
            },
            {
              "value": "0.000000000000",
              "module": "A4"
            },
            {
              "value": "0.000000000000",
              "module": "C1"
            },
            {
              "value": "0.000000000000",
              "module": "C2"
            },
            {
              "value": "0.000000000000",
              "module": "C3"
            },
            {
              "value": "0.000000000000",
              "module": "C4"
            },
            {
              "value": "0.000000000000",
              "module": "D"
            },
            {
              "name": "referenceToUnitGroupDataSet",
              "value": {
                "shortDescription": [
                  {
                    "value": "MJ"
                  }
                ],
                "type": "unit group data set",
                "refObjectId": "93a60a57-a3c8-11da-a746-0800200c9a66",
                "uri": "../unitgroups/93a60a57-a3c8-11da-a746-0800200c9a66"
              }
            }
          ]
        },
        "flowProperties": [],
        "typeOfFlow": "Other flow",
        "classification": {
          "classHierarchy": "Gr\u00f6\u00dfen / Umweltliche Gr\u00f6\u00dfen / EPD EN 15804 / LCI Indikatoren",
          "name": "GaBiCategories"
        }
      }
    ]
  },
  "LCIAResults": {
    "LCIAResult": [
      {
        "referenceToLCIAMethodDataSet": {
          "shortDescription": [
            {
              "value": "Acidification potential, Accumulated Exceedance (AP)",
              "lang": "en"
            },
            {
              "value": "Forsurningspotensial for kilder p\u00e5 land og vann (AP)",
              "lang": "no"
            }
          ],
          "type": "LCIA method data set",
          "refObjectId": "b5c611c6-def3-11e6-bf01-fe55135034f3",
          "version": "00.01.000"
        },
        "meanAmount": 0.0,
        "uncertaintyDistributionType": "undefined",
        "relativeStandardDeviation95In": 0,
        "other": {
          "anies": [
            {
              "value": "1.725719662094",
              "module": "A1"
            },
            {
              "value": "0.067958135150",
              "module": "A2"
            },
            {
              "value": "0.310455015235",
              "module": "A3"
            },
            {
              "value": "0.039517386416",
              "module": "A4"
            },
            {
              "value": "0.503571364759",
              "module": "C1"
            },
            {
              "value": "0.035153935695",
              "module": "C2"
            },
            {
              "value": "0.011207014303",
              "module": "C3"
            },
            {
              "value": "0.002510800176",
              "module": "C4"
            },
            {
              "value": "0.528612608997",
              "module": "D"
            },
            {
              "name": "referenceToUnitGroupDataSet",
              "value": {
                "shortDescription": [
                  {
                    "value": "mol H+ eqv."
                  }
                ],
                "type": "unit group data set",
                "refObjectId": "42e089ac-92bf-4bf2-8ca1-5fc40d18f2ed",
                "uri": "../unitgroups/42e089ac-92bf-4bf2-8ca1-5fc40d18f2ed"
              }
            }
          ]
        }
      },
      {
        "referenceToLCIAMethodDataSet": {
          "shortDescription": [
            {
              "value": "Global Warming Potential - total (GWP-total)",
              "lang": "en"
            },
            {
              "value": "Globalt oppvarmingspotensial -totalt (GWPtotal)",
              "lang": "no"
            }
          ],
          "type": "LCIA method data set",
          "refObjectId": "6a37f984-a4b3-458a-a20a-64418c145fa2",
          "version": "00.02.000"
        },
        "meanAmount": 0.0,
        "uncertaintyDistributionType": "undefined",
        "relativeStandardDeviation95In": 0,
        "other": {
          "anies": [
            {
              "value": "477.867466985986",
              "module": "A1"
            },
            {
              "value": "23.037495011571",
              "module": "A2"
            },
            {
              "value": "133.402780387693",
              "module": "A3"
            },
            {
              "value": "16.794367074941",
              "module": "A4"
            },
            {
              "value": "53.838900736677",
              "module": "C1"
            },
            {
              "value": "17.824300271219",
              "module": "C2"
            },
            {
              "value": "2.362400591016",
              "module": "C3"
            },
            {
              "value": "0.278430794587",
              "module": "C4"
            },
            {
              "value": "141.675721123995",
              "module": "D"
            },
            {
              "name": "referenceToUnitGroupDataSet",
              "value": {
                "shortDescription": [
                  {
                    "value": "kg CO2 eqv."
                  }
                ],
                "type": "unit group data set",
                "refObjectId": "1ebf3012-d0db-4de2-aefd-ef30cedb0be1",
                "uri": "../unitgroups/1ebf3012-d0db-4de2-aefd-ef30cedb0be1"
              }
            }
          ]
        }
      },
      {
        "referenceToLCIAMethodDataSet": {
          "shortDescription": [
            {
              "value": "Global Warming Potential - biogenic (GWP-biogenic)",
              "lang": "en"
            },
            {
              "value": "Globalt oppvarmingspotensial - biogene kilder( GWP-biogenic)",
              "lang": "no"
            }
          ],
          "type": "LCIA method data set",
          "refObjectId": "2356e1ab-0185-4db5-86e5-16de51c7485c",
          "version": "00.02.000"
        },
        "meanAmount": 0.0,
        "uncertaintyDistributionType": "undefined",
        "relativeStandardDeviation95In": 0,
        "other": {
          "anies": [
            {
              "value": "0.221748530349",
              "module": "A1"
            },
            {
              "value": "0.010773064806",
              "module": "A2"
            },
            {
              "value": "0.241440243412",
              "module": "A3"
            },
            {
              "value": "0.002834124073",
              "module": "A4"
            },
            {
              "value": "0.003944306093",
              "module": "C1"
            },
            {
              "value": "0.001309467787",
              "module": "C2"
            },
            {
              "value": "0.007090129130",
              "module": "C3"
            },
            {
              "value": "0.000035891036",
              "module": "C4"
            },
            {
              "value": "0.013244418357",
              "module": "D"
            },
            {
              "name": "referenceToUnitGroupDataSet",
              "value": {
                "shortDescription": [
                  {
                    "value": "kg CO2 eqv."
                  }
                ],
                "type": "unit group data set",
                "refObjectId": "1ebf3012-d0db-4de2-aefd-ef30cedb0be1",
                "uri": "../unitgroups/1ebf3012-d0db-4de2-aefd-ef30cedb0be1"
              }
            }
          ]
        }
      },
      {
        "referenceToLCIAMethodDataSet": {
          "shortDescription": [
            {
              "value": "Global Warming Potential - fossil fuels (GWP-fossil)",
              "lang": "en"
            },
            {
              "value": "Globalt oppvarmingspotensial - fossile brensler (GWP-fossil)",
              "lang": "no"
            }
          ],
          "type": "LCIA method data set",
          "refObjectId": "5f635281-343e-44fb-83df-1971b155e6b6",
          "version": "00.01.000"
        },
        "meanAmount": 0.0,
        "uncertaintyDistributionType": "undefined",
        "relativeStandardDeviation95In": 0,
        "other": {
          "anies": [
            {
              "value": "477.524717868421",
              "module": "A1"
            },
            {
              "value": "23.023771291525",
              "module": "A2"
            },
            {
              "value": "133.104236231349",
              "module": "A3"
            },
            {
              "value": "16.790596036683",
              "module": "A4"
            },
            {
              "value": "53.832798554356",
              "module": "C1"
            },
            {
              "value": "17.822646168631",
              "module": "C2"
            },
            {
              "value": "2.349523075308",
              "module": "C3"
            },
            {
              "value": "0.278381290484",
              "module": "C4"
            },
            {
              "value": "141.649496807441",
              "module": "D"
            },
            {
              "name": "referenceToUnitGroupDataSet",
              "value": {
                "shortDescription": [
                  {
                    "value": "kg CO2 eqv."
                  }
                ],
                "type": "unit group data set",
                "refObjectId": "1ebf3012-d0db-4de2-aefd-ef30cedb0be1",
                "uri": "../unitgroups/1ebf3012-d0db-4de2-aefd-ef30cedb0be1"
              }
            }
          ]
        }
      },
      {
        "referenceToLCIAMethodDataSet": {
          "shortDescription": [
            {
              "value": "Global Warming Potential - land use and land use change (GWP-luluc)",
              "lang": "en"
            },
            {
              "value": "Globalt oppvarmingspotensial arealbruk endringer i bruk av arealer (GWP-luluc)",
              "lang": "no"
            }
          ],
          "type": "LCIA method data set",
          "refObjectId": "4331bbdb-978a-490d-8707-eeb047f01a55",
          "version": "00.02.000"
        },
        "meanAmount": 0.0,
        "uncertaintyDistributionType": "undefined",
        "relativeStandardDeviation95In": 0,
        "other": {
          "anies": [
            {
              "value": "0.121000587217",
              "module": "A1"
            },
            {
              "value": "0.002950655240",
              "module": "A2"
            },
            {
              "value": "0.057103912932",
              "module": "A3"
            },
            {
              "value": "0.000936914185",
              "module": "A4"
            },
            {
              "value": "0.002157876228",
              "module": "C1"
            },
            {
              "value": "0.000344634800",
              "module": "C2"
            },
            {
              "value": "0.005787386578",
              "module": "C3"
            },
            {
              "value": "0.000013613067",
              "module": "C4"
            },
            {
              "value": "0.012979898197",
              "module": "D"
            },
            {
              "name": "referenceToUnitGroupDataSet",
              "value": {
                "shortDescription": [
                  {
                    "value": "kg CO2 eqv."
                  }
                ],
                "type": "unit group data set",
                "refObjectId": "1ebf3012-d0db-4de2-aefd-ef30cedb0be1",
                "uri": "../unitgroups/1ebf3012-d0db-4de2-aefd-ef30cedb0be1"
              }
            }
          ]
        }
      },
      {
        "referenceToLCIAMethodDataSet": {
          "shortDescription": [
            {
              "value": "Potential Comparative Toxic Unit for ecosystems (ETP-fw)",
              "lang": "en"
            },
            {
              "value": "\u00d8kotoksisitet, ferskvann (ETP-fw)",
              "lang": "no"
            }
          ],
          "type": "LCIA method data set",
          "refObjectId": "ee1082d1-b0f7-43ca-a1f0-21e2a4a74511",
          "version": "00.01.000"
        },
        "meanAmount": 0.0,
        "uncertaintyDistributionType": "undefined",
        "relativeStandardDeviation95In": 0,
        "other": {
          "anies": [
            {
              "value": "811.153882172761",
              "module": "A1"
            },
            {
              "value": "108.476181039467",
              "module": "A2"
            },
            {
              "value": "130.527426906523",
              "module": "A3"
            },
            {
              "value": "82.238348812189",
              "module": "A4"
            },
            {
              "value": "277.335719495373",
              "module": "C1"
            },
            {
              "value": "88.434125339680",
              "module": "C2"
            },
            {
              "value": "2.922779191395",
              "module": "C3"
            },
            {
              "value": "1.358316073885",
              "module": "C4"
            },
            {
              "value": "254.125584084856",
              "module": "D"
            },
            {
              "name": "referenceToUnitGroupDataSet",
              "value": {
                "shortDescription": [
                  {
                    "value": "CTUe"
                  }
                ],
                "type": "unit group data set",
                "refObjectId": "aa959ded-f1eb-4efb-9c5c-2d60be36b3e6",
                "uri": "../unitgroups/aa959ded-f1eb-4efb-9c5c-2d60be36b3e6"
              }
            }
          ]
        }
      },
      {
        "referenceToLCIAMethodDataSet": {
          "shortDescription": [
            {
              "value": "Potential incidence of disease due to PM emissions (PM)",
              "lang": "en"
            },
            {
              "value": "Partikkelutslipp (PM)",
              "lang": "no"
            }
          ],
          "type": "LCIA method data set",
          "refObjectId": "b5c602c6-def3-11e6-bf01-fe55135034f3",
          "version": "00.01.000"
        },
        "meanAmount": 0.0,
        "uncertaintyDistributionType": "undefined",
        "relativeStandardDeviation95In": 0,
        "other": {
          "anies": [
            {
              "value": "0.000047617871",
              "module": "A1"
            },
            {
              "value": "0.000001839279",
              "module": "A2"
            },
            {
              "value": "0.000003255751",
              "module": "A3"
            },
            {
              "value": "0.000001307777",
              "module": "A4"
            },
            {
              "value": "0.000014203817",
              "module": "C1"
            },
            {
              "value": "0.000001409831",
              "module": "C2"
            },
            {
              "value": "0.000000103621",
              "module": "C3"
            },
            {
              "value": "0.000000069537",
              "module": "C4"
            },
            {
              "value": "0.000007096426",
              "module": "D"
            },
            {
              "name": "referenceToUnitGroupDataSet",
              "value": {
                "shortDescription": [
                  {
                    "value": "disease incidence"
                  }
                ],
                "type": "unit group data set",
                "refObjectId": "3883559b-648f-4afc-8ba2-0bd24f3affa3",
                "uri": "../unitgroups/3883559b-648f-4afc-8ba2-0bd24f3affa3"
              }
            }
          ]
        }
      },
      {
        "referenceToLCIAMethodDataSet": {
          "shortDescription": [
            {
              "value": "Eutrophication potential - marine (EP-marine)",
              "lang": "en"
            },
            {
              "value": "Overgj\u00f8dslingspotensial til hav (EP-marine), hav og jord",
              "lang": "no"
            }
          ],
          "type": "LCIA method data set",
          "refObjectId": "b5c619fa-def3-11e6-bf01-fe55135034f3",
          "version": "00.01.000"
        },
        "meanAmount": 0.0,
        "uncertaintyDistributionType": "undefined",
        "relativeStandardDeviation95In": 0,
        "other": {
          "anies": [
            {
              "value": "0.334667252011",
              "module": "A1"
            },
            {
              "value": "0.026002925705",
              "module": "A2"
            },
            {
              "value": "0.102173692968",
              "module": "A3"
            },
            {
              "value": "0.013102519523",
              "module": "A4"
            },
            {
              "value": "0.236538142027",
              "module": "C1"
            },
            {
              "value": "0.012340795051",
              "module": "C2"
            },
            {
              "value": "0.002160485281",
              "module": "C3"
            },
            {
              "value": "0.001140537300",
              "module": "C4"
            },
            {
              "value": "0.104042648151",
              "module": "D"
            },
            {
              "name": "referenceToUnitGroupDataSet",
              "value": {
                "shortDescription": [
                  {
                    "value": "kg N eqv."
                  }
                ],
                "type": "unit group data set",
                "refObjectId": "d05bb823-ecdf-4686-8c40-bf1d9257859f",
                "uri": "../unitgroups/d05bb823-ecdf-4686-8c40-bf1d9257859f"
              }
            }
          ]
        }
      },
      {
        "referenceToLCIAMethodDataSet": {
          "shortDescription": [
            {
              "value": "Eutrophication potential - freshwater (EP-freshwater)",
              "lang": "en"
            },
            {
              "value": "Overgj\u00f8dslingspotensial til ferskvann (EP-freshwater)",
              "lang": "no"
            }
          ],
          "type": "LCIA method data set",
          "refObjectId": "b53ec18f-7377-4ad3-86eb-cc3f4f276b2b",
          "version": "00.01.000"
        },
        "meanAmount": 0.0,
        "uncertaintyDistributionType": "undefined",
        "relativeStandardDeviation95In": 0,
        "other": {
          "anies": [
            {
              "value": "0.009550884462",
              "module": "A1"
            },
            {
              "value": "0.000119054649",
              "module": "A2"
            },
            {
              "value": "0.002421430461",
              "module": "A3"
            },
            {
              "value": "0.000037096447",
              "module": "A4"
            },
            {
              "value": "0.000045023439",
              "module": "C1"
            },
            {
              "value": "0.000013815301",
              "module": "C2"
            },
            {
              "value": "0.000115771719",
              "module": "C3"
            },
            {
              "value": "0.000000954098",
              "module": "C4"
            },
            {
              "value": "0.005976484705",
              "module": "D"
            },
            {
              "name": "referenceToUnitGroupDataSet",
              "value": {
                "shortDescription": [
                  {
                    "value": "kg P eqv."
                  }
                ],
                "type": "unit group data set",
                "refObjectId": "0429039d-a61d-4590-ba67-aa4a20a810a1",
                "uri": "../unitgroups/0429039d-a61d-4590-ba67-aa4a20a810a1"
              }
            }
          ]
        }
      },
      {
        "referenceToLCIAMethodDataSet": {
          "shortDescription": [
            {
              "value": "Eutrophication potential - terrestrial (EP-terrestrial)",
              "lang": "en"
            },
            {
              "value": "Overgj\u00f8dslingspotensial til jord (EP-terrestrial)",
              "lang": "no"
            }
          ],
          "type": "LCIA method data set",
          "refObjectId": "b5c614d2-def3-11e6-bf01-fe55135034f3",
          "version": "00.01.000"
        },
        "meanAmount": 0.0,
        "uncertaintyDistributionType": "undefined",
        "relativeStandardDeviation95In": 0,
        "other": {
          "anies": [
            {
              "value": "3.735637824728",
              "module": "A1"
            },
            {
              "value": "0.276888823837",
              "module": "A2"
            },
            {
              "value": "1.127695848244",
              "module": "A3"
            },
            {
              "value": "0.137432611409",
              "module": "A4"
            },
            {
              "value": "2.573197782627",
              "module": "C1"
            },
            {
              "value": "0.128267588059",
              "module": "C2"
            },
            {
              "value": "0.023820980216",
              "module": "C3"
            },
            {
              "value": "0.012409221047",
              "module": "C4"
            },
            {
              "value": "1.203818677551",
              "module": "D"
            },
            {
              "name": "referenceToUnitGroupDataSet",
              "value": {
                "shortDescription": [
                  {
                    "value": "mol N eqv."
                  }
                ],
                "type": "unit group data set",
                "refObjectId": "71b4d617-0ec9-4d3f-b65e-e438940c2401",
                "uri": "../unitgroups/71b4d617-0ec9-4d3f-b65e-e438940c2401"
              }
            }
          ]
        }
      },
      {
        "referenceToLCIAMethodDataSet": {
          "shortDescription": [
            {
              "value": "Potential Comparative Toxic Unit for humans - cancer effects (HTP-c)",
              "lang": "en"
            },
            {
              "value": "Toksisitet p\u00e5virkning p\u00e5 mennesker, kreft (HTP-c)",
              "lang": "no"
            }
          ],
          "type": "LCIA method data set",
          "refObjectId": "2299222a-bbd8-474f-9d4f-4dd1f18aea7c",
          "version": "00.01.000"
        },
        "meanAmount": 0.0,
        "uncertaintyDistributionType": "undefined",
        "relativeStandardDeviation95In": 0,
        "other": {
          "anies": [
            {
              "value": "0.000000139221",
              "module": "A1"
            },
            {
              "value": "0.000000000880",
              "module": "A2"
            },
            {
              "value": "0.000000039362",
              "module": "A3"
            },
            {
              "value": "0.000000000576",
              "module": "A4"
            },
            {
              "value": "0.000000002033",
              "module": "C1"
            },
            {
              "value": "0.000000000607",
              "module": "C2"
            },
            {
              "value": "0.000000000091",
              "module": "C3"
            },
            {
              "value": "0.000000000015",
              "module": "C4"
            },
            {
              "value": "0.000000627442",
              "module": "D"
            },
            {
              "name": "referenceToUnitGroupDataSet",
              "value": {
                "shortDescription": [
                  {
                    "value": "CTUh"
                  }
                ],
                "type": "unit group data set",
                "refObjectId": "d4c9523e-2d7e-49fd-8469-998f547d3a70",
                "uri": "../unitgroups/d4c9523e-2d7e-49fd-8469-998f547d3a70"
              }
            }
          ]
        }
      },
      {
        "referenceToLCIAMethodDataSet": {
          "shortDescription": [
            {
              "value": "Potential Comparative Toxic Unit for humans - non-cancer effects (HTP-nc)",
              "lang": "en"
            },
            {
              "value": "Toksisitet p\u00e5virkning p\u00e5 mennesker, andre effekter enn kreft (HTP-nc) ",
              "lang": "no"
            }
          ],
          "type": "LCIA method data set",
          "refObjectId": "3af763a5-b7a1-48c9-9cee-1f223481fcef",
          "version": "00.01.000"
        },
        "meanAmount": 0.0,
        "uncertaintyDistributionType": "undefined",
        "relativeStandardDeviation95In": 0,
        "other": {
          "anies": [
            {
              "value": "0.000000728344",
              "module": "A1"
            },
            {
              "value": "0.000000061786",
              "module": "A2"
            },
            {
              "value": "0.000003750062",
              "module": "A3"
            },
            {
              "value": "0.000000041117",
              "module": "A4"
            },
            {
              "value": "0.000000231875",
              "module": "C1"
            },
            {
              "value": "0.000000044005",
              "module": "C2"
            },
            {
              "value": "0.000000002016",
              "module": "C3"
            },
            {
              "value": "0.000000002419",
              "module": "C4"
            },
            {
              "value": "0.000002299001",
              "module": "D"
            },
            {
              "name": "referenceToUnitGroupDataSet",
              "value": {
                "shortDescription": [
                  {
                    "value": "CTUh"
                  }
                ],
                "type": "unit group data set",
                "refObjectId": "d4c9523e-2d7e-49fd-8469-998f547d3a70",
                "uri": "../unitgroups/d4c9523e-2d7e-49fd-8469-998f547d3a70"
              }
            }
          ]
        }
      },
      {
        "referenceToLCIAMethodDataSet": {
          "shortDescription": [
            {
              "value": "Potential Human exposure efficiency relative to U235 (IRP)",
              "lang": "en"
            },
            {
              "value": "Ioniserende str\u00e5ling, helseeffekt (IRP)",
              "lang": "no"
            }
          ],
          "type": "LCIA method data set",
          "refObjectId": "b5c632be-def3-11e6-bf01-fe55135034f3",
          "version": "00.01.000"
        },
        "meanAmount": 0.0,
        "uncertaintyDistributionType": "undefined",
        "relativeStandardDeviation95In": 0,
        "other": {
          "anies": [
            {
              "value": "9.465755015623",
              "module": "A1"
            },
            {
              "value": "0.268003672540",
              "module": "A2"
            },
            {
              "value": "4.680156240692",
              "module": "A3"
            },
            {
              "value": "0.086234734254",
              "module": "A4"
            },
            {
              "value": "0.081464650939",
              "module": "C1"
            },
            {
              "value": "0.037217329778",
              "module": "C2"
            },
            {
              "value": "0.140032048207",
              "module": "C3"
            },
            {
              "value": "0.000463551567",
              "module": "C4"
            },
            {
              "value": "-0.960497587154",
              "module": "D"
            },
            {
              "name": "referenceToUnitGroupDataSet",
              "value": {
                "shortDescription": [
                  {
                    "value": "kBq U235 eqv."
                  }
                ],
                "type": "unit group data set",
                "refObjectId": "456b05bf-1415-44a9-9993-02452f554c09",
                "uri": "../unitgroups/456b05bf-1415-44a9-9993-02452f554c09"
              }
            }
          ]
        }
      },
      {
        "referenceToLCIAMethodDataSet": {
          "shortDescription": [
            {
              "value": "Potential Soil quality index (SQP)",
              "lang": "en"
            },
            {
              "value": "P\u00e5virkninger knyttet til arealbruksendringer / jordkvalitet (SQP)",
              "lang": "no"
            }
          ],
          "type": "LCIA method data set",
          "refObjectId": "b2ad6890-c78d-11e6-9d9d-cec0c932ce01",
          "version": "00.01.000"
        },
        "meanAmount": 0.0,
        "uncertaintyDistributionType": "undefined",
        "relativeStandardDeviation95In": 0,
        "other": {
          "anies": [
            {
              "value": "814.833791332910",
              "module": "A1"
            },
            {
              "value": "3.832187989417",
              "module": "A2"
            },
            {
              "value": "90.225449541474",
              "module": "A3"
            },
            {
              "value": "1.127654369151",
              "module": "A4"
            },
            {
              "value": "1.309456023677",
              "module": "C1"
            },
            {
              "value": "0.444400009526",
              "module": "C2"
            },
            {
              "value": "2.889873708536",
              "module": "C3"
            },
            {
              "value": "4.121326952565",
              "module": "C4"
            },
            {
              "value": "219.422195943168",
              "module": "D"
            },
            {
              "name": "referenceToUnitGroupDataSet",
              "value": {
                "shortDescription": [
                  {
                    "value": "unitless"
                  }
                ],
                "type": "unit group data set",
                "refObjectId": "f130951c-e67f-4f7f-8dd4-665de3974e18",
                "uri": "../unitgroups/f130951c-e67f-4f7f-8dd4-665de3974e18"
              }
            }
          ]
        }
      },
      {
        "referenceToLCIAMethodDataSet": {
          "shortDescription": [
            {
              "value": "Depletion potential of the stratospheric ozone layer (ODP)",
              "lang": "en"
            },
            {
              "value": "Potensial for nedbryting av stratosf\u00e6risk ozon (ODP)",
              "lang": "no"
            }
          ],
          "type": "LCIA method data set",
          "refObjectId": "b5c629d6-def3-11e6-bf01-fe55135034f3",
          "version": "00.01.000"
        },
        "meanAmount": 0.0,
        "uncertaintyDistributionType": "undefined",
        "relativeStandardDeviation95In": 0,
        "other": {
          "anies": [
            {
              "value": "0.000012497569",
              "module": "A1"
            },
            {
              "value": "0.000000483858",
              "module": "A2"
            },
            {
              "value": "0.000000680468",
              "module": "A3"
            },
            {
              "value": "0.000000355462",
              "module": "A4"
            },
            {
              "value": "0.000000829444",
              "module": "C1"
            },
            {
              "value": "0.000000379996",
              "module": "C2"
            },
            {
              "value": "0.000000014426",
              "module": "C3"
            },
            {
              "value": "0.000000004016",
              "module": "C4"
            },
            {
              "value": "0.000002552240",
              "module": "D"
            },
            {
              "name": "referenceToUnitGroupDataSet",
              "value": {
                "shortDescription": [
                  {
                    "value": "kg CFC 11 eqv."
                  }
                ],
                "type": "unit group data set",
                "refObjectId": "d9e957c9-7309-4474-bf3a-7777df6c4e5b",
                "uri": "../unitgroups/d9e957c9-7309-4474-bf3a-7777df6c4e5b"
              }
            }
          ]
        }
      },
      {
        "referenceToLCIAMethodDataSet": {
          "shortDescription": [
            {
              "value": "Photochemical Ozone Creation Potential (POCP)",
              "lang": "en"
            },
            {
              "value": "Potensial for fotokjemisk oksidantdanning (POCP)",
              "lang": "no"
            }
          ],
          "type": "LCIA method data set",
          "refObjectId": "b5c610fe-def3-11e6-bf01-fe55135034f3",
          "version": "00.01.000"
        },
        "meanAmount": 0.0,
        "uncertaintyDistributionType": "undefined",
        "relativeStandardDeviation95In": 0,
        "other": {
          "anies": [
            {
              "value": "1.592456459167",
              "module": "A1"
            },
            {
              "value": "0.104242893527",
              "module": "A2"
            },
            {
              "value": "0.306583780794",
              "module": "A3"
            },
            {
              "value": "0.059703657738",
              "module": "A4"
            },
            {
              "value": "0.757151067033",
              "module": "C1"
            },
            {
              "value": "0.059256742436",
              "module": "C2"
            },
            {
              "value": "0.007145939316",
              "module": "C3"
            },
            {
              "value": "0.003712199738",
              "module": "C4"
            },
            {
              "value": "0.645105241541",
              "module": "D"
            },
            {
              "name": "referenceToUnitGroupDataSet",
              "value": {
                "shortDescription": [
                  {
                    "value": "kg NMVOC eqv."
                  }
                ],
                "type": "unit group data set",
                "refObjectId": "d27c25f8-fbc1-44c6-b47b-4adbae4199c6",
                "uri": "../unitgroups/d27c25f8-fbc1-44c6-b47b-4adbae4199c6"
              }
            }
          ]
        }
      },
      {
        "referenceToLCIAMethodDataSet": {
          "shortDescription": [
            {
              "value": "Abiotic depletion potential - fossil resources (ADPF)",
              "lang": "en"
            },
            {
              "value": "Abiotisk utarmingspotensial for fossile ressurser, fosile brensler (ADP-fossil)",
              "lang": "no"
            }
          ],
          "type": "LCIA method data set",
          "refObjectId": "b2ad6110-c78d-11e6-9d9d-cec0c932ce01",
          "version": "00.01.000"
        },
        "meanAmount": 0.0,
        "uncertaintyDistributionType": "undefined",
        "relativeStandardDeviation95In": 0,
        "other": {
          "anies": [
            {
              "value": "8863.735956364130",
              "module": "A1"
            },
            {
              "value": "310.785057038281",
              "module": "A2"
            },
            {
              "value": "856.263213888109",
              "module": "A3"
            },
            {
              "value": "219.561400941767",
              "module": "A4"
            },
            {
              "value": "680.388461144180",
              "module": "C1"
            },
            {
              "value": "229.610985142981",
              "module": "C2"
            },
            {
              "value": "39.643005156434",
              "module": "C3"
            },
            {
              "value": "3.476057417258",
              "module": "C4"
            },
            {
              "value": "1735.663290457210",
              "module": "D"
            },
            {
              "name": "referenceToUnitGroupDataSet",
              "value": {
                "shortDescription": [
                  {
                    "value": "MJ"
                  }
                ],
                "type": "unit group data set",
                "refObjectId": "93a60a57-a3c8-11da-a746-0800200c9a66",
                "uri": "../unitgroups/93a60a57-a3c8-11da-a746-0800200c9a66"
              }
            }
          ]
        }
      },
      {
        "referenceToLCIAMethodDataSet": {
          "shortDescription": [
            {
              "value": "Abiotic depletion potential - non-fossil resources (ADPE)",
              "lang": "en"
            },
            {
              "value": "Abiotisk utarmingspotensial for ikke-fossile ressurser, mineraler (ADP-elements)",
              "lang": "no"
            }
          ],
          "type": "LCIA method data set",
          "refObjectId": "b2ad6494-c78d-11e6-9d9d-cec0c932ce01",
          "version": "00.01.000"
        },
        "meanAmount": 0.0,
        "uncertaintyDistributionType": "undefined",
        "relativeStandardDeviation95In": 0,
        "other": {
          "anies": [
            {
              "value": "0.000065665966",
              "module": "A1"
            },
            {
              "value": "0.000000802536",
              "module": "A2"
            },
            {
              "value": "0.000085404119",
              "module": "A3"
            },
            {
              "value": "0.000000571900",
              "module": "A4"
            },
            {
              "value": "0.000002210628",
              "module": "C1"
            },
            {
              "value": "0.000000604573",
              "module": "C2"
            },
            {
              "value": "0.000000065657",
              "module": "C3"
            },
            {
              "value": "0.000000010729",
              "module": "C4"
            },
            {
              "value": "0.001201371366",
              "module": "D"
            },
            {
              "name": "referenceToUnitGroupDataSet",
              "value": {
                "shortDescription": [
                  {
                    "value": "kg Sb-eqv."
                  }
                ],
                "type": "unit group data set",
                "refObjectId": "54ccd2d9-a32a-4fc2-923d-f2c8c93e89d4",
                "uri": "../unitgroups/54ccd2d9-a32a-4fc2-923d-f2c8c93e89d4"
              }
            }
          ]
        }
      },
      {
        "referenceToLCIAMethodDataSet": {
          "shortDescription": [
            {
              "value": "Water (user) deprivation potential (WDP)",
              "lang": "en"
            },
            {
              "value": "Utarmingspotensial for vannressurser (WDP)",
              "lang": "no"
            }
          ],
          "type": "LCIA method data set",
          "refObjectId": "b2ad66ce-c78d-11e6-9d9d-cec0c932ce01",
          "version": "00.01.000"
        },
        "meanAmount": 0.0,
        "uncertaintyDistributionType": "undefined",
        "relativeStandardDeviation95In": 0,
        "other": {
          "anies": [
            {
              "value": "46.349239982275",
              "module": "A1"
            },
            {
              "value": "0.603036993005",
              "module": "A2"
            },
            {
              "value": "110.863244924339",
              "module": "A3"
            },
            {
              "value": "0.256831899717",
              "module": "A4"
            },
            {
              "value": "0.892040221096",
              "module": "C1"
            },
            {
              "value": "0.215055561865",
              "module": "C2"
            },
            {
              "value": "0.418644035413",
              "module": "C3"
            },
            {
              "value": "0.004818081336",
              "module": "C4"
            },
            {
              "value": "16.598071444590",
              "module": "D"
            },
            {
              "name": "referenceToUnitGroupDataSet",
              "value": {
                "shortDescription": [
                  {
                    "value": "m3 world eqv."
                  }
                ],
                "type": "unit group data set",
                "refObjectId": "6ae2df01-888e-46c8-b17d-49fa3869b476",
                "uri": "../unitgroups/6ae2df01-888e-46c8-b17d-49fa3869b476"
              }
            }
          ]
        }
      },
      {
        "referenceToLCIAMethodDataSet": {
          "shortDescription": [
            {
              "value": "Global warming potential except emissions and uptake of biogenic carbon (GWP-IOBC/GHG)",
              "lang": "en"
            },
            {
              "value": "Globalt oppvarmingspotensial beregnet etter prinsippet om umiddelbar oksidasjon (GWP-IOBC)",
              "lang": "no"
            }
          ],
          "type": "LCIA method data set",
          "refObjectId": "fb774615-0575-45de-9a89-1ded92f19770",
          "version": "00.01.000"
        },
        "meanAmount": 0.0,
        "uncertaintyDistributionType": "undefined",
        "relativeStandardDeviation95In": 0,
        "other": {
          "anies": [
            {
              "name": "referenceToUnitGroupDataSet",
              "value": {
                "shortDescription": [
                  {
                    "value": "kg CO2 eqv."
                  }
                ],
                "type": "unit group data set",
                "refObjectId": "1ebf3012-d0db-4de2-aefd-ef30cedb0be1",
                "uri": "../unitgroups/1ebf3012-d0db-4de2-aefd-ef30cedb0be1"
              }
            }
          ]
        }
      }
    ]
  },
  "otherAttributes": {
    "{http://www.indata.network/EPD/2019}epd-version": "1.2"
  },
  "version": "1.1",
  "source": "https://node.epditaly.it/resource/datastocks/24493f94-1ca8-4cc7-a056-67cbe25aef5a/processes/7b21d245-2b65-41d0-ba30-9b2585402b20"
}