{
  "processInformation": {
    "dataSetInformation": {
      "UUID": "c1a9158c-d3a9-41f5-b7c2-5fe454e4f014",
      "name": {
        "baseName": [
          {
            "value": "CERAMIC TILES - Fiorano Emilia",
            "lang": "en"
          }
        ]
      },
      "classificationInformation": {
        "classification": [
          {
            "class": [
              {
                "value": "Other transportable goods, except metal products, machinery and equipment",
                "level": 0,
                "classId": "3"
              },
              {
                "value": "Glass and glass products and other non-metallic products n.e.c.",
                "level": 1,
                "classId": "37"
              }
            ],
            "name": "CPC 2.1"
          }
        ]
      },
      "generalComment": [
        {
          "value": "EPDITALY0102\r\nViene considerato l'intero ciclo di vita del prodotto (tipo di EPD: dalla culla alla tomba) ed i moduli di seguito descritti: A1, A2, A3, A4, A5, B2, C2, C3, C4, D",
          "lang": "en"
        }
      ]
    },
    "quantitativeReference": {
      "referenceToReferenceFlow": [
        1
      ],
      "type": "Reference flow(s)"
    },
    "time": {
      "referenceYear": 2018,
      "dataSetValidUntil": 2025,
      "timeRepresentativenessDescription": [
        {
          "value": "dal 11/02/2020 al 11/02/2025 (reference year: anno di raccolta dati 2018)",
          "lang": "en"
        }
      ],
      "other": {
        "anies": [
          {
            "name": "publicationDateOfEPD",
            "value": 1588118400000
          }
        ]
      }
    },
    "geography": {
      "locationOfOperationSupplyOrProduction": {
        "descriptionOfRestrictions": [
          {
            "value": "Sito di Fiorano Emil \u2013 linea piastrelle\r\nvia Ghiarola Nuova n\u00b0 29 \u2013 41042 Fiorano M.se (MO), Italia",
            "lang": "en"
          }
        ],
        "location": "GLO"
      }
    },
    "technology": {
      "technologyDescriptionAndIncludedProcesses": [
        {
          "value": "Il processo produttivo del sito di Fiorano Emil \u00e8 un ciclo parziale che ha inizio con la fase di pressatura dell\u2019atomizzato ricevuto dagli altri stabilimenti di Marazzi Group S.r.l. e Emilceramica S.r.l. Ingresso, stoccaggio ed immissione in produzione delle materie prime; Macinazione delle materie prime; Atomizzazione; Pressatura ed Essiccamento; Cottura; Squadratura, scelta e confezionamento; Magazzino spedizioni.",
          "lang": "en"
        }
      ],
      "technologicalApplicability": [
        {
          "value": "Ceramic tiles, object of this study, are intended to be applied to both floor and wall claddings and to be installed both indoors and outdoors for residential, non-residential and commercial use.",
          "lang": "en"
        }
      ],
      "referenceToTechnologyFlowDiagrammOrPicture": [
        {
          "shortDescription": [
            {
              "value": "EPDITALY0102 flowchart",
              "lang": "en"
            }
          ],
          "type": "source data set",
          "refObjectId": "03ff86c3-3410-4007-b2f4-77edc3c00f6f",
          "version": "00.00.003"
        }
      ]
    }
  },
  "modellingAndValidation": {
    "LCIMethodAndAllocation": {
      "typeOfDataSet": "EPD",
      "referenceToLCAMethodDetails": [
        {
          "shortDescription": [
            {
              "value": "PCR ICMQ-001/15 rev2.1",
              "lang": "en"
            }
          ],
          "type": "source data set",
          "refObjectId": "bc34cb82-81d9-4dde-9791-c1f91218a52f",
          "version": "00.00.002"
        }
      ],
      "other": {
        "anies": [
          {
            "name": "subType",
            "value": "average dataset"
          }
        ]
      }
    },
    "dataSourcesTreatmentAndRepresentativeness": {
      "referenceToDataSource": [
        {
          "shortDescription": [
            {
              "value": "GaBi database (general)",
              "lang": "en"
            }
          ],
          "type": "source data set",
          "refObjectId": "28d74cc0-db8b-4d7e-bc44-5f6d56ce0c4a",
          "version": "00.03.002"
        },
        {
          "shortDescription": [
            {
              "value": "GaBi database SP36 2018",
              "lang": "en"
            }
          ],
          "type": "source data set",
          "refObjectId": "dad5023c-8d97-4656-b82a-2fc6480b33a7",
          "version": "00.00.001",
          "uri": "feda7597-12a1-4bd5-93ef-4d8120877b78"
        }
      ],
      "other": {
        "anies": [
          {
            "name": "referenceToOriginalEPD",
            "value": {
              "shortDescription": {
                "value": "EPDITALY0102 PDF",
                "defaultValue": "EPDITALY0102 PDF",
                "lstrings": [
                  {
                    "lang": "en",
                    "value": "EPDITALY0102 PDF"
                  }
                ]
              },
              "version": {
                "version": 3,
                "majorVersion": 0,
                "minorVersion": 0,
                "subMinorVersion": 3,
                "zero": false,
                "versionString": "00.00.003"
              },
              "type": "source data set",
              "uuid": {
                "uuid": "8c6e4d2f-a9b1-4490-9a65-92060f999196"
              },
              "refObjectId": "8c6e4d2f-a9b1-4490-9a65-92060f999196",
              "versionAsString": "00.00.003",
              "resourceURLs": [
                "https://node.epditaly.it/resource/sources/8c6e4d2f-a9b1-4490-9a65-92060f999196/EPDITALY0102_EN.pdf?version=00.00.003"
              ]
            }
          }
        ]
      }
    },
    "validation": {
      "review": [
        {
          "referenceToNameOfReviewerAndInstitution": [
            {
              "shortDescription": [
                {
                  "value": "ICMQ S.p.A.",
                  "lang": "en"
                }
              ],
              "type": "contact data set",
              "refObjectId": "6a2483f7-d823-4b36-ab56-f3b5bbaa976a",
              "version": "00.00.001"
            }
          ],
          "type": "Accredited third party review"
        }
      ]
    },
    "complianceDeclarations": {
      "compliance": [
        {
          "referenceToComplianceSystem": {
            "shortDescription": [
              {
                "value": "ISO 14025",
                "lang": "en"
              }
            ],
            "type": "source data set",
            "refObjectId": "4f2eb655-6e44-4874-a95a-e28f5442cd4d",
            "version": "00.00.001"
          }
        },
        {
          "referenceToComplianceSystem": {
            "shortDescription": [
              {
                "value": "EN 15804",
                "lang": "de"
              }
            ],
            "type": "source data set",
            "refObjectId": "b00f9ec0-7874-11e3-981f-0800200c9a66",
            "version": "00.02.000"
          }
        }
      ]
    }
  },
  "administrativeInformation": {
    "dataEntryBy": {
      "timeStamp": 1646761412957,
      "referenceToDataSetFormat": [
        {
          "shortDescription": [
            {
              "value": "EPD Data Format Extension",
              "lang": "de"
            }
          ],
          "type": "source data set",
          "refObjectId": "cba73800-7874-11e3-981f-0800200c9a66",
          "version": "00.01.000"
        },
        {
          "shortDescription": [
            {
              "value": "ILCD format",
              "lang": "en"
            }
          ],
          "type": "source data set",
          "refObjectId": "a97a0155-0234-4b87-b4ce-a45da52f2a40",
          "version": "01.00.000",
          "uri": "http://lca.jrc.ec.europa.eu/lcainfohub/sample_data/ilcd/sources/ILCD_Format_a97a0155-0234-4b87-b4ce-a45da52f2a40_01.00.000.xml"
        },
        {
          "shortDescription": [
            {
              "value": "EPD Data Format Extensions v1.2",
              "lang": "en"
            },
            {
              "value": "EPD-Datenformaterweiterungen v1.2",
              "lang": "de"
            }
          ],
          "type": "source data set",
          "refObjectId": "a29449fd-aa2f-4de8-b5d7-4b06b43c6fde",
          "version": "00.01.000"
        }
      ]
    },
    "publicationAndOwnership": {
      "dataSetVersion": "00.00.025",
      "referenceToRegistrationAuthority": {
        "shortDescription": [
          {
            "value": "ICMQ S.p.A.",
            "lang": "en"
          }
        ],
        "type": "contact data set",
        "refObjectId": "6a2483f7-d823-4b36-ab56-f3b5bbaa976a",
        "version": "00.00.001"
      },
      "registrationNumber": "EPDITALY0102",
      "referenceToOwnershipOfDataSet": {
        "shortDescription": [
          {
            "value": "Marazzi Group Srl a socio unico",
            "lang": "en"
          }
        ],
        "type": "contact data set",
        "refObjectId": "9f2d54a4-6e2e-473b-a8fb-9f742e793ae7",
        "version": "00.00.002"
      },
      "other": {
        "anies": [
          {
            "name": "referenceToPublisher",
            "value": {
              "shortDescription": [
                {
                  "value": "EPDItaly",
                  "lang": "en"
                }
              ],
              "type": "contact data set",
              "refObjectId": "9433b9cf-1d4a-420f-8c09-88d2472225b9",
              "version": "00.00.001"
            }
          }
        ]
      }
    }
  },
  "exchanges": {
    "exchange": [
      {
        "dataSetInternalID": 1,
        "referenceToFlowDataSet": {
          "shortDescription": [
            {
              "value": "CERAMIC TILES 0102",
              "lang": "en"
            }
          ],
          "type": "flow data set",
          "refObjectId": "32c8c2e6-99cc-4ed6-ac0d-f0f74384e2ce",
          "version": "00.00.003"
        },
        "meanAmount": 1.0,
        "resultingAmount": 1.0,
        "referenceFlow": true,
        "resultingflowAmount": 1.0,
        "flowProperties": [
          {
            "name": [
              {
                "lang": "en",
                "value": "Area"
              },
              {
                "lang": "de",
                "value": "Fl\u00e4che"
              }
            ],
            "uuid": "93a60a56-a3c8-19da-a746-0800200c9a66",
            "referenceFlowProperty": true,
            "meanValue": 1.0,
            "referenceUnit": "qm",
            "unitGroupUUID": "c20a03d7-bd90-4569-bc94-66cfd364dfc8"
          }
        ],
        "materialProperties": [
          {
            "name": "grammage",
            "value": "22.6",
            "unit": "kg/m^2",
            "unitDescription": "kilograms per square metre"
          }
        ],
        "typeOfFlow": "Product flow"
      },
      {
        "dataSetInternalID": 2,
        "referenceToFlowDataSet": {
          "shortDescription": [
            {
              "value": "Components for re-use (CRU)",
              "lang": "en"
            },
            {
              "value": "Komponenten f\u00fcr die Wiederverwendung (CRU)",
              "lang": "de"
            },
            {
              "value": "Componentes para su reutilizaci\u00f3n (CRU)",
              "lang": "es"
            }
          ],
          "type": "flow data set",
          "refObjectId": "a2b32f97-3fc7-4af2-b209-525bc6426f33",
          "version": "30.00.000"
        },
        "exchange direction": "OUTPUT",
        "meanAmount": 0.0,
        "other": {
          "anies": [
            {
              "value": "0.0",
              "module": "A1-A3"
            },
            {
              "value": "0.0",
              "module": "A4"
            },
            {
              "value": "0.226",
              "module": "A5"
            },
            {
              "value": "0.0",
              "module": "B2"
            },
            {
              "value": "0.0",
              "module": "C2"
            },
            {
              "value": "0.0",
              "module": "C3"
            },
            {
              "value": "0.0",
              "module": "C4"
            },
            {
              "value": "0.0",
              "module": "D"
            },
            {
              "name": "referenceToUnitGroupDataSet",
              "value": {
                "shortDescription": [
                  {
                    "value": "kg"
                  }
                ],
                "type": "unit group data set",
                "refObjectId": "ad38d542-3fe9-439d-9b95-2f5f7752acaf",
                "uri": "../unitgroups/ad38d542-3fe9-439d-9b95-2f5f7752acaf"
              }
            }
          ]
        },
        "flowProperties": [],
        "typeOfFlow": "Other flow",
        "classification": {
          "classHierarchy": "Gr\u00f6\u00dfen / Umweltliche Gr\u00f6\u00dfen / EPD EN 15804 / LCI Indikatoren",
          "name": "GaBiCategories"
        }
      },
      {
        "dataSetInternalID": 3,
        "referenceToFlowDataSet": {
          "shortDescription": [
            {
              "value": "Exported electrical energy (EEE)",
              "lang": "en"
            },
            {
              "value": "Exportierte elektrische Energie (EEE)",
              "lang": "de"
            },
            {
              "value": "Energ\u00eda exportada electrica (EEE)",
              "lang": "es"
            }
          ],
          "type": "flow data set",
          "refObjectId": "4da0c987-2b76-40d6-9e9e-82a017aaaf29",
          "version": "30.00.000"
        },
        "exchange direction": "OUTPUT",
        "meanAmount": 0.0,
        "other": {
          "anies": [
            {
              "value": "0.0",
              "module": "A1-A3"
            },
            {
              "value": "0.0",
              "module": "A4"
            },
            {
              "value": "0.603",
              "module": "A5"
            },
            {
              "value": "0.0",
              "module": "B2"
            },
            {
              "value": "0.0",
              "module": "C2"
            },
            {
              "value": "0.0",
              "module": "C3"
            },
            {
              "value": "0.0",
              "module": "C4"
            },
            {
              "value": "0.0",
              "module": "D"
            },
            {
              "name": "referenceToUnitGroupDataSet",
              "value": {
                "shortDescription": [
                  {
                    "value": "MJ"
                  }
                ],
                "type": "unit group data set",
                "refObjectId": "93a60a57-a3c8-11da-a746-0800200c9a66",
                "uri": "../unitgroups/93a60a57-a3c8-11da-a746-0800200c9a66"
              }
            }
          ]
        },
        "flowProperties": [],
        "typeOfFlow": "Other flow",
        "classification": {
          "classHierarchy": "Gr\u00f6\u00dfen / Umweltliche Gr\u00f6\u00dfen / EPD EN 15804 / LCI Indikatoren",
          "name": "GaBiCategories"
        }
      },
      {
        "dataSetInternalID": 4,
        "referenceToFlowDataSet": {
          "shortDescription": [
            {
              "value": "Exported thermal energy (EET)",
              "lang": "en"
            },
            {
              "value": "Exportierte thermische Energie (EET)",
              "lang": "de"
            },
            {
              "value": "Energ\u00eda exportada termal (EET)",
              "lang": "es"
            }
          ],
          "type": "flow data set",
          "refObjectId": "98daf38a-7a79-46d3-9a37-2b7bd0955810",
          "version": "30.00.000"
        },
        "exchange direction": "OUTPUT",
        "meanAmount": 0.0,
        "other": {
          "anies": [
            {
              "value": "0.0",
              "module": "A1-A3"
            },
            {
              "value": "0.0",
              "module": "A4"
            },
            {
              "value": "0.851",
              "module": "A5"
            },
            {
              "value": "0.0",
              "module": "B2"
            },
            {
              "value": "0.0",
              "module": "C2"
            },
            {
              "value": "0.0",
              "module": "C3"
            },
            {
              "value": "0.0",
              "module": "C4"
            },
            {
              "value": "0.0",
              "module": "D"
            },
            {
              "name": "referenceToUnitGroupDataSet",
              "value": {
                "shortDescription": [
                  {
                    "value": "MJ"
                  }
                ],
                "type": "unit group data set",
                "refObjectId": "93a60a57-a3c8-11da-a746-0800200c9a66",
                "uri": "../unitgroups/93a60a57-a3c8-11da-a746-0800200c9a66"
              }
            }
          ]
        },
        "flowProperties": [],
        "typeOfFlow": "Other flow",
        "classification": {
          "classHierarchy": "Gr\u00f6\u00dfen / Umweltliche Gr\u00f6\u00dfen / EPD EN 15804 / LCI Indikatoren",
          "name": "GaBiCategories"
        }
      },
      {
        "dataSetInternalID": 5,
        "referenceToFlowDataSet": {
          "shortDescription": [
            {
              "value": "Hazardous waste disposed (HWD)",
              "lang": "en"
            },
            {
              "value": "Gef\u00e4hrlicher Abfall zur Deponie (HWD)",
              "lang": "de"
            },
            {
              "value": "Residuos peligrosos eliminados (HWD)",
              "lang": "es"
            }
          ],
          "type": "flow data set",
          "refObjectId": "430f9e0f-59b2-46a0-8e0d-55e0e84948fc",
          "version": "30.00.000"
        },
        "exchange direction": "OUTPUT",
        "meanAmount": 0.0,
        "other": {
          "anies": [
            {
              "value": "9.04E-7",
              "module": "A1-A3"
            },
            {
              "value": "3.49E-7",
              "module": "A4"
            },
            {
              "value": "2.03E-7",
              "module": "A5"
            },
            {
              "value": "1.34E-10",
              "module": "B2"
            },
            {
              "value": "7.92E-8",
              "module": "C2"
            },
            {
              "value": "3.3E-8",
              "module": "C3"
            },
            {
              "value": "3.15E-8",
              "module": "C4"
            },
            {
              "value": "-1.36E-8",
              "module": "D"
            },
            {
              "name": "referenceToUnitGroupDataSet",
              "value": {
                "shortDescription": [
                  {
                    "value": "kg"
                  }
                ],
                "type": "unit group data set",
                "refObjectId": "ad38d542-3fe9-439d-9b95-2f5f7752acaf",
                "uri": "../unitgroups/ad38d542-3fe9-439d-9b95-2f5f7752acaf"
              }
            }
          ]
        },
        "flowProperties": [],
        "typeOfFlow": "Other flow",
        "classification": {
          "classHierarchy": "Gr\u00f6\u00dfen / Umweltliche Gr\u00f6\u00dfen / EPD EN 15804 / LCI Indikatoren",
          "name": "GaBiCategories"
        }
      },
      {
        "dataSetInternalID": 6,
        "referenceToFlowDataSet": {
          "shortDescription": [
            {
              "value": "Materials for energy recovery (MER)",
              "lang": "en"
            },
            {
              "value": "Stoffe f\u00fcr die Energier\u00fcckgewinnung (MER)",
              "lang": "de"
            },
            {
              "value": "Materiales para valorizaci\u00f3n energ\u00e9tica (recuperaci\u00f3n de energ\u00eda) (MER)",
              "lang": "es"
            }
          ],
          "type": "flow data set",
          "refObjectId": "59a9181c-3aaf-46ee-8b13-2b3723b6e447",
          "version": "30.00.000"
        },
        "exchange direction": "OUTPUT",
        "meanAmount": 0.0,
        "other": {
          "anies": [
            {
              "value": "0.0",
              "module": "A1-A3"
            },
            {
              "value": "0.0",
              "module": "A4"
            },
            {
              "value": "0.0",
              "module": "A5"
            },
            {
              "value": "0.0",
              "module": "B2"
            },
            {
              "value": "0.0",
              "module": "C2"
            },
            {
              "value": "0.0",
              "module": "C3"
            },
            {
              "value": "0.0",
              "module": "C4"
            },
            {
              "value": "0.0",
              "module": "D"
            },
            {
              "name": "referenceToUnitGroupDataSet",
              "value": {
                "shortDescription": [
                  {
                    "value": "kg"
                  }
                ],
                "type": "unit group data set",
                "refObjectId": "ad38d542-3fe9-439d-9b95-2f5f7752acaf",
                "uri": "../unitgroups/ad38d542-3fe9-439d-9b95-2f5f7752acaf"
              }
            }
          ]
        },
        "flowProperties": [],
        "typeOfFlow": "Other flow",
        "classification": {
          "classHierarchy": "Gr\u00f6\u00dfen / Umweltliche Gr\u00f6\u00dfen / EPD EN 15804 / LCI Indikatoren",
          "name": "GaBiCategories"
        }
      },
      {
        "dataSetInternalID": 7,
        "referenceToFlowDataSet": {
          "shortDescription": [
            {
              "value": "Materials for recycling (MFR)",
              "lang": "en"
            },
            {
              "value": "Stoffe zum Recycling (MFR)",
              "lang": "de"
            },
            {
              "value": "Materiales para el reciclaje (MFR)",
              "lang": "es"
            }
          ],
          "type": "flow data set",
          "refObjectId": "d7fe48a5-4103-49c8-9aae-b0b5dfdbd6ae",
          "version": "30.00.000"
        },
        "exchange direction": "OUTPUT",
        "meanAmount": 0.0,
        "other": {
          "anies": [
            {
              "value": "2.08",
              "module": "A1-A3"
            },
            {
              "value": "0.0",
              "module": "A4"
            },
            {
              "value": "0.229",
              "module": "A5"
            },
            {
              "value": "0.0",
              "module": "B2"
            },
            {
              "value": "0.0",
              "module": "C2"
            },
            {
              "value": "20.0",
              "module": "C3"
            },
            {
              "value": "0.0",
              "module": "C4"
            },
            {
              "value": "0.0",
              "module": "D"
            },
            {
              "name": "referenceToUnitGroupDataSet",
              "value": {
                "shortDescription": [
                  {
                    "value": "kg"
                  }
                ],
                "type": "unit group data set",
                "refObjectId": "ad38d542-3fe9-439d-9b95-2f5f7752acaf",
                "uri": "../unitgroups/ad38d542-3fe9-439d-9b95-2f5f7752acaf"
              }
            }
          ]
        },
        "flowProperties": [],
        "typeOfFlow": "Other flow",
        "classification": {
          "classHierarchy": "Gr\u00f6\u00dfen / Umweltliche Gr\u00f6\u00dfen / EPD EN 15804 / LCI Indikatoren",
          "name": "GaBiCategories"
        }
      },
      {
        "dataSetInternalID": 8,
        "referenceToFlowDataSet": {
          "shortDescription": [
            {
              "value": "Non hazardous waste dispose (NHWD)",
              "lang": "en"
            },
            {
              "value": "Entsorgter nicht gef\u00e4hrlicher Abfall (NHWD)",
              "lang": "de"
            },
            {
              "value": "Residuos no peligrosos eliminados (NHWD)",
              "lang": "es"
            }
          ],
          "type": "flow data set",
          "refObjectId": "b29ef66b-e286-4afa-949f-62f1a7b4d7fa",
          "version": "30.00.000"
        },
        "exchange direction": "OUTPUT",
        "meanAmount": 0.0,
        "other": {
          "anies": [
            {
              "value": "0.352",
              "module": "A1-A3"
            },
            {
              "value": "5.37E-4",
              "module": "A4"
            },
            {
              "value": "2.68",
              "module": "A5"
            },
            {
              "value": "0.00507",
              "module": "B2"
            },
            {
              "value": "1.15E-4",
              "module": "C2"
            },
            {
              "value": "2.17E-4",
              "module": "C3"
            },
            {
              "value": "8.59",
              "module": "C4"
            },
            {
              "value": "-0.809",
              "module": "D"
            },
            {
              "name": "referenceToUnitGroupDataSet",
              "value": {
                "shortDescription": [
                  {
                    "value": "kg"
                  }
                ],
                "type": "unit group data set",
                "refObjectId": "ad38d542-3fe9-439d-9b95-2f5f7752acaf",
                "uri": "../unitgroups/ad38d542-3fe9-439d-9b95-2f5f7752acaf"
              }
            }
          ]
        },
        "flowProperties": [],
        "typeOfFlow": "Other flow",
        "classification": {
          "classHierarchy": "Gr\u00f6\u00dfen / Umweltliche Gr\u00f6\u00dfen / EPD EN 15804 / LCI Indikatoren",
          "name": "GaBiCategories"
        }
      },
      {
        "dataSetInternalID": 9,
        "referenceToFlowDataSet": {
          "shortDescription": [
            {
              "value": "Radioactive waste disposed (RWD)",
              "lang": "en"
            },
            {
              "value": "Entsorgter radioaktiver Abfall (RWD)",
              "lang": "de"
            },
            {
              "value": "Residuos radiactivos eliminados (RWD)",
              "lang": "es"
            }
          ],
          "type": "flow data set",
          "refObjectId": "3449546e-52ad-4b39-b809-9fb77cea8ff6",
          "version": "30.00.000"
        },
        "exchange direction": "OUTPUT",
        "meanAmount": 0.0,
        "other": {
          "anies": [
            {
              "value": "0.00283",
              "module": "A1-A3"
            },
            {
              "value": "1.42E-5",
              "module": "A4"
            },
            {
              "value": "1.97E-4",
              "module": "A5"
            },
            {
              "value": "4.78E-6",
              "module": "B2"
            },
            {
              "value": "1.92E-6",
              "module": "C2"
            },
            {
              "value": "1.57E-5",
              "module": "C3"
            },
            {
              "value": "2.48E-5",
              "module": "C4"
            },
            {
              "value": "-2.74E-5",
              "module": "D"
            },
            {
              "name": "referenceToUnitGroupDataSet",
              "value": {
                "shortDescription": [
                  {
                    "value": "kg"
                  }
                ],
                "type": "unit group data set",
                "refObjectId": "ad38d542-3fe9-439d-9b95-2f5f7752acaf",
                "uri": "../unitgroups/ad38d542-3fe9-439d-9b95-2f5f7752acaf"
              }
            }
          ]
        },
        "flowProperties": [],
        "typeOfFlow": "Other flow",
        "classification": {
          "classHierarchy": "Gr\u00f6\u00dfen / Umweltliche Gr\u00f6\u00dfen / EPD EN 15804 / LCI Indikatoren",
          "name": "GaBiCategories"
        }
      },
      {
        "dataSetInternalID": 10,
        "referenceToFlowDataSet": {
          "shortDescription": [
            {
              "value": "Total use of non renewable primary energy resource (PENRT)",
              "lang": "en"
            },
            {
              "value": "Total nicht erneuerbare Prim\u00e4renergie (PENRT)",
              "lang": "de"
            },
            {
              "value": "Uso total de la energ\u00eda primaria no renovable (energ\u00eda primaria y recursos de energ\u00eda primaria renovable utilizada como materia prima) (PENRT)",
              "lang": "es"
            }
          ],
          "type": "flow data set",
          "refObjectId": "06159210-646b-4c8d-8583-da9b3b95a6c1",
          "version": "30.00.000"
        },
        "exchange direction": "INPUT",
        "meanAmount": 0.0,
        "other": {
          "anies": [
            {
              "value": "194.0",
              "module": "A1-A3"
            },
            {
              "value": "7.41",
              "module": "A4"
            },
            {
              "value": "17.1",
              "module": "A5"
            },
            {
              "value": "0.193",
              "module": "B2"
            },
            {
              "value": "1.42",
              "module": "C2"
            },
            {
              "value": "1.02",
              "module": "C3"
            },
            {
              "value": "1.85",
              "module": "C4"
            },
            {
              "value": "-0.631",
              "module": "D"
            },
            {
              "name": "referenceToUnitGroupDataSet",
              "value": {
                "shortDescription": [
                  {
                    "value": "MJ"
                  }
                ],
                "type": "unit group data set",
                "refObjectId": "93a60a57-a3c8-11da-a746-0800200c9a66",
                "uri": "../unitgroups/93a60a57-a3c8-11da-a746-0800200c9a66"
              }
            }
          ]
        },
        "flowProperties": [],
        "typeOfFlow": "Other flow",
        "classification": {
          "classHierarchy": "Gr\u00f6\u00dfen / Umweltliche Gr\u00f6\u00dfen / EPD EN 15804 / LCI Indikatoren",
          "name": "GaBiCategories"
        }
      },
      {
        "dataSetInternalID": 11,
        "referenceToFlowDataSet": {
          "shortDescription": [
            {
              "value": "Total use of renewable primary energy resources (PERT)",
              "lang": "en"
            },
            {
              "value": "Total erneuerbare Prim\u00e4renergie (PERT)",
              "lang": "de"
            },
            {
              "value": "Uso total de la energ\u00eda primaria renovable (energ\u00eda primaria y recursos de energ\u00eda primaria renovable utilizada como materia prima) (PERT)",
              "lang": "es"
            }
          ],
          "type": "flow data set",
          "refObjectId": "53f97275-fa8a-4cdd-9024-65936002acd0",
          "version": "30.00.000"
        },
        "exchange direction": "INPUT",
        "meanAmount": 0.0,
        "other": {
          "anies": [
            {
              "value": "40.8",
              "module": "A1-A3"
            },
            {
              "value": "0.377",
              "module": "A4"
            },
            {
              "value": "5.09",
              "module": "A5"
            },
            {
              "value": "0.0166",
              "module": "B2"
            },
            {
              "value": "0.0822",
              "module": "C2"
            },
            {
              "value": "0.0687",
              "module": "C3"
            },
            {
              "value": "0.234",
              "module": "C4"
            },
            {
              "value": "-0.183",
              "module": "D"
            },
            {
              "name": "referenceToUnitGroupDataSet",
              "value": {
                "shortDescription": [
                  {
                    "value": "MJ"
                  }
                ],
                "type": "unit group data set",
                "refObjectId": "93a60a57-a3c8-11da-a746-0800200c9a66",
                "uri": "../unitgroups/93a60a57-a3c8-11da-a746-0800200c9a66"
              }
            }
          ]
        },
        "flowProperties": [],
        "typeOfFlow": "Other flow",
        "classification": {
          "classHierarchy": "Gr\u00f6\u00dfen / Umweltliche Gr\u00f6\u00dfen / EPD EN 15804 / LCI Indikatoren",
          "name": "GaBiCategories"
        }
      },
      {
        "dataSetInternalID": 12,
        "referenceToFlowDataSet": {
          "shortDescription": [
            {
              "value": "Use of net fresh water (FW)",
              "lang": "en"
            },
            {
              "value": "Einsatz von S\u00fc\u00dfwasserressourcen (FW)",
              "lang": "de"
            },
            {
              "value": "Uso neto de recursos de agua dulce (FW)",
              "lang": "es"
            }
          ],
          "type": "flow data set",
          "refObjectId": "3cf952c8-f3a4-461d-8c96-96456ca62246",
          "version": "30.00.000"
        },
        "exchange direction": "INPUT",
        "meanAmount": 0.0,
        "other": {
          "anies": [
            {
              "value": "0.292",
              "module": "A1-A3"
            },
            {
              "value": "6.36E-4",
              "module": "A4"
            },
            {
              "value": "0.0219",
              "module": "A5"
            },
            {
              "value": "6.37E-5",
              "module": "B2"
            },
            {
              "value": "1.39E-4",
              "module": "C2"
            },
            {
              "value": "3.1E-4",
              "module": "C3"
            },
            {
              "value": "4.66E-4",
              "module": "C4"
            },
            {
              "value": "-1.38E-4",
              "module": "D"
            },
            {
              "name": "referenceToUnitGroupDataSet",
              "value": {
                "shortDescription": [
                  {
                    "value": "m3"
                  }
                ],
                "type": "unit group data set",
                "refObjectId": "cd950537-0a98-4044-9ba7-9f9a68d0a504",
                "uri": "../unitgroups/cd950537-0a98-4044-9ba7-9f9a68d0a504"
              }
            }
          ]
        },
        "flowProperties": [],
        "typeOfFlow": "Other flow",
        "classification": {
          "classHierarchy": "Gr\u00f6\u00dfen / Umweltliche Gr\u00f6\u00dfen / EPD EN 15804 / LCI Indikatoren",
          "name": "GaBiCategories"
        }
      },
      {
        "dataSetInternalID": 13,
        "referenceToFlowDataSet": {
          "shortDescription": [
            {
              "value": "Use of non renewable primary energy (PENRE)",
              "lang": "en"
            },
            {
              "value": "Nicht-erneuerbare Prim\u00e4renergie als Energietr\u00e4ger (PENRE)",
              "lang": "de"
            },
            {
              "value": "Uso de energ\u00eda primaria no renovable, excluyendo los recursos de energ\u00eda primaria no renovable utilizada como materia prima (PENRE)",
              "lang": "es"
            }
          ],
          "type": "flow data set",
          "refObjectId": "ac857178-2b45-46ec-892a-a9a4332f0372",
          "version": "30.00.000"
        },
        "exchange direction": "INPUT",
        "meanAmount": 0.0,
        "other": {
          "anies": [
            {
              "value": "193.0",
              "module": "A1-A3"
            },
            {
              "value": "7.41",
              "module": "A4"
            },
            {
              "value": "18.4",
              "module": "A5"
            },
            {
              "value": "0.193",
              "module": "B2"
            },
            {
              "value": "1.42",
              "module": "C2"
            },
            {
              "value": "1.02",
              "module": "C3"
            },
            {
              "value": "1.85",
              "module": "C4"
            },
            {
              "value": "-0.631",
              "module": "D"
            },
            {
              "name": "referenceToUnitGroupDataSet",
              "value": {
                "shortDescription": [
                  {
                    "value": "MJ"
                  }
                ],
                "type": "unit group data set",
                "refObjectId": "93a60a57-a3c8-11da-a746-0800200c9a66",
                "uri": "../unitgroups/93a60a57-a3c8-11da-a746-0800200c9a66"
              }
            }
          ]
        },
        "flowProperties": [],
        "typeOfFlow": "Other flow",
        "classification": {
          "classHierarchy": "Gr\u00f6\u00dfen / Umweltliche Gr\u00f6\u00dfen / EPD EN 15804 / LCI Indikatoren",
          "name": "GaBiCategories"
        }
      },
      {
        "dataSetInternalID": 14,
        "referenceToFlowDataSet": {
          "shortDescription": [
            {
              "value": "Use of non renewable primary energy resources used as raw materials (PENRM)",
              "lang": "en"
            },
            {
              "value": "Nicht-erneuerbare Prim\u00e4renergie zur stofflichen Nutzung (PENRM)",
              "lang": "de"
            },
            {
              "value": "Uso de la energ\u00eda primaria no renovable utilizada como materia prima (PENRM)",
              "lang": "es"
            }
          ],
          "type": "flow data set",
          "refObjectId": "1421caa0-679d-4bf4-b282-0eb850ccae27",
          "version": "30.00.000"
        },
        "exchange direction": "INPUT",
        "meanAmount": 0.0,
        "other": {
          "anies": [
            {
              "value": "1.4",
              "module": "A1-A3"
            },
            {
              "value": "0.0",
              "module": "A4"
            },
            {
              "value": "-1.49",
              "module": "A5"
            },
            {
              "value": "0.0",
              "module": "B2"
            },
            {
              "value": "0.0",
              "module": "C2"
            },
            {
              "value": "0.0",
              "module": "C3"
            },
            {
              "value": "0.0",
              "module": "C4"
            },
            {
              "value": "0.0",
              "module": "D"
            },
            {
              "name": "referenceToUnitGroupDataSet",
              "value": {
                "shortDescription": [
                  {
                    "value": "MJ"
                  }
                ],
                "type": "unit group data set",
                "refObjectId": "93a60a57-a3c8-11da-a746-0800200c9a66",
                "uri": "../unitgroups/93a60a57-a3c8-11da-a746-0800200c9a66"
              }
            }
          ]
        },
        "flowProperties": [],
        "typeOfFlow": "Other flow",
        "classification": {
          "classHierarchy": "Gr\u00f6\u00dfen / Umweltliche Gr\u00f6\u00dfen / EPD EN 15804 / LCI Indikatoren",
          "name": "GaBiCategories"
        }
      },
      {
        "dataSetInternalID": 15,
        "referenceToFlowDataSet": {
          "shortDescription": [
            {
              "value": "Use of non renewable secondary fuels (NRSF)",
              "lang": "en"
            },
            {
              "value": "Nicht erneuerbare Sekund\u00e4rbrennstoffe (NRSF)",
              "lang": "de"
            },
            {
              "value": "Uso de combustibles secundarios no renovables (NRSF)",
              "lang": "es"
            }
          ],
          "type": "flow data set",
          "refObjectId": "89def144-d39a-4287-b86f-efde453ddcb2",
          "version": "30.00.000"
        },
        "exchange direction": "INPUT",
        "meanAmount": 0.0,
        "other": {
          "anies": [
            {
              "value": "0.0",
              "module": "A1-A3"
            },
            {
              "value": "0.0",
              "module": "A4"
            },
            {
              "value": "0.0",
              "module": "A5"
            },
            {
              "value": "0.0",
              "module": "B2"
            },
            {
              "value": "0.0",
              "module": "C2"
            },
            {
              "value": "0.0",
              "module": "C3"
            },
            {
              "value": "0.0",
              "module": "C4"
            },
            {
              "value": "0.0",
              "module": "D"
            },
            {
              "name": "referenceToUnitGroupDataSet",
              "value": {
                "shortDescription": [
                  {
                    "value": "MJ"
                  }
                ],
                "type": "unit group data set",
                "refObjectId": "93a60a57-a3c8-11da-a746-0800200c9a66",
                "uri": "../unitgroups/93a60a57-a3c8-11da-a746-0800200c9a66"
              }
            }
          ]
        },
        "flowProperties": [],
        "typeOfFlow": "Other flow",
        "classification": {
          "classHierarchy": "Gr\u00f6\u00dfen / Umweltliche Gr\u00f6\u00dfen / EPD EN 15804 / LCI Indikatoren",
          "name": "GaBiCategories"
        }
      },
      {
        "dataSetInternalID": 16,
        "referenceToFlowDataSet": {
          "shortDescription": [
            {
              "value": "Use of renewable primary energy (PERE)",
              "lang": "en"
            },
            {
              "value": "Erneuerbare Prim\u00e4renergie als Energietr\u00e4ger (PERE)",
              "lang": "de"
            },
            {
              "value": "Uso de energ\u00eda primaria renovable excluyendo los recursos de energ\u00eda primaria renovable utilizada como materia prima (PERE)",
              "lang": "es"
            }
          ],
          "type": "flow data set",
          "refObjectId": "20f32be5-0398-4288-9b6d-accddd195317",
          "version": "30.00.000"
        },
        "exchange direction": "INPUT",
        "meanAmount": 0.0,
        "other": {
          "anies": [
            {
              "value": "32.9",
              "module": "A1-A3"
            },
            {
              "value": "0.377",
              "module": "A4"
            },
            {
              "value": "12.4",
              "module": "A5"
            },
            {
              "value": "0.0166",
              "module": "B2"
            },
            {
              "value": "0.0822",
              "module": "C2"
            },
            {
              "value": "0.0687",
              "module": "C3"
            },
            {
              "value": "0.234",
              "module": "C4"
            },
            {
              "value": "-0.183",
              "module": "D"
            },
            {
              "name": "referenceToUnitGroupDataSet",
              "value": {
                "shortDescription": [
                  {
                    "value": "MJ"
                  }
                ],
                "type": "unit group data set",
                "refObjectId": "93a60a57-a3c8-11da-a746-0800200c9a66",
                "uri": "../unitgroups/93a60a57-a3c8-11da-a746-0800200c9a66"
              }
            }
          ]
        },
        "flowProperties": [],
        "typeOfFlow": "Other flow",
        "classification": {
          "classHierarchy": "Gr\u00f6\u00dfen / Umweltliche Gr\u00f6\u00dfen / EPD EN 15804 / LCI Indikatoren",
          "name": "GaBiCategories"
        }
      },
      {
        "dataSetInternalID": 17,
        "referenceToFlowDataSet": {
          "shortDescription": [
            {
              "value": "Use of renewable primary energy resources used as raw materials (PERM)",
              "lang": "en"
            },
            {
              "value": "Erneuerbare Prim\u00e4renergie zur stofflichen Nutzung (PERM)",
              "lang": "de"
            },
            {
              "value": "Uso de energ\u00eda primaria renovable utilizada como materia prima (PERM)",
              "lang": "es"
            }
          ],
          "type": "flow data set",
          "refObjectId": "fb3ec0de-548d-4508-aea5-00b73bf6f702",
          "version": "30.00.000"
        },
        "exchange direction": "INPUT",
        "meanAmount": 0.0,
        "other": {
          "anies": [
            {
              "value": "7.86",
              "module": "A1-A3"
            },
            {
              "value": "0.0",
              "module": "A4"
            },
            {
              "value": "-8.37",
              "module": "A5"
            },
            {
              "value": "0.0",
              "module": "B2"
            },
            {
              "value": "0.0",
              "module": "C2"
            },
            {
              "value": "0.0",
              "module": "C3"
            },
            {
              "value": "0.0",
              "module": "C4"
            },
            {
              "value": "0.0",
              "module": "D"
            },
            {
              "name": "referenceToUnitGroupDataSet",
              "value": {
                "shortDescription": [
                  {
                    "value": "MJ"
                  }
                ],
                "type": "unit group data set",
                "refObjectId": "93a60a57-a3c8-11da-a746-0800200c9a66",
                "uri": "../unitgroups/93a60a57-a3c8-11da-a746-0800200c9a66"
              }
            }
          ]
        },
        "flowProperties": [],
        "typeOfFlow": "Other flow",
        "classification": {
          "classHierarchy": "Gr\u00f6\u00dfen / Umweltliche Gr\u00f6\u00dfen / EPD EN 15804 / LCI Indikatoren",
          "name": "GaBiCategories"
        }
      },
      {
        "dataSetInternalID": 18,
        "referenceToFlowDataSet": {
          "shortDescription": [
            {
              "value": "Use of renewable secondary fuels (RSF)",
              "lang": "en"
            },
            {
              "value": "Erneuerbare Sekund\u00e4rbrennstoffe (RSF)",
              "lang": "de"
            },
            {
              "value": "Uso de combustibles secundarios renovables (RSF)",
              "lang": "es"
            }
          ],
          "type": "flow data set",
          "refObjectId": "64333088-a55f-4aa2-9a31-c10b07816787",
          "version": "30.00.000"
        },
        "exchange direction": "INPUT",
        "meanAmount": 0.0,
        "other": {
          "anies": [
            {
              "value": "0.0",
              "module": "A1-A3"
            },
            {
              "value": "0.0",
              "module": "A4"
            },
            {
              "value": "0.0",
              "module": "A5"
            },
            {
              "value": "0.0",
              "module": "B2"
            },
            {
              "value": "0.0",
              "module": "C2"
            },
            {
              "value": "0.0",
              "module": "C3"
            },
            {
              "value": "0.0",
              "module": "C4"
            },
            {
              "value": "0.0",
              "module": "D"
            },
            {
              "name": "referenceToUnitGroupDataSet",
              "value": {
                "shortDescription": [
                  {
                    "value": "MJ"
                  }
                ],
                "type": "unit group data set",
                "refObjectId": "93a60a57-a3c8-11da-a746-0800200c9a66",
                "uri": "../unitgroups/93a60a57-a3c8-11da-a746-0800200c9a66"
              }
            }
          ]
        },
        "flowProperties": [],
        "typeOfFlow": "Other flow",
        "classification": {
          "classHierarchy": "Gr\u00f6\u00dfen / Umweltliche Gr\u00f6\u00dfen / EPD EN 15804 / LCI Indikatoren",
          "name": "GaBiCategories"
        }
      },
      {
        "dataSetInternalID": 19,
        "referenceToFlowDataSet": {
          "shortDescription": [
            {
              "value": "Use of secondary material (SM)",
              "lang": "en"
            },
            {
              "value": "Einsatz von Sekund\u00e4rstoffen (SM)",
              "lang": "de"
            },
            {
              "value": "Uso de materiales secundarios (SM)",
              "lang": "es"
            }
          ],
          "type": "flow data set",
          "refObjectId": "c6a1f35f-2d09-4f54-8dfb-97e502e1ce92",
          "version": "30.00.000"
        },
        "exchange direction": "INPUT",
        "meanAmount": 0.0,
        "other": {
          "anies": [
            {
              "value": "1.53",
              "module": "A1-A3"
            },
            {
              "value": "0.0",
              "module": "A4"
            },
            {
              "value": "0.184",
              "module": "A5"
            },
            {
              "value": "0.0",
              "module": "B2"
            },
            {
              "value": "0.0",
              "module": "C2"
            },
            {
              "value": "0.0",
              "module": "C3"
            },
            {
              "value": "0.0",
              "module": "C4"
            },
            {
              "value": "19.4",
              "module": "D"
            },
            {
              "name": "referenceToUnitGroupDataSet",
              "value": {
                "shortDescription": [
                  {
                    "value": "kg"
                  }
                ],
                "type": "unit group data set",
                "refObjectId": "ad38d542-3fe9-439d-9b95-2f5f7752acaf",
                "uri": "../unitgroups/ad38d542-3fe9-439d-9b95-2f5f7752acaf"
              }
            }
          ]
        },
        "flowProperties": [],
        "typeOfFlow": "Other flow",
        "classification": {
          "classHierarchy": "Gr\u00f6\u00dfen / Umweltliche Gr\u00f6\u00dfen / EPD EN 15804 / LCI Indikatoren",
          "name": "GaBiCategories"
        }
      }
    ]
  },
  "LCIAResults": {
    "LCIAResult": [
      {
        "referenceToLCIAMethodDataSet": {
          "shortDescription": [
            {
              "value": "Abiotic depletion potential for fossil resources (ADPF)",
              "lang": "en"
            },
            {
              "value": "Potenzial f\u00fcr den abiotischen Abbau fossiler Brennstoffe (ADPF)",
              "lang": "de"
            },
            {
              "value": "Potencial de agotamiento de recursos abi\u00f3ticos para recursos f\u00f3siles (ADPF)",
              "lang": "es"
            }
          ],
          "type": "LCIA method data set",
          "refObjectId": "804ebcdf-309d-4098-8ed8-fdaf2f389981",
          "version": "00.01.000"
        },
        "meanAmount": 0.0,
        "other": {
          "anies": [
            {
              "value": "187.0",
              "module": "A1-A3"
            },
            {
              "value": "7.37",
              "module": "A4"
            },
            {
              "value": "16.6",
              "module": "A5"
            },
            {
              "value": "0.181",
              "module": "B2"
            },
            {
              "value": "1.41",
              "module": "C2"
            },
            {
              "value": "0.983",
              "module": "C3"
            },
            {
              "value": "1.79",
              "module": "C4"
            },
            {
              "value": "-0.562",
              "module": "D"
            },
            {
              "name": "referenceToUnitGroupDataSet",
              "value": {
                "shortDescription": [
                  {
                    "value": "MJ"
                  }
                ],
                "type": "unit group data set",
                "refObjectId": "93a60a57-a3c8-11da-a746-0800200c9a66",
                "uri": "../unitgroups/93a60a57-a3c8-11da-a746-0800200c9a66"
              }
            }
          ]
        }
      },
      {
        "referenceToLCIAMethodDataSet": {
          "shortDescription": [
            {
              "value": "Abiotic depletion potential for non fossil resources (ADPE)",
              "lang": "en"
            },
            {
              "value": "Potenzial f\u00fcr den abiotischen Abbau nicht fossiler Ressourcen (ADPE)",
              "lang": "de"
            },
            {
              "value": "Potencial de agotamiento de recursos abi\u00f3ticos para recursos no f\u00f3siles (ADPE)",
              "lang": "es"
            }
          ],
          "type": "LCIA method data set",
          "refObjectId": "f7c73bb9-ab1a-4249-9c6d-379a0de6f67e",
          "version": "00.01.000"
        },
        "meanAmount": 0.0,
        "other": {
          "anies": [
            {
              "value": "0.00149",
              "module": "A1-A3"
            },
            {
              "value": "4.26E-8",
              "module": "A4"
            },
            {
              "value": "1.01E-4",
              "module": "A5"
            },
            {
              "value": "5.03E-9",
              "module": "B2"
            },
            {
              "value": "8.03E-9",
              "module": "C2"
            },
            {
              "value": "6.68E-8",
              "module": "C3"
            },
            {
              "value": "4.7E-8",
              "module": "C4"
            },
            {
              "value": "-1.54E-8",
              "module": "D"
            },
            {
              "name": "referenceToUnitGroupDataSet",
              "value": {
                "shortDescription": [
                  {
                    "value": "kg Sb-\u00c4qv."
                  }
                ],
                "type": "unit group data set",
                "refObjectId": "54ccd2d9-a32a-4fc2-923d-f2c8c93e89d4",
                "uri": "../unitgroups/54ccd2d9-a32a-4fc2-923d-f2c8c93e89d4"
              }
            }
          ]
        }
      },
      {
        "referenceToLCIAMethodDataSet": {
          "shortDescription": [
            {
              "value": "Acidification potential of soil and water (AP)",
              "lang": "en"
            },
            {
              "value": "Versauerungspotenzial von Boden und Wasser (AP)",
              "lang": "de"
            },
            {
              "value": "Potencial de acidificaci\u00f3n del suelo y de los recursos de agua (AP)",
              "lang": "es"
            }
          ],
          "type": "LCIA method data set",
          "refObjectId": "b4274add-93b7-4905-a5e4-2e878c4e4216",
          "version": "00.01.000"
        },
        "meanAmount": 0.0,
        "other": {
          "anies": [
            {
              "value": "0.0391",
              "module": "A1-A3"
            },
            {
              "value": "0.00322",
              "module": "A4"
            },
            {
              "value": "0.00458",
              "module": "A5"
            },
            {
              "value": "1.65E-5",
              "module": "B2"
            },
            {
              "value": "4.45E-4",
              "module": "C2"
            },
            {
              "value": "3.61E-4",
              "module": "C3"
            },
            {
              "value": "7.65E-4",
              "module": "C4"
            },
            {
              "value": "-2.18E-4",
              "module": "D"
            },
            {
              "name": "referenceToUnitGroupDataSet",
              "value": {
                "shortDescription": [
                  {
                    "value": "kg SO2-\u00c4qv."
                  }
                ],
                "type": "unit group data set",
                "refObjectId": "bc50c624-a9bc-45b1-a9b0-e6b10d00476f",
                "uri": "../unitgroups/bc50c624-a9bc-45b1-a9b0-e6b10d00476f"
              }
            }
          ]
        }
      },
      {
        "referenceToLCIAMethodDataSet": {
          "shortDescription": [
            {
              "value": "Eutrophication potential (EP)",
              "lang": "en"
            },
            {
              "value": "Eutrophierungspotenzial (EP)",
              "lang": "de"
            },
            {
              "value": "Potencial de eutrofizaci\u00f3n (EP)",
              "lang": "es"
            }
          ],
          "type": "LCIA method data set",
          "refObjectId": "f58827d0-b407-4ec6-be75-8b69efb98a0f",
          "version": "00.01.000"
        },
        "meanAmount": 0.0,
        "other": {
          "anies": [
            {
              "value": "0.00418",
              "module": "A1-A3"
            },
            {
              "value": "3.9E-4",
              "module": "A4"
            },
            {
              "value": "7.78E-4",
              "module": "A5"
            },
            {
              "value": "2.69E-5",
              "module": "B2"
            },
            {
              "value": "1.13E-4",
              "module": "C2"
            },
            {
              "value": "8.69E-5",
              "module": "C3"
            },
            {
              "value": "8.67E-5",
              "module": "C4"
            },
            {
              "value": "-4.33E-5",
              "module": "D"
            },
            {
              "name": "referenceToUnitGroupDataSet",
              "value": {
                "shortDescription": [
                  {
                    "value": "kg Phosphat-\u00c4qv."
                  }
                ],
                "type": "unit group data set",
                "refObjectId": "67b5401d-873c-485f-bcf3-6ae83b918822",
                "uri": "../unitgroups/67b5401d-873c-485f-bcf3-6ae83b918822"
              }
            }
          ]
        }
      },
      {
        "referenceToLCIAMethodDataSet": {
          "shortDescription": [
            {
              "value": "Global warming potential (GWP)",
              "lang": "en"
            },
            {
              "value": "Globales Erw\u00e4rmungspotenzial (GWP)",
              "lang": "de"
            },
            {
              "value": "Potencial de calentamiento global (GWP)",
              "lang": "es"
            }
          ],
          "type": "LCIA method data set",
          "refObjectId": "77e416eb-a363-4258-a04e-171d843a6460",
          "version": "00.01.000"
        },
        "meanAmount": 0.0,
        "other": {
          "anies": [
            {
              "value": "11.7",
              "module": "A1-A3"
            },
            {
              "value": "0.552",
              "module": "A4"
            },
            {
              "value": "2.53",
              "module": "A5"
            },
            {
              "value": "0.0132",
              "module": "B2"
            },
            {
              "value": "0.103",
              "module": "C2"
            },
            {
              "value": "0.0506",
              "module": "C3"
            },
            {
              "value": "0.128",
              "module": "C4"
            },
            {
              "value": "-0.0467",
              "module": "D"
            },
            {
              "name": "referenceToUnitGroupDataSet",
              "value": {
                "shortDescription": [
                  {
                    "value": "kg CO2-\u00c4qv."
                  }
                ],
                "type": "unit group data set",
                "refObjectId": "1ebf3012-d0db-4de2-aefd-ef30cedb0be1",
                "uri": "../unitgroups/1ebf3012-d0db-4de2-aefd-ef30cedb0be1"
              }
            }
          ]
        }
      },
      {
        "referenceToLCIAMethodDataSet": {
          "shortDescription": [
            {
              "value": "Depletion potential of the stratospheric ozone layer (ODP)",
              "lang": "en"
            },
            {
              "value": "Abbau Potential der stratosph\u00e4rischen Ozonschicht (ODP)",
              "lang": "de"
            },
            {
              "value": "Potencial de agotamiento de la capa de ozono estratosf\u00e9rico (ODP)",
              "lang": "es"
            }
          ],
          "type": "LCIA method data set",
          "refObjectId": "06dcd26f-025f-401a-a7c1-5e457eb54637",
          "version": "00.01.000"
        },
        "meanAmount": 0.0,
        "other": {
          "anies": [
            {
              "value": "1.93E-12",
              "module": "A1-A3"
            },
            {
              "value": "1.26E-16",
              "module": "A4"
            },
            {
              "value": "1.21E-12",
              "module": "A5"
            },
            {
              "value": "6.32E-16",
              "module": "B2"
            },
            {
              "value": "1.72E-17",
              "module": "C2"
            },
            {
              "value": "2.27E-14",
              "module": "C3"
            },
            {
              "value": "7.42E-16",
              "module": "C4"
            },
            {
              "value": "-9.4E-16",
              "module": "D"
            },
            {
              "name": "referenceToUnitGroupDataSet",
              "value": {
                "shortDescription": [
                  {
                    "value": "kg R11-\u00c4qv."
                  }
                ],
                "type": "unit group data set",
                "refObjectId": "88054749-b0a6-47ea-a82b-dc5b29326512",
                "uri": "../unitgroups/88054749-b0a6-47ea-a82b-dc5b29326512"
              }
            }
          ]
        }
      },
      {
        "referenceToLCIAMethodDataSet": {
          "shortDescription": [
            {
              "value": "Formation potential of tropospheric ozone (POCP)",
              "lang": "en"
            },
            {
              "value": "Bildungspotential f\u00fcr troposph\u00e4risches Ozon (POCP)",
              "lang": "de"
            },
            {
              "value": "Potencial de formaci\u00f3n de ozono troposf\u00e9rico (POCP)",
              "lang": "es"
            }
          ],
          "type": "LCIA method data set",
          "refObjectId": "1e84a202-dae6-42aa-9e9d-71ea48b8be00",
          "version": "00.01.000"
        },
        "meanAmount": 0.0,
        "other": {
          "anies": [
            {
              "value": "0.00223",
              "module": "A1-A3"
            },
            {
              "value": "1.59E-4",
              "module": "A4"
            },
            {
              "value": "2.92E-4",
              "module": "A5"
            },
            {
              "value": "2.66E-6",
              "module": "B2"
            },
            {
              "value": "-1.84E-4",
              "module": "C2"
            },
            {
              "value": "3.94E-5",
              "module": "C3"
            },
            {
              "value": "5.87E-5",
              "module": "C4"
            },
            {
              "value": "-1.97E-5",
              "module": "D"
            },
            {
              "name": "referenceToUnitGroupDataSet",
              "value": {
                "shortDescription": [
                  {
                    "value": "kg Ethen-\u00c4qv."
                  }
                ],
                "type": "unit group data set",
                "refObjectId": "01c26c17-9a76-406e-8295-f17b55fd909e",
                "uri": "../unitgroups/01c26c17-9a76-406e-8295-f17b55fd909e"
              }
            }
          ]
        }
      }
    ]
  },
  "otherAttributes": {
    "{http://www.okworx.com/ILCD/Extensions/2018/Profile}profile": "EN_15804",
    "{http://www.indata.network/EPD/2019}epd-version": "1.2"
  },
  "version": "1.1",
  "source": "https://node.epditaly.it/resource/datastocks/24493f94-1ca8-4cc7-a056-67cbe25aef5a/processes/c1a9158c-d3a9-41f5-b7c2-5fe454e4f014"
}